@prefix : <http://w3id.org/emmo/domain/neo#> .
@prefix owl: <http://www.w3.org/2002/07/owl#> .
@prefix rdf: <http://www.w3.org/1999/02/22-rdf-syntax-ns#> .
@prefix xml: <http://www.w3.org/XML/1998/namespace> .
@prefix xsd: <http://www.w3.org/2001/XMLSchema#> .
@prefix rdfs: <http://www.w3.org/2000/01/rdf-schema#> .
@prefix elite: <http://w3id.org/emmo-lite#> .
@base <http://w3id.org/emmo/domain/neo#> .

<http://w3id.org/emmo/domain/neo/neo> rdf:type owl:Ontology ;
                                       owl:versionIRI <http://w3id.org/emmo/domain/neo/0.0.1/neo> ;
                                       owl:imports <http://w3id.org/emmo-lite/0.0.1> ;
                                       <http://purl.org/dc/terms/contributor> "Anna Anchini"@en ,
                                                                              "Dario Rimondini"@it ,
                                                                              "Francesco Antonio Zaccarini"@it ,
                                                                              "Ilaria Maria Paponetti"@it ,
                                                                              "Samuele Baldini"@it ,
                                                                              "Saverio Quaranta"@it ,
                                                                              """The Nuclear Energy Ontology (NEO) is a domain ontology developed under the EMMO framework for the representation of concepts in the field of nuclear energy. It is based on commonly used standardization vocabularies, such as:
    - ISO 12749 - Nuclear energy, nuclear technologies, and radiological protection
    - \"Construction Technologies for Nuclear Power Plants\", IAEA Nuclear Energy Series, No. NP-T-2.5, IAEA, Vienna (AU), 2011
    - IAEA Safety Glossary, Terminology Used in Nuclear Safety and Radiation Protection, 2018 Edition.

It includes the representation of the Fukushima Daichi accident, based on the official IAEA report: \"The Fukushima Daiichi accident - Technical Volume 1: Description and Context of the Accident\", IAEA, Vienna (AU), 2015, STI/PUB/1710, ISBN 978–92–0–107015–9

The ontology is still in development phase and provides a partial cover of the nuclear engineering domain and Fukushima Daichi accident report."""@en ;
                                       <http://purl.org/dc/terms/creator> "Emanuele Ghedini"@it ;
                                       <http://purl.org/dc/terms/license> "https://creativecommons.org/licenses/by/4.0/legalcode"^^xsd:anyURI ;
                                       <http://purl.org/dc/terms/title> "Nuclear Energy Ontology"@en .

#################################################################
#    Annotation properties
#################################################################

###  http://purl.org/dc/terms/abstract
<http://purl.org/dc/terms/abstract> rdf:type owl:AnnotationProperty .


###  http://purl.org/dc/terms/contributor
<http://purl.org/dc/terms/contributor> rdf:type owl:AnnotationProperty .


###  http://purl.org/dc/terms/creator
<http://purl.org/dc/terms/creator> rdf:type owl:AnnotationProperty .


###  http://purl.org/dc/terms/license
<http://purl.org/dc/terms/license> rdf:type owl:AnnotationProperty .


###  http://purl.org/dc/terms/title
<http://purl.org/dc/terms/title> rdf:type owl:AnnotationProperty .


###  http://w3id.org/emmo/domain/neo#R8xx0dhbEh1tjGMDwNZfckV
:R8xx0dhbEh1tjGMDwNZfckV rdf:type owl:AnnotationProperty ;
                         :R8xx0dhbEh1tjGMDwNZfckV "A short explanation aimed to guide the reader towards the intended interpretation of the ontological concept."@en ;
                         <http://www.w3.org/2004/02/skos/core#prefLabel> "definition"@en ;
                         rdfs:subPropertyOf rdfs:comment .


###  http://w3id.org/emmo/domain/neo#R9Q7fCgWnAkzqnVMtRJ4WDv
:R9Q7fCgWnAkzqnVMtRJ4WDv rdf:type owl:AnnotationProperty ;
                         :R8xx0dhbEh1tjGMDwNZfckV "A reference to real entities aimed to explain the intended interpretation for the ontological concept."@en ;
                         <http://www.w3.org/2004/02/skos/core#prefLabel> "example"@en ;
                         rdfs:subPropertyOf rdfs:comment .


###  http://w3id.org/emmo/domain/neo#RR3uD2d7YfhHohfv2Nm6sX
:RR3uD2d7YfhHohfv2Nm6sX rdf:type owl:AnnotationProperty ;
                        :R8xx0dhbEh1tjGMDwNZfckV "Additional text aimed to explain the conceptual choices of the authors."@en ;
                        <http://www.w3.org/2004/02/skos/core#prefLabel> "comment"@en ;
                        rdfs:subPropertyOf rdfs:comment .


###  http://www.w3.org/2000/01/rdf-schema#comment
rdfs:comment rdf:type owl:AnnotationProperty .


###  http://www.w3.org/2004/02/skos/core#altLabel
<http://www.w3.org/2004/02/skos/core#altLabel> rdf:type owl:AnnotationProperty ;
                                               rdfs:subPropertyOf rdfs:label .


###  http://www.w3.org/2004/02/skos/core#comment
<http://www.w3.org/2004/02/skos/core#comment> rdf:type owl:AnnotationProperty .


###  http://www.w3.org/2004/02/skos/core#definition
<http://www.w3.org/2004/02/skos/core#definition> rdf:type owl:AnnotationProperty .


###  http://www.w3.org/2004/02/skos/core#example
<http://www.w3.org/2004/02/skos/core#example> rdf:type owl:AnnotationProperty .


###  http://www.w3.org/2004/02/skos/core#prefLabel
<http://www.w3.org/2004/02/skos/core#prefLabel> rdf:type owl:AnnotationProperty ;
                                                rdfs:subPropertyOf rdfs:label .


#################################################################
#    Object Properties
#################################################################

###  http://w3id.org/emmo/domain/neo#RB4rNlczhggIx7lqdEK2d9c
:RB4rNlczhggIx7lqdEK2d9c rdf:type owl:ObjectProperty ;
                         rdfs:subPropertyOf elite:isConstituentOf ;
                         rdfs:comment "Defines the position of an object in a Nuclear Power Plant."@en ;
                         <http://www.w3.org/2004/02/skos/core#definition> "The spatial relation  between an entity and another the entity that contains it."@en ;
                         <http://www.w3.org/2004/02/skos/core#prefLabel> "isContainedBy"@en .


###  http://w3id.org/emmo/domain/neo#RBbSkE1mWA7Oq2RnEiKiOzM
:RBbSkE1mWA7Oq2RnEiKiOzM rdf:type owl:ObjectProperty ;
                         rdfs:subPropertyOf owl:topObjectProperty ;
                         rdfs:domain :RDZtzLsQmngV2BtJvmS5pbg ;
                         <http://www.w3.org/2004/02/skos/core#definition> "It relates the Nuclear Power Plant Workers to the place where they can enter, following safety requirements"@en ;
                         <http://www.w3.org/2004/02/skos/core#prefLabel> "CanAccessIn"@en .


#################################################################
#    Classes
#################################################################

###  http://w3id.org/emmo/domain/neo#R0N27qMQzeRjM0vSOeAvUT
:R0N27qMQzeRjM0vSOeAvUT rdf:type owl:Class ;
                        rdfs:subClassOf elite:Object ;
                        rdfs:comment "Nuclear power plant is a nuclear reactor or reactors together with all structures, systems and components necessary for safety and for the production of power, i.e. heat or electricity (ISO 12749-5:2018)."@en ;
                        rdfs:isDefinedBy <https://www.iso.org/obp/ui/#iso:std:iso:12749:-5:ed-1:v1:en:term:3.2.5> ;
                        rdfs:seeAlso <https://en.wikipedia.org/wiki/Nuclear_power_plant> ;
                        <http://www.w3.org/2004/02/skos/core#altLabel> "NPP"@en ;
                        <http://www.w3.org/2004/02/skos/core#definition> "A nuclear reactor installation that produces electrical and/or heat energy (ISO 12749-5:2018)."@en ;
                        <http://www.w3.org/2004/02/skos/core#prefLabel> "NuclearPowerPlant"@en .


###  http://w3id.org/emmo/domain/neo#R0ZnwwPdidaBfZOg6tgZJr
:R0ZnwwPdidaBfZOg6tgZJr rdf:type owl:Class ;
                        rdfs:subClassOf :R8hTHDGsCdkEbILOuzUhlEr ;
                        rdfs:comment "On the IAEA report is called \"reactor building\""@en ;
                        rdfs:isDefinedBy <https://aris.iaea.org/sites/Glossary.html> ;
                        <http://www.w3.org/2004/02/skos/core#altLabel> "ReactorBuilding"@en ;
                        <http://www.w3.org/2004/02/skos/core#definition> "A hermetically sealed building which houses the nuclear reactor core and other systems that could potentially release fission products to the atmosphere during an accident."@en ;
                        <http://www.w3.org/2004/02/skos/core#prefLabel> "ContainmentBuilding"@en .


###  http://w3id.org/emmo/domain/neo#R1DAH32q3UDTp3GZGqe5Re
:R1DAH32q3UDTp3GZGqe5Re rdf:type owl:Class ;
                        rdfs:subClassOf :RDpEA8qdRk99FAT0xSGZgGS ;
                        rdfs:isDefinedBy <https://en.wikipedia.org/wiki/Shutdown> ;
                        <http://www.w3.org/2004/02/skos/core#definition> "Shutdown is the state of a nuclear reactor when the fission reaction is slowed significantly or halted completely"@en ;
                        <http://www.w3.org/2004/02/skos/core#prefLabel> "NPPShutdown"@en .


###  http://w3id.org/emmo/domain/neo#R1bLylxOI5EPBIWCiqLVQv
:R1bLylxOI5EPBIWCiqLVQv rdf:type owl:Class ;
                        rdfs:subClassOf :R9p0u8Gh9Tup5P416Wl32S7 ,
                                        [ rdf:type owl:Restriction ;
                                          owl:onProperty elite:isSubProcessOf ;
                                          owl:someValuesFrom :RBU28e2pgiTqsaTCPWnAJ6y
                                        ] ;
                        rdfs:comment """electron scattering in which energy and/or momentum are not conserved in the collision system
Note 1 to entry: For inelastic scattering, the electron trajectory is modified by plasmon loss, core loss, and other multiple scatterings"""@en ;
                        rdfs:isDefinedBy "Stacey, W. (2018). Nuclear Reactor Physics (3rd ed.). Wiley. Retrieved from https://www.perlego.com/book/993700/nuclear-reactor-physics-pdf (Original work published 2018)" ;
                        rdfs:seeAlso <https://www.iso.org/obp/ui/en/#iso:std:iso:15932:ed-1:v1:en:term:2.2.2> ;
                        <http://www.w3.org/2004/02/skos/core#definition> """When the compound nucleus formed by neutron capture decays by the emission of
one neutron, leaving the nucleus in an excited state which subsequently undergoes
further decays, the event is referred to as inelastic scattering."""@en ;
                        <http://www.w3.org/2004/02/skos/core#prefLabel> "NuclearInelasticScattering"@en .


###  http://w3id.org/emmo/domain/neo#R1pzLL39gf2pPU0vtkTmnm
:R1pzLL39gf2pPU0vtkTmnm rdf:type owl:Class ;
                        rdfs:subClassOf :RC9Vnqc96TS4VVdygnxu8UP ,
                                        [ rdf:type owl:Restriction ;
                                          owl:onProperty elite:affects ;
                                          owl:someValuesFrom :R7VGQozOvQbYzOvcFQCwv8P
                                        ] ;
                        rdfs:isDefinedBy <https://www.nrc.gov/docs/ML1125/ML11258A366.pdf> ;
                        <http://www.w3.org/2004/02/skos/core#definition> "Rapidly lower reactor pressure to allow low pressure injection sources to maintain reactor water level above the Top of Active Fuel."@en ;
                        <http://www.w3.org/2004/02/skos/core#prefLabel> "AutomaticReactorDepressurization"@en .


###  http://w3id.org/emmo/domain/neo#R2eIY10Bw0mNaYfKDcCmDd
:R2eIY10Bw0mNaYfKDcCmDd rdf:type owl:Class ;
                        rdfs:subClassOf :RDoeQzvUClmOY7fNhDvK0L1 ,
                                        [ rdf:type owl:Restriction ;
                                          owl:onProperty :RB4rNlczhggIx7lqdEK2d9c ;
                                          owl:someValuesFrom :R0ZnwwPdidaBfZOg6tgZJr
                                        ] ;
                        rdfs:isDefinedBy <https://www.nrc.gov/docs/ML1209/ML120970422.pdf> ;
                        <http://www.w3.org/2004/02/skos/core#altLabel> "MUWC"@en ,
                                                                       "ReactorMakeUpWaterCondensateSystem"@en ,
                                                                       "ReactorWaterCleanupSystem"@en ;
                        <http://www.w3.org/2004/02/skos/core#definition> "The purpose of the reactor water cleanup system (RWCU) is to maintain a high reactor water quality by removing fission products, corrosion products, and other soluble and insoluble impurities. The reactor water cleanup pump takes water from the recirculation system and the vessel bottom head and pumps the water through heat exchangers to cool the flow. The water is then sent through filter/demineralizers for cleanup. After cleanup, the water is returned to the reactor vessel via the feedwater piping."@en ;
                        <http://www.w3.org/2004/02/skos/core#prefLabel> "MakeUpWaterCondensateSystem"@en .


###  http://w3id.org/emmo/domain/neo#R2sZehPfJJ1VHSqzgnHkJX
:R2sZehPfJJ1VHSqzgnHkJX rdf:type owl:Class ;
                        rdfs:subClassOf :R83A2MMCcbIwrdyWy2Q6clL ;
                        rdfs:comment """Se mettiamo un processo tipo separazione o scollegamento possiamo poi creare una relazione \"from\" turbine.
Tipo protective  separation
electrically protective  separation
separation of one electric circuit from another by means of:
— double insulation  (3.4.8); or
— basic insulation  (3.4.6) and electrically protective screening (shielding); or
— reinforced insulation  (3.4.9)
[SOURCE: IEC 61140:2016, 3.24]
ISO 18246:2023(en), 3.4.12"""@en ;
                        <http://www.w3.org/2004/02/skos/core#altLabel> "MainLineSeparation" ;
                        <http://www.w3.org/2004/02/skos/core#prefLabel> "ProtectiveSeparation"@en .


###  http://w3id.org/emmo/domain/neo#R6dO6yatvM1kcW0Iuf8Z0R
:R6dO6yatvM1kcW0Iuf8Z0R rdf:type owl:Class ;
                        rdfs:subClassOf :R7Ss5qBF98KBgXN3rhg0rEl ;
                        rdfs:isDefinedBy "ISO 12749-5:2018(en) Nuclear energy, nuclear technologies, and radiological protection — Vocabulary — Part 5: Nuclear reactors" ;
                        <http://www.w3.org/2004/02/skos/core#altLabel> "RPS"@en ;
                        <http://www.w3.org/2004/02/skos/core#definition> """system that monitors the operation (3.9.1) of a reactor and which, on sensing an abnormal condition, automatically initiates actions to prevent an unsafe or potentially unsafe condition 

Note 1 to entry: This use of the term protection refers to protection of the plant; the system in this case encompasses all electrical and mechanical devices and circuitry, from sensors to actuation device input terminals. 

Note 2 to entry: The reactor protection system (RPS) provides protection against abnormal conditions such as reactor over-power, too fast neutron (3.1.5.1) flux increase, high reactor inlet temperature, primary heat transport system (3.7.2.5) over-pressure, etc. 

Note 3 to entry: The reactor protection system (RPS) imposes actions on several systems, especially, the reactor regulation system (3.7.2.1.2) (RRS), the reactor shutdown system (3.8.16.1) (SDS) and the emergency core cooling system (3.8.16.2) (ECCS). ﻿"""@en ;
                        <http://www.w3.org/2004/02/skos/core#prefLabel> "ReactorProtectionSystem"@en .


###  http://w3id.org/emmo/domain/neo#R70ALPF758Xyidhnwjti86x
:R70ALPF758Xyidhnwjti86x rdf:type owl:Class ;
                         rdfs:subClassOf :R7Z0T126p23eNAE1CkhAPXZ ,
                                         [ rdf:type owl:Restriction ;
                                           owl:onProperty [ owl:inverseOf elite:isInputOf
                                                          ] ;
                                           owl:someValuesFrom :RDS0g8UekSMDWjEgBp6z2sP
                                         ] ;
                         <http://www.w3.org/2004/02/skos/core#prefLabel> "FastInducedFission"@en .


###  http://w3id.org/emmo/domain/neo#R70ZOvZxdVYhbMrv2o1bK8I
:R70ZOvZxdVYhbMrv2o1bK8I rdf:type owl:Class ;
                         rdfs:subClassOf :RDoeQzvUClmOY7fNhDvK0L1 ,
                                         [ rdf:type owl:Restriction ;
                                           owl:onProperty :RB4rNlczhggIx7lqdEK2d9c ;
                                           owl:someValuesFrom :R85FFwLPHIursWfa6K6sKK9
                                         ] ;
                         <http://www.w3.org/2004/02/skos/core#prefLabel> "ReactorCavity"@en .


###  http://w3id.org/emmo/domain/neo#R71VApFUw4RxU2SFxCwNxMd
:R71VApFUw4RxU2SFxCwNxMd rdf:type owl:Class ;
                         rdfs:subClassOf :R9DvBOiqnlOM3kdfemfLOhd ,
                                         [ rdf:type owl:Restriction ;
                                           owl:onProperty elite:isConstitutiveProcessOf ;
                                           owl:someValuesFrom :RBp2yVTrXRyb55JnYdvAGux
                                         ] ;
                         rdfs:isDefinedBy <https://www.nrc.gov/reading-rm/basic-ref/students/for-educators/03.pdf> ;
                         <http://www.w3.org/2004/02/skos/core#definition> """Emergency cooling system Operation  (ECCS) provide core cooling under loss of coolant accident
conditions to limit fuel cladding damage. The emergency core cooling systems consist of two high
pressure and two low pressure systems."""@en ;
                         <http://www.w3.org/2004/02/skos/core#prefLabel> "ECCSOperation"@en .


###  http://w3id.org/emmo/domain/neo#R75fZKWD5XTzNF0Lht4vvWr
:R75fZKWD5XTzNF0Lht4vvWr rdf:type owl:Class ;
                         rdfs:subClassOf :RapiFOXlLXIKxdiWW4ljdc ;
                         rdfs:isDefinedBy <https://www.nrc.gov/reading-rm/basic-ref/glossary/loss-of-coolant-accident-loca.html> ;
                         <http://www.w3.org/2004/02/skos/core#altLabel> "LOCA"@en ,
                                                                        "LossOfReactorCoolingFunction"@en ;
                         <http://www.w3.org/2004/02/skos/core#definition> "Accident in which a breach in a reactor’s pressure boundary causes the coolant water to rush out of the reactor faster than makeup water can be added back in"@en ;
                         <http://www.w3.org/2004/02/skos/core#prefLabel> "LossOfCoolantAccident"@en .


###  http://w3id.org/emmo/domain/neo#R76QRzIQVjwDFrNAttIw9RF
:R76QRzIQVjwDFrNAttIw9RF rdf:type owl:Class ;
                         rdfs:subClassOf :R1DAH32q3UDTp3GZGqe5Re ,
                                         :R8MPIXNWSb8RCelrAeGNxMc ,
                                         [ rdf:type owl:Restriction ;
                                           owl:onProperty elite:isConstitutiveProcessOf ;
                                           owl:someValuesFrom :RB8nGLKVMobwZ43LOnPJsjS
                                         ] ;
                         :R8xx0dhbEh1tjGMDwNZfckV "The rapid insertion of a chemically soluble neutron poison (such as boric acid) into the reactor coolant system to ensure reactor shutdown."@en ;
                         rdfs:isDefinedBy <https://www.nrc.gov/reading-rm/basic-ref/glossary/safety-injection.html> ;
                         <http://www.w3.org/2004/02/skos/core#altLabel> "NuclearPoisonInjection"@en ;
                         <http://www.w3.org/2004/02/skos/core#prefLabel> "SafetyInjection"@en .


###  http://w3id.org/emmo/domain/neo#R78r8gHpSEIS6CD3QqneUoR
:R78r8gHpSEIS6CD3QqneUoR rdf:type owl:Class ;
                         rdfs:subClassOf :RBtkzbuLn6g0vdtDU3mijH0 ;
                         rdfs:seeAlso "INTERNATIONAL ATOMIC ENERGY AGENCY, Approaches for Overall Instrumentation and Control Architectures of Nuclear Power Plants, IAEA Nuclear Energy Series No. NP-T-2.11, IAEA, Vienna (2018)" ;
                         <http://www.w3.org/2004/02/skos/core#prefLabel> "PostulateMultipleFaiulureEvent"@en .


###  http://w3id.org/emmo/domain/neo#R78xqY4QQFGfjRzx8MpzQWe
:R78xqY4QQFGfjRzx8MpzQWe rdf:type owl:Class ;
                         rdfs:subClassOf :RDpEA8qdRk99FAT0xSGZgGS ;
                         rdfs:isDefinedBy <https://www.nrc.gov/docs/ML0707/ML070710376.pdf> ;
                         <http://www.w3.org/2004/02/skos/core#definition> """Conditions of normal operation that are expected to occur one or
more times during the life of the nuclear power unit and include but
are not limited to loss of power to all recirculation pumps, tripping of
the turbine generator set, isolation of the main condenser, and loss of
all offsite power.""" ;
                         <http://www.w3.org/2004/02/skos/core#prefLabel> "AnticipatedOperationalOccurrence"@en .


###  http://w3id.org/emmo/domain/neo#R79WXwPF5ZWjRPArxbbVAgU
:R79WXwPF5ZWjRPArxbbVAgU rdf:type owl:Class ;
                         rdfs:subClassOf elite:Process ;
                         rdfs:comment "controlled" ;
                         rdfs:seeAlso "EMMO" ;
                         <http://www.w3.org/2004/02/skos/core#prefLabel> "IntentionalProcess"@en .


###  http://w3id.org/emmo/domain/neo#R7ASmNcKrlRjzYHkUz3vfQT
:R7ASmNcKrlRjzYHkUz3vfQT rdf:type owl:Class ;
                         rdfs:subClassOf elite:Object ;
                         rdfs:isDefinedBy <https://www.iso.org/obp/ui/en/#iso:std:iso-iec:13273:-1:ed-1:v1:en:term:3.4.8> ;
                         <http://www.w3.org/2004/02/skos/core#definition> """organization that delivers energy efficiency services (3.4.5)
[SOURCE: CEN-CLC/TR 16103:2010, 4.6.4, modified – The term “entity” was changed to “organization” in the definition and the Note was deleted.]"""@en ;
                         <http://www.w3.org/2004/02/skos/core#prefLabel> "EnergyEfficiencyServiceCompany"@en .


###  http://w3id.org/emmo/domain/neo#R7Jf7CRh5B3US0yNBl08EK7
:R7Jf7CRh5B3US0yNBl08EK7 rdf:type owl:Class ;
                         rdfs:subClassOf elite:Object ,
                                         [ rdf:type owl:Restriction ;
                                           owl:onProperty :RB4rNlczhggIx7lqdEK2d9c ;
                                           owl:someValuesFrom :RRKk7nTYd2pj3LFUG4j9yj
                                         ] ;
                         rdfs:isDefinedBy <https://www.iso.org/obp/ui/en/#iso:std:iso:iwa:33:-1:ed-1:v1:en:term:7.5.9> ;
                         <http://www.w3.org/2004/02/skos/core#altLabel> "ControlRoom"@en ,
                                                                        "MCR"@en ,
                                                                        "MainReactorControlRoom"@en ;
                         <http://www.w3.org/2004/02/skos/core#definition> "structure required for accommodating the instruments, devices and computers for monitoring and controlling all types of mechanical and electrical equipment for the whole plant"@en ;
                         <http://www.w3.org/2004/02/skos/core#prefLabel> "MainControlRoom"@en .


###  http://w3id.org/emmo/domain/neo#R7KAfaev0soZNlAXHICHSJd
:R7KAfaev0soZNlAXHICHSJd rdf:type owl:Class ;
                         rdfs:subClassOf :RDoeQzvUClmOY7fNhDvK0L1 ,
                                         [ rdf:type owl:Restriction ;
                                           owl:onProperty :RB4rNlczhggIx7lqdEK2d9c ;
                                           owl:someValuesFrom :RCRVu2hmIevYnx0eZzyJEPs
                                         ] ;
                         rdfs:isDefinedBy "ISO 18077:2022(en) Reload startup physics tests for pressurized water reactors." ;
                         <http://www.w3.org/2004/02/skos/core#definition> """One or more rods that are inserted or withdrawn simultaneously 

Note 1 to entry: The term “all control rod groups” means all safety and regulating control rod groups. This term may also be shortened to simply “rod group.” 

Note 2 to entry: Some utilities use the term \"bank\" instead of \"group\". A control rod bank is the same as a control rod group."""@en ;
                         <http://www.w3.org/2004/02/skos/core#prefLabel> "ControlRodGroup"@en .


###  http://w3id.org/emmo/domain/neo#R7MjWOBoCnDd3BD1IBHjlRe
:R7MjWOBoCnDd3BD1IBHjlRe rdf:type owl:Class ;
                         rdfs:subClassOf elite:Object ,
                                         [ rdf:type owl:Restriction ;
                                           owl:onProperty elite:isParticipantOf ;
                                           owl:someValuesFrom :Rryk3Z5XNZ11ZiiLuT5M8Q
                                         ] ;
                         rdfs:isDefinedBy <https://www.iso.org/obp/ui/en/#iso:std:iso:tr:19083:-1:ed-1:v1:en:term:3.12> ;
                         <http://www.w3.org/2004/02/skos/core#definition> """group of people that has its own functions with responsibilities, authorities and relationships to the overall approach preventing and managing emergencies that might occur
Note 1 to entry: In general, emergency management utilizes a risk management approach to prevention, preparedness, response and recovery before, during and after potentially destabilizing or disruptive events.
[SOURCE: ISO 22320:2011, 3.35 modified]"""@en ;
                         <http://www.w3.org/2004/02/skos/core#prefLabel> "EmergencyManagementOrganization"@en .


###  http://w3id.org/emmo/domain/neo#R7NYEyrtAsNuF6n0QNOFmHm
:R7NYEyrtAsNuF6n0QNOFmHm rdf:type owl:Class ;
                         rdfs:subClassOf elite:Object ;
                         rdfs:isDefinedBy <https://www.iso.org/obp/ui/en/#iso:std:iso:3977:-1:ed-1:v1:en:term:2.16> ;
                         <http://www.w3.org/2004/02/skos/core#definition> "Term which when used alone refers to the turbine action only. It is that component of the gas turbine which produces power from expansion of the working fluid."@en ;
                         <http://www.w3.org/2004/02/skos/core#prefLabel> "Turbine"@en .


###  http://w3id.org/emmo/domain/neo#R7QpMP9Mf1mRrRVeMT7UcIX
:R7QpMP9Mf1mRrRVeMT7UcIX rdf:type owl:Class ;
                         rdfs:subClassOf :R9PjB5mvpVfreaI0pbTQFj6 ,
                                         :RtX7ESf673Z9eYoseycPyl ,
                                         [ rdf:type owl:Restriction ;
                                           owl:onProperty elite:isConstituentOf ;
                                           owl:someValuesFrom :RyMmVkVf9zClluOSgfr1Rh
                                         ] ,
                                         [ rdf:type owl:Restriction ;
                                           owl:onProperty elite:isOutputOf ;
                                           owl:someValuesFrom :R9p0u8Gh9Tup5P416Wl32S7
                                         ] ,
                                         [ rdf:type owl:Restriction ;
                                           owl:onProperty elite:isOutputOf ;
                                           owl:someValuesFrom :RDuDSbKh236WI6rqMad7Ar4
                                         ] ;
                         rdfs:comment "Fission products and actinides produced by neutron absorption of nuclear fuel itself are normally referred to by those specific names, and activation product reserved for products of neutron capture by other materials, such as structural components of the nuclear reactor or nuclear bomb, the reactor coolant, control rods or other neutron poisons, or materials in the environment. All of these, however, need to be handled as radioactive waste. Some nuclides originate in more than one way, as activation products or fission products."@en ;
                         rdfs:seeAlso <https://en.wikipedia.org/wiki/Activation_product> ;
                         <http://www.w3.org/2004/02/skos/core#prefLabel> "NPPActivationProduct"@en .


###  http://w3id.org/emmo/domain/neo#R7Ss5qBF98KBgXN3rhg0rEl
:R7Ss5qBF98KBgXN3rhg0rEl rdf:type owl:Class ;
                         rdfs:subClassOf elite:Object ,
                                         [ rdf:type owl:Restriction ;
                                           owl:onProperty elite:isConstituentOf ;
                                           owl:someValuesFrom :R0N27qMQzeRjM0vSOeAvUT
                                         ] ,
                                         [ rdf:type owl:Restriction ;
                                           owl:onProperty elite:participatesTo ;
                                           owl:someValuesFrom :R83A2MMCcbIwrdyWy2Q6clL
                                         ] ;
                         rdfs:isDefinedBy <https://www.iso.org/obp/ui/en/#iso:std:iso:4126:-9:ed-1:v1:en:term:3.2> ;
                         <http://www.w3.org/2004/02/skos/core#altLabel> "SafetyElements"@en ;
                         <http://www.w3.org/2004/02/skos/core#definition> """system including the safety devices and the interconnections between the equipment to be protected and any discharge connection to the nearest location of a safe disposal place
Note 1 to entry: This location can either be an atmospheric outlet or the connection into a safe collecting system or flare."""@en ;
                         <http://www.w3.org/2004/02/skos/core#prefLabel> "SafetySystem"@en .


###  http://w3id.org/emmo/domain/neo#R7VGQozOvQbYzOvcFQCwv8P
:R7VGQozOvQbYzOvcFQCwv8P rdf:type owl:Class ;
                         rdfs:subClassOf :RBp2yVTrXRyb55JnYdvAGux ,
                                         :RDoeQzvUClmOY7fNhDvK0L1 ,
                                         [ rdf:type owl:Restriction ;
                                           owl:onProperty :RB4rNlczhggIx7lqdEK2d9c ;
                                           owl:someValuesFrom :R0ZnwwPdidaBfZOg6tgZJr
                                         ] ;
                         rdfs:isDefinedBy <https://www.nrc.gov/docs/ML1209/ML120970422.pdf> ;
                         <http://www.w3.org/2004/02/skos/core#definition> """The low pressure emergency core cooling systems consist of two separate and independent systems, the core spray system and the low pressure coolant injection (LPCI) mode of the residual heat removal system. The core spray system consists of two separate and independent pumping loops, each capable of pumping water from the suppression pool into the reactor vessel. Core cooling is accomplished by spraying water on top of the fuel assemblies.
The low pressure coolant injection mode of the residual heat removal system provides makeup water to the reactor vessel for core cooling under loss of coolant accident conditions. The residual heat removal system is a multipurpose system with several operational modes, each utilizing the same major pieces of equipment. The low pressure coolant injection mode is the dominant mode and normal valve lineup configuration of the residual heat removal system. The low pressure coolant injection mode operates automatically to restore and, if necessary, maintain the reactor vessel coolant inventory to preclude fuel cladding temperatures in excess of 2200EF. During low pressure coolant injection operation, the residual heat removal pumps take water from the suppression pool and discharge to the reactor vessel."""@en ;
                         <http://www.w3.org/2004/02/skos/core#prefLabel> "LowPressureEmergencyCoreCoolingSystems"@en .


###  http://w3id.org/emmo/domain/neo#R7Z0T126p23eNAE1CkhAPXZ
:R7Z0T126p23eNAE1CkhAPXZ rdf:type owl:Class ;
                         rdfs:subClassOf :R9ZCvqvWWCWSwBxX7K82iwL ,
                                         [ rdf:type owl:Restriction ;
                                           owl:onProperty elite:isStageOf ;
                                           owl:someValuesFrom :R7tsY17A1s9DZ7gbZrjbVt6
                                         ] ;
                         rdfs:isDefinedBy <https://www.iso.org/obp/ui/en/#iso:std:iso:12749:-5:ed-1:v1:en:term:3.1.1.1> ;
                         <http://www.w3.org/2004/02/skos/core#definition> """nuclear fission (3.1.1) initiated by a nucleus when an external colliding particle is absorbed
Note 1 to entry: The absorption of the external colliding particle, usually a neutron, generates a strong increase in the compound nucleus internal energy and, hence, increases the compound nucleus instability, favouring a large energy release by means of a nucleus partition."""@en ;
                         <http://www.w3.org/2004/02/skos/core#prefLabel> "NeutronInducedFission"@en .


###  http://w3id.org/emmo/domain/neo#R7bsMx2CiGpSWjcw2VdBxqs
:R7bsMx2CiGpSWjcw2VdBxqs rdf:type owl:Class ;
                         rdfs:subClassOf :R7Ss5qBF98KBgXN3rhg0rEl ,
                                         :R7i2YiNCalwlsxcsL7AR3VF ,
                                         [ rdf:type owl:Restriction ;
                                           owl:onProperty :RB4rNlczhggIx7lqdEK2d9c ;
                                           owl:someValuesFrom :R0N27qMQzeRjM0vSOeAvUT
                                         ] ;
                         rdfs:comment """Meanwhile, an attempt to enter the Unit 1 RB to conduct radiation measurements at 03:45 on 12 March was abandoned, when the team encountered white fog-like steam upon opening the airlock
door, although the measurements at the radiation monitoring post near the site’s main gate did not show any anomaly to indicate a release from RPV or PCV at 04:00."""@en ;
                         rdfs:seeAlso """pag 29,The Fukushima Daiichi Accident Technical Volume 1/5 
link: https://www-pub.iaea.org/MTCD/Publications/PDF/AdditionalVolumes/P1710/Pub1710-TV1-Web.pdf""" ;
                         <http://www.w3.org/2004/02/skos/core#prefLabel> "MobileRadiationMonitor"@en .


###  http://w3id.org/emmo/domain/neo#R7e7zmzKt5Jl3O9HFQImLAV
:R7e7zmzKt5Jl3O9HFQImLAV rdf:type owl:Class ;
                         rdfs:subClassOf :RBnyfPxRohc9STM4mfSMMFq ;
                         rdfs:isDefinedBy """ISO 11999-1:2015(en) 
PPE for firefighters — Test methods and requirements for PPE used by firefighters who are at risk of exposure to high levels of heat and/or flame while fighting fires occurring in structures — Part 1: General """ ;
                         <http://www.w3.org/2004/02/skos/core#altLabel> "NPPFullFaceMask"@en ;
                         <http://www.w3.org/2004/02/skos/core#definition> "Facepiece which covers the eyes, nose, mouth, and chin and provides adequate sealing on the face of the wearer of a respiratory protective device against the ambient atmosphere "@en ;
                         <http://www.w3.org/2004/02/skos/core#prefLabel> "FullFaceMask"@en .


###  http://w3id.org/emmo/domain/neo#R7f91MxYlPSe16WDD1Wtw5E
:R7f91MxYlPSe16WDD1Wtw5E rdf:type owl:Class ;
                         rdfs:subClassOf :R80RaxHVqr4QPiv8ASxXxi3 ;
                         rdfs:comment "automatic function which ensures that a protective measure (3.36) is initiated if the ability of the SRP/CS to perform a function is diminished, or if the process conditions are changed such that hazards are generated"@en ;
                         rdfs:seeAlso <https://www.iso.org/obp/ui/en/#iso:std:iso:25119:-1:ed-2:v1:en:term:3.33> ;
                         <http://www.w3.org/2004/02/skos/core#altLabel> "AutomaticManipulation"@en ;
                         <http://www.w3.org/2004/02/skos/core#prefLabel> "AutomaticMonitoring"@en .


###  http://w3id.org/emmo/domain/neo#R7fkBdyMeKQvQzm3yRgM2iz
:R7fkBdyMeKQvQzm3yRgM2iz rdf:type owl:Class ;
                         rdfs:subClassOf :Rryk3Z5XNZ11ZiiLuT5M8Q ;
                         :R8xx0dhbEh1tjGMDwNZfckV "Plant procedures that direct operators' actions necessary to mitigate the consequences of transients and accidents that have caused plant parameters to exceed reactor protection system set points or engineered safety feature set points, or other established limits."@en ;
                         rdfs:isDefinedBy <https://www.nrc.gov/docs/ML1025/ML102560007.pdf> ;
                         <http://www.w3.org/2004/02/skos/core#altLabel> "EOP"@en ;
                         <http://www.w3.org/2004/02/skos/core#prefLabel> "EmergencyOperationProcedures"@en .


###  http://w3id.org/emmo/domain/neo#R7gZLWyPCimwGhHTueSRPhd
:R7gZLWyPCimwGhHTueSRPhd rdf:type owl:Class ;
                         rdfs:subClassOf :R7Ss5qBF98KBgXN3rhg0rEl ;
                         <http://www.w3.org/2004/02/skos/core#prefLabel> "ReactorPreventiveSystems"@en .


###  http://w3id.org/emmo/domain/neo#R7hYLnBucjQ8XgAj5RsQvpF
:R7hYLnBucjQ8XgAj5RsQvpF rdf:type owl:Class ;
                         rdfs:subClassOf elite:Object ,
                                         [ rdf:type owl:Restriction ;
                                           owl:onProperty elite:isConstituentOf ;
                                           owl:someValuesFrom :R0N27qMQzeRjM0vSOeAvUT
                                         ] ;
                         rdfs:isDefinedBy <https://www.iso.org/obp/ui/en/#iso:std:iso:81346:-10:ed-1:v1:en:term:3.9> ;
                         <http://www.w3.org/2004/02/skos/core#altLabel> "EPGS"@en ;
                         <http://www.w3.org/2004/02/skos/core#definition> "system representing a process for conversion, transmission and/or distribution of energy"@en ;
                         <http://www.w3.org/2004/02/skos/core#prefLabel> "PowerSupplySystem"@en .


###  http://w3id.org/emmo/domain/neo#R7i2YiNCalwlsxcsL7AR3VF
:R7i2YiNCalwlsxcsL7AR3VF rdf:type owl:Class ;
                         rdfs:subClassOf :R7Ss5qBF98KBgXN3rhg0rEl ;
                         rdfs:comment "This term refers all the devices used to measure parameters and properties  about system."@en ;
                         <http://www.w3.org/2004/02/skos/core#prefLabel> "SafetySensors"@en .


###  http://w3id.org/emmo/domain/neo#R7lNdF3mOkJN1rq1wQCfwG3
:R7lNdF3mOkJN1rq1wQCfwG3 rdf:type owl:Class ;
                         rdfs:subClassOf :R7QpMP9Mf1mRrRVeMT7UcIX ,
                                         :RPURhpVoxOOYoC2J28Rgfd ,
                                         [ rdf:type owl:Restriction ;
                                           owl:onProperty elite:isOutputOf ;
                                           owl:someValuesFrom :RBU28e2pgiTqsaTCPWnAJ6y
                                         ] ;
                         rdfs:isDefinedBy "IAEA Safety Glossary, Terminology Used in Nuclear Safety and Radiation Protection, 2018 Edition" ;
                         <http://www.w3.org/2004/02/skos/core#definition> "Nuclear fuel removed from a reactor following irradiation that is no longer usable in its present form because of depletion of fissile material, poison buildup or radiation damage."@en ;
                         <http://www.w3.org/2004/02/skos/core#prefLabel> "NuclearSpentFuel"@en .


###  http://w3id.org/emmo/domain/neo#R7oHlh8OgEkyG3XXGpiYlC5
:R7oHlh8OgEkyG3XXGpiYlC5 rdf:type owl:Class ;
                         rdfs:subClassOf :R7pKuzitkkIAgc5NxDlqfH4 ,
                                         :R7s6BZ18NYlgydAQozd7POd ,
                                         [ rdf:type owl:Restriction ;
                                           owl:onProperty elite:hasNext ;
                                           owl:someValuesFrom :R9TI5UbsBXnAYSIi17pJARr
                                         ] ;
                         rdfs:comment """An occurrence that results in a component’s loss of capability to
perform its intended safety functions.""" ;
                         rdfs:isDefinedBy <https://www-ns.iaea.org/downloads/standards/glossary/iaea-safety-glossary-draft-2016.pdf> ;
                         rdfs:seeAlso <https://www.nrc.gov/docs/ML0707/ML070710376.pdf> ;
                         <http://www.w3.org/2004/02/skos/core#altLabel> "Failure"@en ,
                                                                        "SingleFailure" ;
                         <http://www.w3.org/2004/02/skos/core#definition> "Loss of the ability of a structure, system or component to function within acceptance criteria. The structure, system or component is considered to fail when it becomes incapable of functioning, whether or not this is needed at that time. A failure may be the result of e.g. a hardware fault, a software fault, a system fault, an operator error or a maintenance error."@en ;
                         <http://www.w3.org/2004/02/skos/core#prefLabel> "ObjectFailure"@en .


###  http://w3id.org/emmo/domain/neo#R7pKuzitkkIAgc5NxDlqfH4
:R7pKuzitkkIAgc5NxDlqfH4 rdf:type owl:Class ;
                         rdfs:subClassOf :RDP6jdP3MdBK59hhoDGY0Vw ;
                         :RR3uD2d7YfhHohfv2Nm6sX "qualcosa che conduce ad una deviazione, a prescidere da chi lo ha fatto e perchè" ;
                         rdfs:comment "It is an event that can occur due to human error or the failure of artificial or industrial structures or phenomena."@en ;
                         <http://www.w3.org/2004/02/skos/core#altLabel> "UnexpectedEvent" ;
                         <http://www.w3.org/2004/02/skos/core#definition> "An unintended event is any casual occurrence, not controlled that can lead to hazardous condition to the surrounding environment where it takes place"@en ;
                         <http://www.w3.org/2004/02/skos/core#prefLabel> "UnintendedEvent"@en .


###  http://w3id.org/emmo/domain/neo#R7pvNIWMyFBzmeL9EcH58g8
:R7pvNIWMyFBzmeL9EcH58g8 rdf:type owl:Class ;
                         rdfs:subClassOf :REnnyld9FmnAjLpeDyUsnv ;
                         rdfs:isDefinedBy "ISO 12749-5:2018(en) Nuclear energy, nuclear technologies, and radiological protection — Vocabulary — Part 5: Nuclear reactors " ;
                         <http://www.w3.org/2004/02/skos/core#altLabel> "BWR"@en ;
                         <http://www.w3.org/2004/02/skos/core#definition> """nuclear reactor (3.1.22) with water as a coolant and as a moderator (3.1.23.1.2), boiling in the core 
Note 1 to entry: In a boiling water reactor the generated heat is removed from the core by evaporation. """@en ;
                         <http://www.w3.org/2004/02/skos/core#prefLabel> "BoilingWaterReactor"@en .


###  http://w3id.org/emmo/domain/neo#R7qSTtjQZPRR80bVjivshI8
:R7qSTtjQZPRR80bVjivshI8 rdf:type owl:Class ;
                         rdfs:subClassOf :R7gZLWyPCimwGhHTueSRPhd ,
                                         :RDoeQzvUClmOY7fNhDvK0L1 ,
                                         [ rdf:type owl:Restriction ;
                                           owl:onProperty :RB4rNlczhggIx7lqdEK2d9c ;
                                           owl:someValuesFrom :R0ZnwwPdidaBfZOg6tgZJr
                                         ] ;
                         rdfs:isDefinedBy "ISO 12749-5:2018(en) Nuclear energy, nuclear technologies, and radiological protection — Vocabulary — Part 5: Nuclear reactors " ;
                         <http://www.w3.org/2004/02/skos/core#altLabel> "SCS"@en ;
                         <http://www.w3.org/2004/02/skos/core#definition> "plant system (3.7.2) designed to cool the main parts of the reactor shield in order to maintain reasonable values of temperature in all the main shield parts, especially under normal on-power conditions "@en ;
                         <http://www.w3.org/2004/02/skos/core#prefLabel> "ReactorShieldCoolingSystem"@en .


###  http://w3id.org/emmo/domain/neo#R7qv2nUGxSNZRvXyF3CXPTr
:R7qv2nUGxSNZRvXyF3CXPTr rdf:type owl:Class ;
                         rdfs:subClassOf elite:Object ;
                         rdfs:isDefinedBy <https://www.iso.org/obp/ui/en/#iso:std:iso:10303:-2:ed-1:v1:en:term:3.1.21> ;
                         <http://www.w3.org/2004/02/skos/core#definition> "type of substance that cannot be divided or changed into different substances by ordinary chemical methods"@en ;
                         <http://www.w3.org/2004/02/skos/core#prefLabel> "ChemicalElement"@en .


###  http://w3id.org/emmo/domain/neo#R7s6BZ18NYlgydAQozd7POd
:R7s6BZ18NYlgydAQozd7POd rdf:type owl:Class ;
                         rdfs:subClassOf elite:Process ,
                                         [ rdf:type owl:Restriction ;
                                           owl:onProperty elite:isSubProcessOf ;
                                           owl:someValuesFrom :RCP7vIugzt8V7rXL11buOZH
                                         ] ;
                         rdfs:isDefinedBy <https://nvlpubs.nist.gov/nistpubs/SpecialPublications/NIST.SP.800-160v2r1.pdf> ;
                         <http://www.w3.org/2004/02/skos/core#altLabel> "ObjectDamage"@en ,
                                                                        "PhysicalObjectDamage"@en ;
                         <http://www.w3.org/2004/02/skos/core#definition> "Harm caused to something in such a way as to reduce or destroy its value, usefulness, or normal function."@en ;
                         <http://www.w3.org/2004/02/skos/core#prefLabel> "Damage"@en .


###  http://w3id.org/emmo/domain/neo#R7t1vs1VKDAzHkcQsFbt9JC
:R7t1vs1VKDAzHkcQsFbt9JC rdf:type owl:Class ;
                         rdfs:subClassOf :RC9Vnqc96TS4VVdygnxu8UP ;
                         rdfs:isDefinedBy <https://www.nrc.gov/docs/ML1125/ML11258A365.pdf> ;
                         <http://www.w3.org/2004/02/skos/core#definition> """Maintain adequate reactor vessel inventory – For core cooling – On small break LOCAs On small break LOCAs
 Depressurize the reactor vessel – To allow low pressure ECCSs to inject – On intermediate break LOCAs
 Backup RCIC when reactor vessel isolated"""@en ;
                         <http://www.w3.org/2004/02/skos/core#prefLabel> "HPCIOperation"@en .


###  http://w3id.org/emmo/domain/neo#R7tsY17A1s9DZ7gbZrjbVt6
:R7tsY17A1s9DZ7gbZrjbVt6 rdf:type owl:Class ;
                         rdfs:subClassOf elite:Whole ,
                                         :R9p0u8Gh9Tup5P416Wl32S7 ,
                                         [ rdf:type owl:Restriction ;
                                           owl:onProperty elite:isSubProcessOf ;
                                           owl:someValuesFrom :RBU28e2pgiTqsaTCPWnAJ6y
                                         ] ;
                         rdfs:isDefinedBy <https://www.iso.org/obp/ui/en/#iso:std:iso:1709:ed-3:v1:en:term:3.8> ;
                         <http://www.w3.org/2004/02/skos/core#definition> "series of nuclear reactions in which one of the agents necessary to the series is itself produced by the same reactions"@en ;
                         <http://www.w3.org/2004/02/skos/core#prefLabel> "NuclearChainReaction"@en .


###  http://w3id.org/emmo/domain/neo#R7twPwtQmmXFTKrDWM3POCD
:R7twPwtQmmXFTKrDWM3POCD rdf:type owl:Class ;
                         rdfs:subClassOf :RDoeQzvUClmOY7fNhDvK0L1 ;
                         rdfs:comment """In the Unit 1 design, there were two separate and redundant isolation condenser loops.
In these closed loops, the primary side of the isolation condenser received steam generated in the reactor and condensed it by cooling inside the heat exchanger tubes that were submerged in colder water tanks (isolation condenser pools) located outside the primary containment vessel. Condensed steam was then sent as cold water back to the reactor by gravity (see the diagram below). 
Without mixing with the radioactive primary side water, the secondary side water in the isolation condenser pools boiled, and the evaporated steam was vented to the atmosphere, which served as the heat sink. 
The secondary side water volume of the isolation condenser (both trains together) was sufficient for eight hours of cooling before requiring replenishment from a dedicated water source."""@en ;
                         rdfs:isDefinedBy "https://nrcoe.inl.gov/SysStudy/IC.aspx"@en ;
                         <http://www.w3.org/2004/02/skos/core#altLabel> "IC"@en ;
                         <http://www.w3.org/2004/02/skos/core#definition> "The IC is used in older boiling water reactor designs. The IC system transfers residual and decay heat from the reactor coolant to the water in the shell side of the heat exchanger resulting in steam generation. The steam generated in the shell side of the heat exchanger is then vented to the outside atmosphere. The system employs natural circulation as the driving head from the reactor steam side, through the isolation condenser tubes, and back to the reactor."@en ;
                         <http://www.w3.org/2004/02/skos/core#prefLabel> "IsolationCondenserSystem"@en .


###  http://w3id.org/emmo/domain/neo#R7uMg3wtcrU3GAUhIRZUQ8m
:R7uMg3wtcrU3GAUhIRZUQ8m rdf:type owl:Class ;
                         rdfs:subClassOf :RDoeQzvUClmOY7fNhDvK0L1 ,
                                         :Rw4mCgviqd6HTitZEzST6w ,
                                         [ rdf:type owl:Restriction ;
                                           owl:onProperty elite:isOutputOf ;
                                           owl:someValuesFrom :RB5vIXZFuMYcHWSzNAPjPtF
                                         ] ,
                                         [ rdf:type owl:Restriction ;
                                           owl:onProperty :RB4rNlczhggIx7lqdEK2d9c ;
                                           owl:someValuesFrom :R0ZnwwPdidaBfZOg6tgZJr
                                         ] ;
                         rdfs:isDefinedBy <https://www.nrc.gov/docs/ML1410/ML14107A411.pdf> ;
                         <http://www.w3.org/2004/02/skos/core#altLabel> "ReactorUltimateHeatSink"@en ,
                                                                        "UHS"@en ;
                         <http://www.w3.org/2004/02/skos/core#definition> "The UHS is the system of structures and components and associated assured water supply and atmospheric condition(s) credited for functioning as a heat sink to absorb reactor residual heat and essential station heat loads after a normal reactor shutdown or a shutdown following an accident or transient including a loss-of-coolant accident (LOCA). "@en ;
                         <http://www.w3.org/2004/02/skos/core#prefLabel> "UltimateHeatSink"@en .


###  http://w3id.org/emmo/domain/neo#R7unkqShg3WHoE9WWDhuPJE
:R7unkqShg3WHoE9WWDhuPJE rdf:type owl:Class ;
                         rdfs:subClassOf :R8KlSYQnSKI6PoJZNIdhwNI ,
                                         [ rdf:type owl:Restriction ;
                                           owl:onProperty elite:participatesTo ;
                                           owl:someValuesFrom :R76QRzIQVjwDFrNAttIw9RF
                                         ] ;
                         <http://www.w3.org/2004/02/skos/core#prefLabel> "BoratedWater"@en .


###  http://w3id.org/emmo/domain/neo#R80L6MpJJVkL4hoNB7thCRV
:R80L6MpJJVkL4hoNB7thCRV rdf:type owl:Class ;
                         rdfs:subClassOf :RDpEA8qdRk99FAT0xSGZgGS ;
                         rdfs:isDefinedBy <https://www.nrc.gov/reading-rm/basic-ref/glossary/startup.html> ;
                         <http://www.w3.org/2004/02/skos/core#definition> "An increase in the rate of fission (and heat production) in a reactor (usually by the removal of control rods from the core)."@en ;
                         <http://www.w3.org/2004/02/skos/core#prefLabel> "NPPStartUpPhase"@en .


###  http://w3id.org/emmo/domain/neo#R80RaxHVqr4QPiv8ASxXxi3
:R80RaxHVqr4QPiv8ASxXxi3 rdf:type owl:Class ;
                         rdfs:subClassOf :RDpEA8qdRk99FAT0xSGZgGS ;
                         rdfs:seeAlso <https://www.iso.org/obp/ui/en/#iso:std:iso-iec:11072:ed-1:v1:en:term:2.6.5> ;
                         <http://www.w3.org/2004/02/skos/core#altLabel> "Manipulation"@en ,
                                                                        "Monitoring"@en ;
                         <http://www.w3.org/2004/02/skos/core#comment> "A process which accesses and changes the contents of data elements."@en ;
                         <http://www.w3.org/2004/02/skos/core#prefLabel> "Controlling"@en .


###  http://w3id.org/emmo/domain/neo#R81QzLfYKssKKQ25a1Ibyv7
:R81QzLfYKssKKQ25a1Ibyv7 rdf:type owl:Class ;
                         rdfs:subClassOf :R7Z0T126p23eNAE1CkhAPXZ ,
                                         [ rdf:type owl:Restriction ;
                                           owl:onProperty [ owl:inverseOf elite:isInputOf
                                                          ] ;
                                           owl:someValuesFrom :R9s3bSmQntRAaUAzg5iKhyy
                                         ] ;
                         <http://www.w3.org/2004/02/skos/core#prefLabel> "ThermalInducedFission"@en .


###  http://w3id.org/emmo/domain/neo#R83A2MMCcbIwrdyWy2Q6clL
:R83A2MMCcbIwrdyWy2Q6clL rdf:type owl:Class ;
                         rdfs:subClassOf :RtdecAtZ9C9xUJNtjefY4D ;
                         rdfs:comment "No off-site radiological impact or only minor radiological impact"@en ,
                                      "have the objective of Control of accidents with core melt to limit off-site releases"@en ;
                         rdfs:isDefinedBy "INTERNATIONAL ATOMIC ENERGY AGENCY, Approaches for Overall Instrumentation and Control Architectures of Nuclear Power Plants, IAEA Nuclear Energy Series No. NP-T-2.11, IAEA, Vienna (2018) p.12" ;
                         <http://www.w3.org/2004/02/skos/core#altLabel> "Level3DiD"@en ,
                                                                        "NuclearReactorProtection"@en ;
                         <http://www.w3.org/2004/02/skos/core#definition> """Protection (i.e. reactor trip and actuation of engineered safety features) to control and/or limit the
consequences of accident conditions. This is based on demand and works very differently from control: real
demands occur rarely, so there is little opportunity to detect hidden failures or to experience conditions that
were insufficiently considered in the design. Therefore, the provision of a diverse means of protection is an
important feature at this level."""@en ;
                         <http://www.w3.org/2004/02/skos/core#prefLabel> "NPPProtection"@en .


###  http://w3id.org/emmo/domain/neo#R84TLuFmfSZMhgSh0uL0LXk
:R84TLuFmfSZMhgSh0uL0LXk rdf:type owl:Class ;
                         rdfs:subClassOf :RDpEA8qdRk99FAT0xSGZgGS ;
                         rdfs:isDefinedBy """ISO 44001:2017(en)
Collaborative business relationship management systems — Requirements and framework""" ;
                         <http://www.w3.org/2004/02/skos/core#definition> "process to determine a value"@en ;
                         <http://www.w3.org/2004/02/skos/core#prefLabel> "Measurement"@en .


###  http://w3id.org/emmo/domain/neo#R85FFwLPHIursWfa6K6sKK9
:R85FFwLPHIursWfa6K6sKK9 rdf:type owl:Class ;
                         rdfs:subClassOf :RDoeQzvUClmOY7fNhDvK0L1 ,
                                         [ rdf:type owl:Restriction ;
                                           owl:onProperty :RB4rNlczhggIx7lqdEK2d9c ;
                                           owl:someValuesFrom :RBW32C4x3sn1YahVG7uYVun
                                         ] ;
                         rdfs:isDefinedBy <https://www.tepco.co.jp/en/decommision/planaction/images/140127_01.pdf> ;
                         <http://www.w3.org/2004/02/skos/core#altLabel> "PCV"@en ;
                         <http://www.w3.org/2004/02/skos/core#definition> "Steel vessel containing the Reactor Pressure Vessel (RPV) and other main reactor facilities"@en ;
                         <http://www.w3.org/2004/02/skos/core#prefLabel> "PrimaryContainmentVessel"@en .


###  http://w3id.org/emmo/domain/neo#R86VrLeGdKN00eQd0A9HjPc
:R86VrLeGdKN00eQd0A9HjPc rdf:type owl:Class ;
                         rdfs:subClassOf :RDoeQzvUClmOY7fNhDvK0L1 ,
                                         [ rdf:type owl:Restriction ;
                                           owl:onProperty elite:isConstituentOf ;
                                           owl:someValuesFrom :R7twPwtQmmXFTKrDWM3POCD
                                         ] ;
                         rdfs:comment "In the Unit 1 design, there were two separate and redundant isolation condenser loops. In these closed loops, the primary side of the isolation condenser received steam generated in the reactor and condensed it by cooling inside the heat exchanger tubes that were submerged in colder water tanks (isolation condenser pools) located outside the primary containment vessel."@en ;
                         rdfs:seeAlso """Box 1.1–2. Systems for cooling the core when the reactor is isolated from the turbines. The Fukushima Daiichi Accident Technical Volume 1/5 
link: https://www-pub.iaea.org/MTCD/Publications/PDF/AdditionalVolumes/P1710/Pub1710-TV1-Web.pdf"""@en ;
                         <http://www.w3.org/2004/02/skos/core#altLabel> "IsolatioCondenserPool"@en ,
                                                                        "ReactorIsolationCondenserTank"@en ;
                         <http://www.w3.org/2004/02/skos/core#prefLabel> "IsolationCondenserTank"@en .


###  http://w3id.org/emmo/domain/neo#R89Yy2V18LstH4xGXyNb9XN
:R89Yy2V18LstH4xGXyNb9XN rdf:type owl:Class ;
                         rdfs:subClassOf elite:Object ,
                                         [ rdf:type owl:Restriction ;
                                           owl:onProperty elite:isConstituentOf ;
                                           owl:someValuesFrom :R0N27qMQzeRjM0vSOeAvUT
                                         ] ;
                         <http://www.w3.org/2004/02/skos/core#prefLabel> "TurbineBuildingContents"@en .


###  http://w3id.org/emmo/domain/neo#R8CzBJHXymJx05c6sDhbspt
:R8CzBJHXymJx05c6sDhbspt rdf:type owl:Class ;
                         rdfs:subClassOf :R8hTHDGsCdkEbILOuzUhlEr ;
                         rdfs:comment <https://en.wikipedia.org/wiki/Turbine_hall> ;
                         rdfs:isDefinedBy <https://www.iso.org/obp/ui#iso:std:iso:12749:-5:ed-1:v1:en> ;
                         <http://www.w3.org/2004/02/skos/core#altLabel> "NuclearTurbineBuilding"@en ,
                                                                        "TurbineIsland"@en ;
                         <http://www.w3.org/2004/02/skos/core#prefLabel> "TurbineBuilding"@en .


###  http://w3id.org/emmo/domain/neo#R8FmlobZiHsCZi4CHKxgtMg
:R8FmlobZiHsCZi4CHKxgtMg rdf:type owl:Class ;
                         rdfs:subClassOf :R83A2MMCcbIwrdyWy2Q6clL ,
                                         [ rdf:type owl:Restriction ;
                                           owl:onProperty elite:affects ;
                                           owl:someValuesFrom :R85FFwLPHIursWfa6K6sKK9
                                         ] ,
                                         [ rdf:type owl:Restriction ;
                                           owl:onProperty elite:isConstitutiveProcessOf ;
                                           owl:someValuesFrom :RCPFRkyBbFadwcQUuWavdPl
                                         ] ;
                         rdfs:isDefinedBy <https://www.nrc.gov/docs/ML1215/ML12159A162.pdf> ;
                         <http://www.w3.org/2004/02/skos/core#altLabel> "PCV"@en ;
                         <http://www.w3.org/2004/02/skos/core#definition> "The purpose of the primary containment ventilation is to allow for influent air to be brought into the drywell and suppression chamber and for effluent atmosphere to be discharged from the drywell and suppression chamber."@en ;
                         <http://www.w3.org/2004/02/skos/core#prefLabel> "PrimaryContainmentVentilation"@en .


###  http://w3id.org/emmo/domain/neo#R8HV58d46m6thaiYmxePBRu
:R8HV58d46m6thaiYmxePBRu rdf:type owl:Class ;
                         rdfs:subClassOf :R8KlSYQnSKI6PoJZNIdhwNI ;
                         <http://www.w3.org/2004/02/skos/core#prefLabel> "SeaWater"@en .


###  http://w3id.org/emmo/domain/neo#R8Jjvo3bjpE389mPpX0uOxQ
:R8Jjvo3bjpE389mPpX0uOxQ rdf:type owl:Class ;
                         rdfs:subClassOf :RC9Vnqc96TS4VVdygnxu8UP ;
                         rdfs:isDefinedBy <https://www-pub.iaea.org/MTCD/Publications/PDF/PUB1830_web.pdf> ;
                         <http://www.w3.org/2004/02/skos/core#definition> "Any measures that may be carried out to reduce the radiation exposure due to existing contamination of land areas through actions applied to the contamination itself (the source) or to the exposure pathways to humans."@en ;
                         <http://www.w3.org/2004/02/skos/core#prefLabel> "Remediation"@en .


###  http://w3id.org/emmo/domain/neo#R8KlSYQnSKI6PoJZNIdhwNI
:R8KlSYQnSKI6PoJZNIdhwNI rdf:type owl:Class ;
                         rdfs:subClassOf elite:Object ;
                         rdfs:isDefinedBy <https://www.iso.org/obp/ui/en/#iso:std:iso:14452:ed-1:v1:en:term:2.40> ;
                         <http://www.w3.org/2004/02/skos/core#definition> "water used for water supply"@en ;
                         <http://www.w3.org/2004/02/skos/core#prefLabel> "Water﻿"@en .


###  http://w3id.org/emmo/domain/neo#R8MGsTLlqoWXKEU5FfQd71X
:R8MGsTLlqoWXKEU5FfQd71X rdf:type owl:Class ;
                         rdfs:subClassOf :RDoeQzvUClmOY7fNhDvK0L1 ,
                                         [ rdf:type owl:Restriction ;
                                           owl:onProperty :RB4rNlczhggIx7lqdEK2d9c ;
                                           owl:someValuesFrom :R85FFwLPHIursWfa6K6sKK9
                                         ] ;
                         rdfs:seeAlso """Box 1.1–1. Boiling water reactors
The Fukushima Daiichi Accident Technical Volume 1/5 
link: https://www-pub.iaea.org/MTCD/Publications/PDF/AdditionalVolumes/P1710/Pub1710-TV1-Web.pdf"""@en ;
                         <http://www.w3.org/2004/02/skos/core#altLabel> "CoreRecirculationPumps"@en ;
                         <http://www.w3.org/2004/02/skos/core#prefLabel> "RecirculationPumps"@en .


###  http://w3id.org/emmo/domain/neo#R8MPIXNWSb8RCelrAeGNxMc
:R8MPIXNWSb8RCelrAeGNxMc rdf:type owl:Class ;
                         rdfs:subClassOf :RDpEA8qdRk99FAT0xSGZgGS ;
                         rdfs:isDefinedBy <https://dictionary.cambridge.org/it/dizionario/inglese/injection> ;
                         <http://www.w3.org/2004/02/skos/core#altLabel> "Injection"@en ;
                         <http://www.w3.org/2004/02/skos/core#definition> "The introduction of something new that is necessary or helpful to a situation or process."@en ;
                         <http://www.w3.org/2004/02/skos/core#prefLabel> "MaterialInjection"@en .


###  http://w3id.org/emmo/domain/neo#R8O2O7mng5QSpkSaLJGAPbi
:R8O2O7mng5QSpkSaLJGAPbi rdf:type owl:Class ;
                         rdfs:subClassOf :R80RaxHVqr4QPiv8ASxXxi3 ;
                         rdfs:isDefinedBy <https://www.iso.org/obp/ui/en/#iso:std:iso:1213:-1:ed-3:v1:en:term:11.1.7> ;
                         <http://www.w3.org/2004/02/skos/core#altLabel> "RemoteControl"@en ,
                                                                        "RemoteManipulation"@en ;
                         <http://www.w3.org/2004/02/skos/core#definition> "initiation of control operations for a process or machine at a point remote from the motive power"@en ;
                         <http://www.w3.org/2004/02/skos/core#prefLabel> "RemoteControlling"@en .


###  http://w3id.org/emmo/domain/neo#R8PAMnGRP5NOBTguHsOmRSl
:R8PAMnGRP5NOBTguHsOmRSl rdf:type owl:Class ;
                         rdfs:subClassOf :RtdecAtZ9C9xUJNtjefY4D ,
                                         [ rdf:type owl:Restriction ;
                                           owl:onProperty elite:isSubProcessOf ;
                                           owl:someValuesFrom :RdPoUW04SB1jvKPJcXoVCW
                                         ] ;
                         rdfs:isDefinedBy "INTERNATIONAL ATOMIC ENERGY AGENCY, Approaches for Overall Instrumentation and Control Architectures of Nuclear Power Plants, IAEA Nuclear Energy Series No. NP-T-2.11, IAEA, Vienna (2018) p.12" ;
                         <http://www.w3.org/2004/02/skos/core#altLabel> "Lelev4DiD"@en ;
                         <http://www.w3.org/2004/02/skos/core#definition> """Severe accident management (i.e. monitoring and mitigation) to confine radioactive material. For this, a
small set of highly robust instrument channels are needed. Additionally, the I&C system design needs to
facilitate the operator’s ability to use any relevant I&C functions available. Alternative means of actuating
systems — needed to inject coolant, depressurize the reactor and maintain containment integrity — must also
be considered. The possible need to support mobile means might also be considered."""@en ;
                         <http://www.w3.org/2004/02/skos/core#prefLabel> "SevereAccidentManagement"@en .


###  http://w3id.org/emmo/domain/neo#R8RC4XINR1dcZ29MVHcvtI2
:R8RC4XINR1dcZ29MVHcvtI2 rdf:type owl:Class ;
                         rdfs:subClassOf :R89Yy2V18LstH4xGXyNb9XN ,
                                         [ rdf:type owl:Restriction ;
                                           owl:onProperty :RB4rNlczhggIx7lqdEK2d9c ;
                                           owl:someValuesFrom :R8CzBJHXymJx05c6sDhbspt
                                         ] ;
                         <http://www.w3.org/2004/02/skos/core#altLabel> "NPPCirculatingWaterPump"@en ;
                         <http://www.w3.org/2004/02/skos/core#prefLabel> "CirculatingWaterPump"@en .


###  http://w3id.org/emmo/domain/neo#R8SUtkHvWQxLIC7oGi7FZGx
:R8SUtkHvWQxLIC7oGi7FZGx rdf:type owl:Class ;
                         rdfs:subClassOf :R6dO6yatvM1kcW0Iuf8Z0R ,
                                         :R7NYEyrtAsNuF6n0QNOFmHm ,
                                         :RDoeQzvUClmOY7fNhDvK0L1 ,
                                         [ rdf:type owl:Restriction ;
                                           owl:onProperty elite:isConstituentOf ;
                                           owl:someValuesFrom :R9j7jE0NWQS6xBqDD8iJRbf
                                         ] ;
                         rdfs:comment "It is inside th RCIC"@en ;
                         rdfs:isDefinedBy <https://www.nrc.gov/docs/ML1125/ML11258A311.pdf> ;
                         <http://www.w3.org/2004/02/skos/core#definition> "The RCIC turbine is designed to rapidly accelerate from standby to the full load condition within 30 seconds. The RCIC turbine is a horizontally mounted radial re-entry, non-condensing Terry turbine. The RCIC turbine is designed to operate with a steam supply pressure ranging from 150 to 1135 psig. The RCIC turbine exhausts to the suppression pool under water."@en ;
                         <http://www.w3.org/2004/02/skos/core#prefLabel> "RCICTurbine"@en .


###  http://w3id.org/emmo/domain/neo#R8XKJXm7vS0D4Y1OEvOkXde
:R8XKJXm7vS0D4Y1OEvOkXde rdf:type owl:Class ;
                         rdfs:subClassOf :RCP7vIugzt8V7rXL11buOZH ;
                         rdfs:isDefinedBy <https://www.iso.org/obp/ui/en/#iso:std:iso:26802:ed-1:v1:en:term:3.1.1> ;
                         <http://www.w3.org/2004/02/skos/core#altLabel> "DBA"@en ;
                         <http://www.w3.org/2004/02/skos/core#definition> "accident conditions against which a facility is designed according to established design criteria, and for which the damage to the fuel and the release of radioactive material are kept within authorized limits"@en ;
                         <http://www.w3.org/2004/02/skos/core#prefLabel> "DesignBasisAccident"@en .


###  http://w3id.org/emmo/domain/neo#R8bUZpp1yY81qmfgGNH0TyF
:R8bUZpp1yY81qmfgGNH0TyF rdf:type owl:Class ;
                         rdfs:subClassOf :RlYMwSSvmqekLRLzmf5IzV ,
                                         [ rdf:type owl:Restriction ;
                                           owl:onProperty elite:isBehaviourOf ;
                                           owl:someValuesFrom :RBsAUchYFBwAtcVUeFr8EFq
                                         ] ;
                         <http://www.w3.org/2004/02/skos/core#prefLabel> "Closing"@en .


###  http://w3id.org/emmo/domain/neo#R8baDZRwKkBRaeQKFoM4Z4N
:R8baDZRwKkBRaeQKFoM4Z4N rdf:type owl:Class ;
                         rdfs:subClassOf :R8lgbjRv5CeOJ43GygJ143n ;
                         rdfs:isDefinedBy <https://www.iso.org/obp/ui/en/#iso:std:iso:37100:ed-1:v1:en:term:3.1.14> ;
                         <http://www.w3.org/2004/02/skos/core#definition> "natural event such as a flood, earthquake, or hurricane that causes great damage or loss of life"@en ;
                         <http://www.w3.org/2004/02/skos/core#prefLabel> "NaturalDisaster"@en .


###  http://w3id.org/emmo/domain/neo#R8hTHDGsCdkEbILOuzUhlEr
:R8hTHDGsCdkEbILOuzUhlEr rdf:type owl:Class ;
                         rdfs:subClassOf elite:Object ,
                                         [ rdf:type owl:Restriction ;
                                           owl:onProperty elite:isConstituentOf ;
                                           owl:someValuesFrom :R0N27qMQzeRjM0vSOeAvUT
                                         ] ;
                         rdfs:isDefinedBy <https://www.iso.org/obp/ui/en/#iso:std:iso:ts:19883:ed-1:v1:en:term:3.15> ;
                         <http://www.w3.org/2004/02/skos/core#altLabel> "Building"@en ;
                         <http://www.w3.org/2004/02/skos/core#definition> "structure that has a roof and walls, with the similar function as a container (3.14) for a hydrogen PSA system or the components of a hydrogen PSA system"@en ;
                         <http://www.w3.org/2004/02/skos/core#prefLabel> "NuclearPowerPlantBuilding"@en .


###  http://w3id.org/emmo/domain/neo#R8lgbjRv5CeOJ43GygJ143n
:R8lgbjRv5CeOJ43GygJ143n rdf:type owl:Class ;
                         rdfs:subClassOf :RDP6jdP3MdBK59hhoDGY0Vw ;
                         rdfs:comment "It is not controlled and created by natural phenomena" ;
                         rdfs:isDefinedBy <https://www.fgdc.gov/HSWG/testing/ref_pages/Natural_Events_ref.htm> ;
                         <http://www.w3.org/2004/02/skos/core#definition> "Phenomenon found in or created by naturally occuring conditions."@en ;
                         <http://www.w3.org/2004/02/skos/core#prefLabel> "NaturalEvent"@en .


###  http://w3id.org/emmo/domain/neo#R8nenqdCSaU473TbSbvjjvz
:R8nenqdCSaU473TbSbvjjvz rdf:type owl:Class ;
                         rdfs:subClassOf :R9p0u8Gh9Tup5P416Wl32S7 ,
                                         [ rdf:type owl:Restriction ;
                                           owl:onProperty elite:isSubProcessOf ;
                                           owl:someValuesFrom :RBU28e2pgiTqsaTCPWnAJ6y
                                         ] ;
                         rdfs:comment """collision between a moving particle and a second particle in which the total kinetic energy (3.35) and the total momentum are conserved
Note 1 to entry: See inelastic scattering (4.2).
Note 2 to entry: In elastic scattering interactions, the moving particle can be deflected through angles of up to 180°."""@en ;
                         <http://www.w3.org/2004/02/skos/core#altLabel> "BinaryElasticScattering" ;
                         <http://www.w3.org/2004/02/skos/core#definition> "collision between a neutron and a nucleus in which the total kinetic energy (3.35) and the total momentum are conserved"@en ;
                         <http://www.w3.org/2004/02/skos/core#prefLabel> "NuclearElasticScattering"@en .


###  http://w3id.org/emmo/domain/neo#R8qKVAw3v5SZK2O6Y8cyDEr
:R8qKVAw3v5SZK2O6Y8cyDEr rdf:type owl:Class ;
                         rdfs:subClassOf :R7QpMP9Mf1mRrRVeMT7UcIX ;
                         rdfs:isDefinedBy "https://aris.iaea.org/sites/Glossary.html Glossary of Terms in ARIS Reports"@en ;
                         <http://www.w3.org/2004/02/skos/core#altLabel> "Moderator" ;
                         <http://www.w3.org/2004/02/skos/core#definition> "A material that is used to decrease the speed of the fast neutron produced during a fission even and thus sustaining a chain reaction."@en ;
                         <http://www.w3.org/2004/02/skos/core#prefLabel> "ReactorNuclearModerator"@en .


###  http://w3id.org/emmo/domain/neo#R8rcf1IQoRtZq8YkEpiByPn
:R8rcf1IQoRtZq8YkEpiByPn rdf:type owl:Class ;
                         rdfs:subClassOf :RDpEA8qdRk99FAT0xSGZgGS ,
                                         [ rdf:type owl:Restriction ;
                                           owl:onProperty elite:affects ;
                                           owl:someValuesFrom :R7MjWOBoCnDd3BD1IBHjlRe
                                         ] ;
                         rdfs:isDefinedBy <https://www.iso.org/obp/ui/en/#iso:std:iso:17419:ed-1:v1:en:term:3.29> ;
                         <http://www.w3.org/2004/02/skos/core#definition> "Process of the promulgation, monitoring, and enforcement of rules defined in 'regulation (document)', established by primary and/or delegated legislation"@en ;
                         <http://www.w3.org/2004/02/skos/core#prefLabel> "Regulation"@en .


###  http://w3id.org/emmo/domain/neo#R8sjiaUqifg1oq1iJBb45A6
:R8sjiaUqifg1oq1iJBb45A6 rdf:type owl:Class ;
                         rdfs:subClassOf :R9TI5UbsBXnAYSIi17pJARr ,
                                         [ rdf:type owl:Restriction ;
                                           owl:onProperty elite:hasNext ;
                                           owl:someValuesFrom :RZ7eQ19CTPh8iKBmvqWp16
                                         ] ,
                                         [ rdf:type owl:Restriction ;
                                           owl:onProperty elite:isStageOf ;
                                           owl:someValuesFrom :RCP7vIugzt8V7rXL11buOZH
                                         ] ;
                         <http://www.w3.org/2004/02/skos/core#definition> "It is the first event, in temporary order, of the sequence of the events in a nuclear accident" ;
                         <http://www.w3.org/2004/02/skos/core#prefLabel> "NuclearAccidentInitialEvent"@en .


###  http://w3id.org/emmo/domain/neo#R8uIjbM4VtJ8beM5k0lze7B
:R8uIjbM4VtJ8beM5k0lze7B rdf:type owl:Class ;
                         rdfs:subClassOf :R7oHlh8OgEkyG3XXGpiYlC5 ,
                                         :RRxSYO9r2FD1rHmRPugfob ;
                         rdfs:isDefinedBy <https://www.nrc.gov/docs/ML0707/ML070710376.pdf> ;
                         <http://www.w3.org/2004/02/skos/core#definition> """The result of an event which, because of dependencies, causes a
coincidence of failure states of components in two or more separate
channels of a redundancy system, leading to the failure of the defined
system to perform its intended function."""@en ;
                         <http://www.w3.org/2004/02/skos/core#prefLabel> "CommonModeFailureEvents"@en .


###  http://w3id.org/emmo/domain/neo#R8yJFxRXki6jB3lgKxV6thW
:R8yJFxRXki6jB3lgKxV6thW rdf:type owl:Class ;
                         rdfs:subClassOf :R84TLuFmfSZMhgSh0uL0LXk ,
                                         :RBv35jM3VSFKKxtWNVyDILw ;
                         :R8xx0dhbEh1tjGMDwNZfckV "Measurement of dose or contamination for the purpose of the assessment or control of exposure to radiation or radioactive material, and the interpretation of the results."@en ;
                         rdfs:isDefinedBy <https://www.iso.org/obp/ui/en/#iso:std:iso:20553:ed-1:v1:en:term:3.15> ;
                         <http://www.w3.org/2004/02/skos/core#altLabel> "ContaminationMonitoring"@en ;
                         <http://www.w3.org/2004/02/skos/core#prefLabel> "ContaminationMeasurement"@en .


###  http://w3id.org/emmo/domain/neo#R8ym94st1azekRHdt3ayDq5
:R8ym94st1azekRHdt3ayDq5 rdf:type owl:Class ;
                         rdfs:subClassOf :R7pKuzitkkIAgc5NxDlqfH4 ,
                                         [ rdf:type owl:Restriction ;
                                           owl:onProperty elite:affects ;
                                           owl:someValuesFrom :R85FFwLPHIursWfa6K6sKK9
                                         ] ,
                                         [ rdf:type owl:Restriction ;
                                           owl:onProperty elite:affects ;
                                           owl:someValuesFrom :R89Yy2V18LstH4xGXyNb9XN
                                         ] ,
                                         [ rdf:type owl:Restriction ;
                                           owl:onProperty elite:affects ;
                                           owl:someValuesFrom :RDZtzLsQmngV2BtJvmS5pbg
                                         ] ,
                                         [ rdf:type owl:Restriction ;
                                           owl:onProperty elite:affects ;
                                           owl:someValuesFrom :RDoeQzvUClmOY7fNhDvK0L1
                                         ] ;
                         rdfs:isDefinedBy """ISO 12749-1:2020(en)
Nuclear energy — Vocabulary — Part 1: General terminology""" ;
                         <http://www.w3.org/2004/02/skos/core#definition> "Radioactive substances on surfaces, or within solids, liquids, or gases (including the human body), where their presence is unintended or undesirable, or the process giving rise to their presence in such places."@en ;
                         <http://www.w3.org/2004/02/skos/core#prefLabel> "RadiologicalContamination"@en .


###  http://w3id.org/emmo/domain/neo#R8zYURIM0mP33CaMTE6iACV
:R8zYURIM0mP33CaMTE6iACV rdf:type owl:Class ;
                         rdfs:subClassOf :R7hYLnBucjQ8XgAj5RsQvpF ,
                                         [ rdf:type owl:Restriction ;
                                           owl:onProperty elite:isConstituentOf ;
                                           owl:someValuesFrom :RRVTDj2E9x5cjit7EQ9Dkx
                                         ] ;
                         rdfs:isDefinedBy "IWA 33-1:2019(en) Technical guidelines for the development of small hydropower plants — Part 1: Vocabulary "@en ;
                         <http://www.w3.org/2004/02/skos/core#definition> "DC power source equipment transforming electric energy into chemical energy for storage"@en ;
                         <http://www.w3.org/2004/02/skos/core#prefLabel> "StorageBattery"@en .


###  http://w3id.org/emmo/domain/neo#R91s5ihcKvYBOzeCaNlNVVK
:R91s5ihcKvYBOzeCaNlNVVK rdf:type owl:Class ;
                         rdfs:subClassOf elite:Object ;
                         rdfs:isDefinedBy <https://www.iso.org/obp/ui/en/#iso:std:iso:10303:-227:ed-2:v1:en:term:3.3.27> ;
                         <http://www.w3.org/2004/02/skos/core#definition> "a quantity of matter"@en ;
                         <http://www.w3.org/2004/02/skos/core#prefLabel> "Material"@en .


###  http://w3id.org/emmo/domain/neo#R94o7o1nZqxzHLLqTyhHY08
:R94o7o1nZqxzHLLqTyhHY08 rdf:type owl:Class ;
                         rdfs:subClassOf :RDpEA8qdRk99FAT0xSGZgGS ;
                         rdfs:comment "any periodic or unplanned support and verification operations designed to keep premises and equipment in proper working condition" ;
                         rdfs:seeAlso <https://www.iso.org/obp/ui/en/#iso:std:iso:22716:ed-1:v2:en:term:2.19> ;
                         <http://www.w3.org/2004/02/skos/core#definition> "any periodic or unplanned support and verification operations designed to keep premises and equipment in proper working condition in a nuclear reactor" ;
                         <http://www.w3.org/2004/02/skos/core#prefLabel> "NuclearReactorMaintanance"@en .


###  http://w3id.org/emmo/domain/neo#R95M6reIX3ya776PtOPLGmY
:R95M6reIX3ya776PtOPLGmY rdf:type owl:Class ;
                         rdfs:subClassOf :RCP7vIugzt8V7rXL11buOZH ;
                         rdfs:isDefinedBy <https://www.iso.org/obp/ui/en/#iso:std:iso:26802:ed-1:v1:en:term:3.1.2> ;
                         <http://www.w3.org/2004/02/skos/core#altLabel> "BDBA"@en ;
                         <http://www.w3.org/2004/02/skos/core#definition> "accident conditions more severe than a design basis accident"@en ;
                         <http://www.w3.org/2004/02/skos/core#prefLabel> "BeyondDesignBasisAccident"@en .


###  http://w3id.org/emmo/domain/neo#R98XsS8Lh28DOd8LW80vc2w
:R98XsS8Lh28DOd8LW80vc2w rdf:type owl:Class ;
                         rdfs:subClassOf elite:Whole ;
                         rdfs:isDefinedBy <https://www.nrc.gov/docs/ML0707/ML070710376.pdf> ;
                         <http://www.w3.org/2004/02/skos/core#definition> """Conditions of normal operation that are expected to occur one or
more times during the life of the nuclear power unit and include but
are not limited to loss of power to all recirculation pumps, tripping of
the turbine generator set, isolation of the main condenser, and loss of
all offsite power."""@en ;
                         <http://www.w3.org/2004/02/skos/core#prefLabel> "NuclearPlantAOO"@en .


###  http://w3id.org/emmo/domain/neo#R99rf4ECHdvdIhjRSeggwHm
:R99rf4ECHdvdIhjRSeggwHm rdf:type owl:Class ;
                         rdfs:subClassOf :RLEjSGGgoWOVMGjQsskCsb ,
                                         [ rdf:type owl:Restriction ;
                                           owl:onProperty elite:isBehaviourOf ;
                                           owl:someValuesFrom :RDZtzLsQmngV2BtJvmS5pbg
                                         ] ;
                         <http://www.w3.org/2004/02/skos/core#prefLabel> "NPPOperatorError"@en .


###  http://w3id.org/emmo/domain/neo#R9BGIwbHOtd3ACG5ZuCdHJP
:R9BGIwbHOtd3ACG5ZuCdHJP rdf:type owl:Class ;
                         rdfs:subClassOf :R7qv2nUGxSNZRvXyF3CXPTr ,
                                         [ rdf:type owl:Restriction ;
                                           owl:onProperty elite:isParticipantOf ;
                                           owl:someValuesFrom :RgAy137nXA9FNxJLdXeh2G
                                         ] ;
                         rdfs:comment """Radionuclides that occur naturally on Earth in significant quantities.
 The term is usually used to refer to the primordial radionuclides 40K, 235U, 238U,
232Th and their radioactive decay products.
 Contrasted with radionuclides of artificial origin, anthropogenic radionuclides and human made radionuclides (which all mean the same), and also with artificialì radionuclides (which exclude radionuclides of artificial origin that are also naturally occurring). Radionuclides of artificial origin may include radionuclides that are also naturally occurring but may not include radionuclides of natural origin"""@en ;
                         rdfs:isDefinedBy <https://www.nrc.gov/reading-rm/basic-ref/glossary/radionuclide.html)> ;
                         rdfs:seeAlso """IAEA Safety Glossary, Terminology Used in Nuclear Safety 
and Radiation Protection, 2018 Edition """ ;
                         <http://www.w3.org/2004/02/skos/core#definition> "An unstable isotope of an element that decays or disintegrates spontaneously, thereby emitting radiation. Approximately 5,000 natural and artificial radioisotopes have been identified."@en ;
                         <http://www.w3.org/2004/02/skos/core#prefLabel> "Radionuclide"@en .


###  http://w3id.org/emmo/domain/neo#R9DvBOiqnlOM3kdfemfLOhd
:R9DvBOiqnlOM3kdfemfLOhd rdf:type owl:Class ;
                         rdfs:subClassOf :R8PAMnGRP5NOBTguHsOmRSl ;
                         rdfs:isDefinedBy <https://www.iso.org/obp/ui/en/#iso:std:iso:ts:16901:ed-2:v1:en:term:3.20> ;
                         <http://www.w3.org/2004/02/skos/core#definition> "limitation of any negative consequence (3.6) of a particular event"@en ;
                         <http://www.w3.org/2004/02/skos/core#prefLabel> "Mitigation"@en .


###  http://w3id.org/emmo/domain/neo#R9Hn7TrsF0nNCCTri5RWDXP
:R9Hn7TrsF0nNCCTri5RWDXP rdf:type owl:Class ;
                         rdfs:subClassOf :RlYMwSSvmqekLRLzmf5IzV ;
                         rdfs:isDefinedBy """ISO 14313:2007(en)
Petroleum and natural gas industries — Pipeline transportation systems — Pipeline valves""" ;
                         <http://www.w3.org/2004/02/skos/core#definition> "To unobstruct an opening"@en ;
                         <http://www.w3.org/2004/02/skos/core#prefLabel> "Open"@en .


###  http://w3id.org/emmo/domain/neo#R9Iwkpvro1luxgrYOcKzuPX
:R9Iwkpvro1luxgrYOcKzuPX rdf:type owl:Class ;
                         rdfs:subClassOf :Rw4mCgviqd6HTitZEzST6w ;
                         rdfs:comment <https://www.nra.go.jp/data/000292313.pdf> ,
                                      """At around 21:55 on 14 March, the recently restored containment atmospheric monitoring system
(CAMS) — the radiation monitoring equipment inside the Unit 2 RPV — indicated that the radiation
levels inside the containment had increased substantially ..."""@en ;
                         rdfs:seeAlso """Pag 28, The Fukushima Daiichi Accident Technical Volume 1/5 
link: https://www-pub.iaea.org/MTCD/Publications/PDF/AdditionalVolumes/P1710/Pub1710-TV1-Web.pdf."""@en ;
                         <http://www.w3.org/2004/02/skos/core#altLabel> "CAMS"@en ,
                                                                        "NPP ContainmentAtmosphericMonitoringSystem"@en ;
                         <http://www.w3.org/2004/02/skos/core#prefLabel> "ContainmentAtmosphericMonitoringSystem"@en .


###  http://w3id.org/emmo/domain/neo#R9LQGc8WSd4vzQtq1aNhNEq
:R9LQGc8WSd4vzQtq1aNhNEq rdf:type owl:Class ;
                         rdfs:subClassOf :R7oHlh8OgEkyG3XXGpiYlC5 ;
                         rdfs:seeAlso <https://www-ns.iaea.org/downloads/standards/glossary/iaea-safety-glossary-draft-2016.pdf> ;
                         <http://www.w3.org/2004/02/skos/core#definition> "Loss of the ability of a structure to function within acceptance criteria. The structure is considered to fail when it becomes incapable of functioning, whether or not this is needed at that time."@en ;
                         <http://www.w3.org/2004/02/skos/core#prefLabel> "StructureFailure"@en .


###  http://w3id.org/emmo/domain/neo#R9MK7U9YLf7RtEpfQTDDr1q
:R9MK7U9YLf7RtEpfQTDDr1q rdf:type owl:Class ;
                         rdfs:subClassOf :R6dO6yatvM1kcW0Iuf8Z0R ,
                                         :RBsAUchYFBwAtcVUeFr8EFq ,
                                         :RDoeQzvUClmOY7fNhDvK0L1 ,
                                         [ rdf:type owl:Restriction ;
                                           owl:onProperty :RB4rNlczhggIx7lqdEK2d9c ;
                                           owl:someValuesFrom :R0ZnwwPdidaBfZOg6tgZJr
                                         ] ,
                                         [ rdf:type owl:Restriction ;
                                           owl:onProperty :RB4rNlczhggIx7lqdEK2d9c ;
                                           owl:someValuesFrom :RZtNAG3BL7lDm8L77EbEBd
                                         ] ;
                         rdfs:comment "here are detailed descriptions for both BWR and PWR in this document.﻿"@en ;
                         rdfs:isDefinedBy <https://inis.iaea.org/collection/NCLCollectionStore/_Public/27/051/27051618.pdf> ;
                         <http://www.w3.org/2004/02/skos/core#altLabel> "MSIV"@en ,
                                                                        "ReactorMainSteamIsolationValve"@en ;
                         <http://www.w3.org/2004/02/skos/core#definition> """The MSIVs are engineered safety features designed to limit the release of radioactive materials to the environment and to minimize reactor vessel inventory loss during a Design Basis Accident Redundant valves are located on each main steam line: one inside the drywell and one in the steam tunnel in the auxiliary building. The MSIVs are air- and spring-operated valves — air to open, air and spring to close .... (BWR)

The MSIVs are engineered safety features designed to limit the consequences of a steam line break. In the event of a steam line break inside containment, the MSIVs must close within 5 seconds to isolate the reverse steam flow from the intact SG to limit containment pressure below its design limits. The reverse steam flow is the result of the intact SG's feeding the steam line break through the pressure-equalizing header located in the turbine building. The containment is designed to accommodate only one SG blowdown... (PWR)"""@en ;
                         <http://www.w3.org/2004/02/skos/core#prefLabel> "MainSteamIsolationValve"@en .


###  http://w3id.org/emmo/domain/neo#R9OmYzkYNkqi6kwcE7kNZkF
:R9OmYzkYNkqi6kwcE7kNZkF rdf:type owl:Class ;
                         rdfs:subClassOf :R7oHlh8OgEkyG3XXGpiYlC5 ,
                                         :RRxSYO9r2FD1rHmRPugfob ;
                         rdfs:isDefinedBy <https://www.nrc.gov/docs/ML0707/ML070710376.pdf> ;
                         <http://www.w3.org/2004/02/skos/core#definition> """An occurrence that results in a component’s loss of capability to
perform its intended safety functions."""@en ;
                         <http://www.w3.org/2004/02/skos/core#prefLabel> "SingleFailureEvent"@en .


###  http://w3id.org/emmo/domain/neo#R9PjB5mvpVfreaI0pbTQFj6
:R9PjB5mvpVfreaI0pbTQFj6 rdf:type owl:Class ;
                         rdfs:subClassOf :R91s5ihcKvYBOzeCaNlNVVK ;
                         rdfs:comment "Material designated in national law or by a regulatory body as being  subject to regulatory control because of its radioactivity."@en ,
                                      """This is the ‘regulatory’ meaning of radioactive (2), and should not be confused with
the ‘scientific’ meaning of radioactive (1): ‘exhibiting radioactivity; emitting or
relating to the emission of ionizing radiation or particles’."""@en ,
                                      """Any material containing radionuclides where both the activity
concentration and the total activity in the consignment exceed the values specified
in [section IV of the Transport Regulations [2]]. (See SSR-6 (Rev. 1) [2].)""" ;
                         rdfs:isDefinedBy <https://www.undrr.org/understanding-disaster-risk/terminology/hips/tl0002> ;
                         rdfs:seeAlso """IAEA Safety Glossary, Terminology Used in Nuclear Safety 
and Radiation Protection, 2018 Edition """ ;
                         <http://www.w3.org/2004/02/skos/core#altLabel> "NuclearMaterial" ,
                                                                        "NuclearReactorMaterial" ;
                         <http://www.w3.org/2004/02/skos/core#definition> "A radioactive material is a substance or a material emitting, or related to the emission of, ionising radiation (either in the form of electromagnetic waves or particle radiation) (IAEA, 2018)."@en ;
                         <http://www.w3.org/2004/02/skos/core#prefLabel> "RadioactiveMaterials"@en .


###  http://w3id.org/emmo/domain/neo#R9Q7QurACY7OmMRPPPbDU7J
:R9Q7QurACY7OmMRPPPbDU7J rdf:type owl:Class ;
                         rdfs:subClassOf :RC5Uc3vBrAsYC8gCNkTsLH ;
                         <http://www.w3.org/2004/02/skos/core#prefLabel> "ContinuosInjection"@en .


###  http://w3id.org/emmo/domain/neo#R9TI5UbsBXnAYSIi17pJARr
:R9TI5UbsBXnAYSIi17pJARr rdf:type owl:Class ;
                         rdfs:subClassOf elite:Role ;
                         rdfs:seeAlso <http://www-ns.iaea.org/downloads/ni/training/specific_expert_knowledge/psa-level1/III1_1_A%20%20Initiating%20Event%20Analysis.pdf> ;
                         <http://www.w3.org/2004/02/skos/core#altLabel> "NuclearPlantAccidentEvents"@en ;
                         <http://www.w3.org/2004/02/skos/core#definition> "An event that creates disturbance in a Nuclear Reactor Plant Management and that leads to hazardous condition to the surrounding environment where it takes place"@en ;
                         <http://www.w3.org/2004/02/skos/core#prefLabel> "HazardousNuclearEvent"@en .


###  http://w3id.org/emmo/domain/neo#R9ZCvqvWWCWSwBxX7K82iwL
:R9ZCvqvWWCWSwBxX7K82iwL rdf:type owl:Class ;
                         rdfs:subClassOf elite:Role ,
                                         :R9p0u8Gh9Tup5P416Wl32S7 ,
                                         [ rdf:type owl:Restriction ;
                                           owl:onProperty elite:isSubProcessOf ;
                                           owl:someValuesFrom :RBU28e2pgiTqsaTCPWnAJ6y
                                         ] ,
                                         [ rdf:type owl:Restriction ;
                                           owl:onProperty [ owl:inverseOf elite:isOutputOf
                                                          ] ;
                                           owl:someValuesFrom :RDGsX7GTlCOL8Jlk3fXBK7U
                                         ] ;
                         rdfs:isDefinedBy <https://www.iso.org/obp/ui/en/#iso:std:iso:12749:-1:ed-1:v1:en:term:3.2.2> ;
                         <http://www.w3.org/2004/02/skos/core#definition> """splitting of a nucleus into fission fragments, either spontaneously or as a result of the impact of a particle, usually with an associated release of energy
Note 1 to entry: The nucleus usually has a high mass number, together with an intermediate or low average-binding-energy-per-nucleon; hence, an inherent instability exists, and the fission fragments are usually highly unstable.
[SOURCE: ISO 12749‑5:2018, 3.1.1]"""@en ;
                         <http://www.w3.org/2004/02/skos/core#prefLabel> "NuclearFission"@en .


###  http://w3id.org/emmo/domain/neo#R9aF6fIPWPEzkHdmnDKNorP
:R9aF6fIPWPEzkHdmnDKNorP rdf:type owl:Class ;
                         rdfs:subClassOf :R83A2MMCcbIwrdyWy2Q6clL ;
                         rdfs:isDefinedBy <https://www.nrc.gov/reading-rm/basic-ref/glossary/scram.html> ;
                         <http://www.w3.org/2004/02/skos/core#altLabel> "ReactorTrip"@en ;
                         <http://www.w3.org/2004/02/skos/core#definition> "The sudden shutting down of a nuclear reactor, usually by rapid insertion of control rods, either automatically or manually by the reactor operator. Also known as a \"reactor trip\""@en ;
                         <http://www.w3.org/2004/02/skos/core#prefLabel> "SCRAM"@en .


###  http://w3id.org/emmo/domain/neo#R9fLBLIc534UvSEEJ2pDkuM
:R9fLBLIc534UvSEEJ2pDkuM rdf:type owl:Class ;
                         rdfs:subClassOf :R7gZLWyPCimwGhHTueSRPhd ;
                         rdfs:isDefinedBy <https://www.iso.org/obp/ui/en/#iso:std:iso:13628:-7:ed-1:v1:en:term:3.1.7> ;
                         <http://www.w3.org/2004/02/skos/core#altLabel> "Barrier"@en ;
                         <http://www.w3.org/2004/02/skos/core#definition> "One or several barrier elements that are designed to prevent unintended flow of formation fluid﻿."@en ;
                         <http://www.w3.org/2004/02/skos/core#prefLabel> "NPPBarrier"@en .


###  http://w3id.org/emmo/domain/neo#R9j7jE0NWQS6xBqDD8iJRbf
:R9j7jE0NWQS6xBqDD8iJRbf rdf:type owl:Class ;
                         rdfs:subClassOf :R6dO6yatvM1kcW0Iuf8Z0R ,
                                         :RDoeQzvUClmOY7fNhDvK0L1 ,
                                         [ rdf:type owl:Restriction ;
                                           owl:onProperty :RB4rNlczhggIx7lqdEK2d9c ;
                                           owl:someValuesFrom :R0ZnwwPdidaBfZOg6tgZJr
                                         ] ;
                         rdfs:isDefinedBy <https://www.nrc.gov/docs/ML1209/ML120970422.pdf> ;
                         <http://www.w3.org/2004/02/skos/core#altLabel> "RCIC"@en ;
                         <http://www.w3.org/2004/02/skos/core#definition> "The reactor core isolation cooling (RCIC) system provides makeup water to the reactor vessel for core cooling when the main steam lines are isolated and the normal supply of water to the reactor vessel is lost. The RCIC system consists of a turbine-driven pump, piping, and valves necessary to deliver water to the reactor vessel at operating conditions. "@en ;
                         <http://www.w3.org/2004/02/skos/core#prefLabel> "ReactorCoreIsolationCoolingSystem"@en .


###  http://w3id.org/emmo/domain/neo#R9p0u8Gh9Tup5P416Wl32S7
:R9p0u8Gh9Tup5P416Wl32S7 rdf:type owl:Class ;
                         rdfs:subClassOf elite:Process ;
                         rdfs:isDefinedBy <https://en.wikipedia.org/wiki/Nuclear_reaction> ;
                         <http://www.w3.org/2004/02/skos/core#definition> "In nuclear physics and nuclear chemistry, a nuclear reaction is a process in which two nuclei, or a nucleus and an external subatomic particle, collide to produce one or more new nuclides. Thus, a nuclear reaction must cause a transformation of at least one nuclide to another."@en ;
                         <http://www.w3.org/2004/02/skos/core#prefLabel> "NuclearReaction"@en .


###  http://w3id.org/emmo/domain/neo#R9s3bSmQntRAaUAzg5iKhyy
:R9s3bSmQntRAaUAzg5iKhyy rdf:type owl:Class ;
                         rdfs:subClassOf elite:Role ,
                                         :RBfqFRty5Hp4V4caVtEvWdD ,
                                         [ rdf:type owl:Restriction ;
                                           owl:onProperty elite:isInputOf ;
                                           owl:someValuesFrom :R81QzLfYKssKKQ25a1Ibyv7
                                         ] ,
                                         [ rdf:type owl:Restriction ;
                                           owl:onProperty elite:isOutputOf ;
                                           owl:someValuesFrom :R7tsY17A1s9DZ7gbZrjbVt6
                                         ] ;
                         rdfs:isDefinedBy "ISO 12749-5:2018(en) Nuclear energy, nuclear technologies, and radiological protection — Vocabulary — Part 5: Nuclear reactors" ;
                         <http://www.w3.org/2004/02/skos/core#altLabel> "Neutron that has, by collision with other particles, reached an energy state equal to that of its surroundings."@en ;
                         <http://www.w3.org/2004/02/skos/core#prefLabel> "ThermalNeutron"@en .


###  http://w3id.org/emmo/domain/neo#R9zZ4RQWyUSCDicHqv3X2B8
:R9zZ4RQWyUSCDicHqv3X2B8 rdf:type owl:Class ;
                         rdfs:subClassOf :R89Yy2V18LstH4xGXyNb9XN ,
                                         [ rdf:type owl:Restriction ;
                                           owl:onProperty :RB4rNlczhggIx7lqdEK2d9c ;
                                           owl:someValuesFrom :R8CzBJHXymJx05c6sDhbspt
                                         ] ;
                         rdfs:isDefinedBy "ISO 12749-5:2018(en)  Nuclear energy, nuclear technologies, and radiological protection — Vocabulary — Part 5: Nuclear reactors "@en ;
                         <http://www.w3.org/2004/02/skos/core#altLabel> "NppSteamCondenser "@en ;
                         <http://www.w3.org/2004/02/skos/core#definition> "equipment in a steam turbine BOP (3.4.1.3), aimed at receiving the exhausting low-pressure turbine steam, bringing this fluid into the liquid state by massive cooling "@en ;
                         <http://www.w3.org/2004/02/skos/core#prefLabel> "SteamCondenser"@en .


###  http://w3id.org/emmo/domain/neo#RB5vIXZFuMYcHWSzNAPjPtF
:RB5vIXZFuMYcHWSzNAPjPtF rdf:type owl:Class ;
                         rdfs:subClassOf :RDpEA8qdRk99FAT0xSGZgGS ;
                         rdfs:comment """Residual heat transfer systems include systems designed to transfer heat from the residual heat removal systems to the ultimate heat sink.
 The capabilities to discharge residual heat to the ultimate heat sink are based on at least one heat sink and one heat transfer chain always being available for the different shutdown conditions."""@en ;
                         <http://www.w3.org/2004/02/skos/core#prefLabel> "RHROperation"@en .


###  http://w3id.org/emmo/domain/neo#RB8FKmPNbcy1ViUT2RE8alB
:RB8FKmPNbcy1ViUT2RE8alB rdf:type owl:Class ;
                         rdfs:subClassOf :R89Yy2V18LstH4xGXyNb9XN ,
                                         :RBsAUchYFBwAtcVUeFr8EFq ,
                                         [ rdf:type owl:Restriction ;
                                           owl:onProperty :RB4rNlczhggIx7lqdEK2d9c ;
                                           owl:someValuesFrom :R8CzBJHXymJx05c6sDhbspt
                                         ] ;
                         rdfs:isDefinedBy "ISO 17536-1:2015(en) Road vehicles — Aerosol separator performance test for internal combustion engines — Part 1: General" ;
                         <http://www.w3.org/2004/02/skos/core#altLabel> "NuclearBypassValve﻿"@en ;
                         <http://www.w3.org/2004/02/skos/core#definition> "Device to direct a portion of the flow around a separation device due to pressure difference, usually venting downstream of the bypassed separation device."@en ;
                         <http://www.w3.org/2004/02/skos/core#prefLabel> "BypassValve"@en .


###  http://w3id.org/emmo/domain/neo#RB8nGLKVMobwZ43LOnPJsjS
:RB8nGLKVMobwZ43LOnPJsjS rdf:type owl:Class ;
                         rdfs:subClassOf :RBUlm53v3Y42xdxWXvJZvzy ,
                                         :RDoeQzvUClmOY7fNhDvK0L1 ,
                                         [ rdf:type owl:Restriction ;
                                           owl:onProperty :RB4rNlczhggIx7lqdEK2d9c ;
                                           owl:someValuesFrom :R0ZnwwPdidaBfZOg6tgZJr
                                         ] ;
                         rdfs:isDefinedBy <https://www.nrc.gov/docs/ML1209/ML120970422.pdf> ;
                         <http://www.w3.org/2004/02/skos/core#altLabel> "ReactorStandbyLiquidControlSystem"@en ,
                                                                        "SLC"@en ;
                         <http://www.w3.org/2004/02/skos/core#definition> """The standby liquid control system injects a neutron poison (boron) into the reactor vessel to shutdown the chain reaction, independent of the control rods, and maintains the reactor shutdown as the plant is cooled to maintenance temperatures.
The standby liquid control system consists of a heated storage tank, two positive displacement pumps, two explosive valves, and the piping necessary to inject the neutron absorbing solution into the reactor vessel. The standby liquid control system is manually initiated and provides the operator with a relatively slow method of achieving reactor shutdown conditions."""@en ;
                         <http://www.w3.org/2004/02/skos/core#prefLabel> "StandbyLiquidControlSystem"@en .


###  http://w3id.org/emmo/domain/neo#RBA8h87iH1lIFBwAyDriYiS
:RBA8h87iH1lIFBwAyDriYiS rdf:type owl:Class ;
                         rdfs:subClassOf :R84TLuFmfSZMhgSh0uL0LXk ;
                         rdfs:isDefinedBy <https://www.chemeurope.com/en/encyclopedia/Neutron_detection.html> ;
                         <http://www.w3.org/2004/02/skos/core#definition> "Effective detection of neutrons entering a well-positioned detector"@en ;
                         <http://www.w3.org/2004/02/skos/core#prefLabel> "NeutronDetection"@en .


###  http://w3id.org/emmo/domain/neo#RBBzyqSEv3bIRXZvqAVCF4x
:RBBzyqSEv3bIRXZvqAVCF4x rdf:type owl:Class ;
                         rdfs:subClassOf :RLEjSGGgoWOVMGjQsskCsb ;
                         rdfs:isDefinedBy <https://en.wikipedia.org/wiki/Power_outage> ;
                         <http://www.w3.org/2004/02/skos/core#definition> "Is the loss of the electrical power network supply to an end user."@en ;
                         <http://www.w3.org/2004/02/skos/core#prefLabel> "NPPPowerLoss"@en .


###  http://w3id.org/emmo/domain/neo#RBHWfELWZVXyLNJa8MflI25
:RBHWfELWZVXyLNJa8MflI25 rdf:type owl:Class ;
                         rdfs:subClassOf :RBp2yVTrXRyb55JnYdvAGux ,
                                         :RDoeQzvUClmOY7fNhDvK0L1 ,
                                         [ rdf:type owl:Restriction ;
                                           owl:onProperty :RB4rNlczhggIx7lqdEK2d9c ;
                                           owl:someValuesFrom :R0ZnwwPdidaBfZOg6tgZJr
                                         ] ;
                         rdfs:isDefinedBy <https://www.nrc.gov/reading-rm/basic-ref/students/for-educators/03.pdf> ;
                         <http://www.w3.org/2004/02/skos/core#altLabel> "HPCI"@en ,
                                                                        "HighPressureEmergency CoreCoolingSystems"@en ,
                                                                        "ReactorHighPressureCoolantInjectionSystem"@en ;
                         <http://www.w3.org/2004/02/skos/core#definition> "The high pressure coolant injection (HPCI) system is an independent emergency core cooling system requiring no auxiliary ac power, plant air systems, or external cooling water systems to perform its purpose of providing make up water to the reactor vessel for core cooling under small and intermediate size loss of coolant accidents. The high pressure coolant injection system can supply make up water to the reactor vessel from above rated reactor pressure to a reactor pressure below that at which the low pressure emergency core cooling systems can inject."@en ;
                         <http://www.w3.org/2004/02/skos/core#prefLabel> "HighPressureCoolantInjectionSystem"@en .


###  http://w3id.org/emmo/domain/neo#RBJevCDiVa5kURep7JQX4ti
:RBJevCDiVa5kURep7JQX4ti rdf:type owl:Class ;
                         rdfs:subClassOf :R9p0u8Gh9Tup5P416Wl32S7 ;
                         rdfs:isDefinedBy <https://www.nrc.gov/reading-rm/basic-ref/glossary/activation.html> ;
                         <http://www.w3.org/2004/02/skos/core#definition> "The process of making a radioisotope by bombarding a stable element with neutrons or protons."@en ;
                         <http://www.w3.org/2004/02/skos/core#prefLabel> "NuclearActivation"@en .


###  http://w3id.org/emmo/domain/neo#RBPz6UINahiYOAyy7SWLOIs
:RBPz6UINahiYOAyy7SWLOIs rdf:type owl:Class ;
                         rdfs:subClassOf :R6dO6yatvM1kcW0Iuf8Z0R ,
                                         [ rdf:type owl:Restriction ;
                                           owl:onProperty :RB4rNlczhggIx7lqdEK2d9c ;
                                           owl:someValuesFrom :R0N27qMQzeRjM0vSOeAvUT
                                         ] ;
                         rdfs:comment "It is a label used within the Fukushima report to represent the entire system used in case of an emergency to restore power (electricity) in a Nuclear Power Plant."@en ,
                                      "They flooded the primary and backup power systems and equipment, as well as the ultimate heat sink systems and structures, of all six units on the site"@en ;
                         rdfs:seeAlso """Pag 2 , The Fukushima Daiichi Accident Technical Volume 1/5 
link: https://www-pub.iaea.org/MTCD/Publications/PDF/AdditionalVolumes/P1710/Pub1710-TV1-Web.pdf""" ;
                         <http://www.w3.org/2004/02/skos/core#prefLabel> "BackupPowerSystem"@en .


###  http://w3id.org/emmo/domain/neo#RBU28e2pgiTqsaTCPWnAJ6y
:RBU28e2pgiTqsaTCPWnAJ6y rdf:type owl:Class ;
                         rdfs:subClassOf elite:Process ,
                                         [ rdf:type owl:Restriction ;
                                           owl:onProperty elite:isAddedTo ;
                                           owl:someValuesFrom :R7ASmNcKrlRjzYHkUz3vfQT
                                         ] ,
                                         [ rdf:type owl:Restriction ;
                                           owl:onProperty [ owl:inverseOf elite:isSubProcessOf
                                                          ] ;
                                           owl:someValuesFrom :R7tsY17A1s9DZ7gbZrjbVt6
                                         ] ;
                         <http://www.w3.org/2004/02/skos/core#definition> "The process for producing energy from nuclear sources, in a reactor core of a nuclear power plant."@en ;
                         <http://www.w3.org/2004/02/skos/core#prefLabel> "ReactorCoreEnergyProduction"@en .


###  http://w3id.org/emmo/domain/neo#RBUlm53v3Y42xdxWXvJZvzy
:RBUlm53v3Y42xdxWXvJZvzy rdf:type owl:Class ;
                         rdfs:subClassOf :R7Ss5qBF98KBgXN3rhg0rEl ,
                                         :RBzruvoEUI9hIHVtX34kGJu ;
                         <http://www.w3.org/2004/02/skos/core#prefLabel> "SafetyInjectionSystem"@en .


###  http://w3id.org/emmo/domain/neo#RBW32C4x3sn1YahVG7uYVun
:RBW32C4x3sn1YahVG7uYVun rdf:type owl:Class ;
                         rdfs:subClassOf elite:Object ,
                                         [ rdf:type owl:Restriction ;
                                           owl:onProperty elite:isConstituentOf ;
                                           owl:someValuesFrom :R0N27qMQzeRjM0vSOeAvUT
                                         ] ;
                         rdfs:isDefinedBy <https://miro.com/app/board/uXjVN7uPMjA=/?moveToWidget=3458764577688681164&cot=14> ;
                         <http://www.w3.org/2004/02/skos/core#definition> "The central part of the a nuclear power plant in which the nuclear core is located and the fission reaction takes place"@en ;
                         <http://www.w3.org/2004/02/skos/core#prefLabel> "NuclearReactor"@en .


###  http://w3id.org/emmo/domain/neo#RBXC5sM9ZUESVnrsgaqxqxy
:RBXC5sM9ZUESVnrsgaqxqxy rdf:type owl:Class ;
                         rdfs:subClassOf :R7gZLWyPCimwGhHTueSRPhd ,
                                         :RDoeQzvUClmOY7fNhDvK0L1 ,
                                         [ rdf:type owl:Restriction ;
                                           owl:onProperty elite:isInputOf ;
                                           owl:someValuesFrom :RB5vIXZFuMYcHWSzNAPjPtF
                                         ] ,
                                         [ rdf:type owl:Restriction ;
                                           owl:onProperty :RB4rNlczhggIx7lqdEK2d9c ;
                                           owl:someValuesFrom :R0ZnwwPdidaBfZOg6tgZJr
                                         ] ;
                         rdfs:isDefinedBy <https://www.nrc.gov/docs/ML1209/ML120970422.pdf> ;
                         <http://www.w3.org/2004/02/skos/core#altLabel> "DecayHeatRemoval"@en ,
                                                                        "RHR"@en ,
                                                                        "ReactorResidualHeatRemovalSystem"@en ;
                         <http://www.w3.org/2004/02/skos/core#definition> "Heat is removed during normal power operation by generating steam in the reactor vessel and then using that steam to generate electrical energy. When the reactor is shutdown, the core will still continue to generate decay heat. The heat is removed by bypassing the turbine and dumping the steam directly to the condenser. The shutdown cooling mode of the residual heat removal (RHR) system is used to complete the cooldown process when pressure decreases to approximately 50 psig. Water is pumped from the reactor recirculation loop through a heat exchanger and back to the reactor via the recirculation loop. The recirculation loop is used to limit the number of penetrations into the reactor vessel."@en ;
                         <http://www.w3.org/2004/02/skos/core#prefLabel> "ResidualHeatRemovalSystem"@en .


###  http://w3id.org/emmo/domain/neo#RBabRZaZUznmBkL7QrHJTkR
:RBabRZaZUznmBkL7QrHJTkR rdf:type owl:Class ;
                         rdfs:subClassOf :R8hTHDGsCdkEbILOuzUhlEr ;
                         <http://www.w3.org/2004/02/skos/core#altLabel> "MainReactorAdminstratorBuilding" ;
                         <http://www.w3.org/2004/02/skos/core#prefLabel> "MainAdminstratorBuilding"@en .


###  http://w3id.org/emmo/domain/neo#RBeV8ftYy9jGBHA6rECN3Gx
:RBeV8ftYy9jGBHA6rECN3Gx rdf:type owl:Class ;
                         rdfs:subClassOf :RBzruvoEUI9hIHVtX34kGJu ,
                                         :Rw4mCgviqd6HTitZEzST6w ;
                         rdfs:comment "This report outlines the use of fire engines in an attempt to inject water into the reactors at Fukushima Daiichi. After the tsunami, much of the cooling function on-site was lost. The slides below document what fire engines were on site at what time, and what sources of water were injected where. Later research shows that little of the injected water made it to the reactors due to the lack of backflow valves in the fire line systems"@en ;
                         rdfs:seeAlso <https://fdada.info/develop/docs/pdf/ES-Unit123-04.pdf> ;
                         <http://www.w3.org/2004/02/skos/core#altLabel> "NPPFireEngine"@en ;
                         <http://www.w3.org/2004/02/skos/core#prefLabel> "FireEngine"@en .


###  http://w3id.org/emmo/domain/neo#RBfqFRty5Hp4V4caVtEvWdD
:RBfqFRty5Hp4V4caVtEvWdD rdf:type owl:Class ;
                         rdfs:subClassOf elite:PhysicalParticle ;
                         rdfs:isDefinedBy <https://www.iso.org/obp/ui/en/#iso:std:iso-iec:39794:-16:ed-1:v1:en:term:3.52> ;
                         <http://www.w3.org/2004/02/skos/core#definition> """subatomic particles used for neutron imaging (3.41) (NI) purposes by the neutron attenuation process in a similar fashion to X-rays (3.76)
Note 1 to entry: Neutron imaging can be used to detect changes in hydrogen abundance that can be correlated with the post-mortem (3.57) interval, i.e. the time that has elapsed since a person has died."""@en ;
                         <http://www.w3.org/2004/02/skos/core#prefLabel> "Neutron"@en .


###  http://w3id.org/emmo/domain/neo#RBimLTlArOY8mxOSFe6qiEZ
:RBimLTlArOY8mxOSFe6qiEZ rdf:type owl:Class ;
                         rdfs:subClassOf :Rw4mCgviqd6HTitZEzST6w ,
                                         [ rdf:type owl:Restriction ;
                                           owl:onProperty :RB4rNlczhggIx7lqdEK2d9c ;
                                           owl:someValuesFrom :R0ZnwwPdidaBfZOg6tgZJr
                                         ] ;
                         rdfs:comment "The RB surrounds the primary containment and provides the second fission product barrier and is commonly called as secondary containment. In case of an accident, the standby gas treatment system (SGTS), which needs AC power for operation, filters the gases and keeps the inside pressure below the atmospheric pressure to prevent radioactive materials release."@en ;
                         rdfs:seeAlso <https://www.tepco.co.jp/en/nu/fukushima-np/images/handouts_110827_02-e.pdf> ,
                                      """pag 74,The Fukushima Daiichi Accident Technical Volume 1/5 
link: https://www-pub.iaea.org/MTCD/Publications/PDF/AdditionalVolumes/P1710/Pub1710-TV1-Web.pdf""" ;
                         <http://www.w3.org/2004/02/skos/core#altLabel> "EmergencyGasTreatmentsystem"@en ,
                                                                        "ReactorStandbyGasTreatmentSystem"@en ,
                                                                        "SGTS"@en ;
                         <http://www.w3.org/2004/02/skos/core#prefLabel> "StandbyGasTreatmentSystem"@en .


###  http://w3id.org/emmo/domain/neo#RBnyfPxRohc9STM4mfSMMFq
:RBnyfPxRohc9STM4mfSMMFq rdf:type owl:Class ;
                         rdfs:subClassOf elite:Object ;
                         rdfs:isDefinedBy <https://www.iso.org/obp/ui/en/#iso:std:iso:14224:ed-3:v2:en:term:3.84> ;
                         <http://www.w3.org/2004/02/skos/core#definition> "equipment and items of permanent, temporary and portable equipment playing an important role in safety systems/functions"@en ;
                         <http://www.w3.org/2004/02/skos/core#prefLabel> "SafetyCriticalEquipment"@en .


###  http://w3id.org/emmo/domain/neo#RBp2yVTrXRyb55JnYdvAGux
:RBp2yVTrXRyb55JnYdvAGux rdf:type owl:Class ;
                         rdfs:subClassOf :RBzruvoEUI9hIHVtX34kGJu ,
                                         :RDoeQzvUClmOY7fNhDvK0L1 ,
                                         :Rw4mCgviqd6HTitZEzST6w ;
                         <http://www.w3.org/2004/02/skos/core#definition> "devices that aim to the limitation of any negative consequence (3.6) of a particular event, injecting refrigerants with the aim of decrease the temperature of the core and the pressure inside the Vessel"@en ;
                         <http://www.w3.org/2004/02/skos/core#prefLabel> "ReactorMitigationCoolingSystem"@en .


###  http://w3id.org/emmo/domain/neo#RBq5QrucFPH0MIg2wnaVaMD
:RBq5QrucFPH0MIg2wnaVaMD rdf:type owl:Class ;
                         rdfs:subClassOf :R7s6BZ18NYlgydAQozd7POd ;
                         rdfs:isDefinedBy """ISO 14624-5:2023(en)
Space systems — Safety and compatibility of materials — Part 5: Determination of reactivity of system/component materials with aerospace propellants"""@en ;
                         <http://www.w3.org/2004/02/skos/core#definition> "Adverse physical or chemical change in a substance"@en ;
                         <http://www.w3.org/2004/02/skos/core#prefLabel> "Degradation"@en .


###  http://w3id.org/emmo/domain/neo#RBq9x5WmblYOc4D7eFlfpdJ
:RBq9x5WmblYOc4D7eFlfpdJ rdf:type owl:Class ;
                         rdfs:subClassOf :R7pKuzitkkIAgc5NxDlqfH4 ;
                         rdfs:isDefinedBy <https://www.collinsdictionary.com/dictionary/english/explosion#:~:text=explosion%20in%20Chemical%20Engineering&text=An%20explosion%20is%20a%20sudden%20catastrophic%20release%20of%20energy%2C%20causing,container%20of%20pressurized%20gas%20ruptures.> ;
                         <http://www.w3.org/2004/02/skos/core#altLabel> "Blast"@en ;
                         <http://www.w3.org/2004/02/skos/core#definition> "An explosion is a sudden catastrophic release of energy, causing a pressure wave. An explosion happens when a free gas expands very quickly, because of a chemical reaction that produces a gas, or because a container of pressurized gas ruptures."@en ;
                         <http://www.w3.org/2004/02/skos/core#prefLabel> "Explosion"@en .


###  http://w3id.org/emmo/domain/neo#RBr5qtxSEMQ2oYZd1frAYZL
:RBr5qtxSEMQ2oYZd1frAYZL rdf:type owl:Class ;
                         rdfs:subClassOf :R80RaxHVqr4QPiv8ASxXxi3 ;
                         rdfs:isDefinedBy <https://www.iso.org/obp/ui/en/#iso:std:iso:iwa:33:-1:ed-1:v1:en:term:11.6.1.3> ;
                         <http://www.w3.org/2004/02/skos/core#altLabel> "ManualControl"@en ,
                                                                        "ManualManipulation"@en ;
                         <http://www.w3.org/2004/02/skos/core#definition> "Control in which the system or main device, whether direct or power-aided in operation, is directly controlled by an operator"@en ;
                         <http://www.w3.org/2004/02/skos/core#prefLabel> "ManualControlling"@en .


###  http://w3id.org/emmo/domain/neo#RBsAUchYFBwAtcVUeFr8EFq
:RBsAUchYFBwAtcVUeFr8EFq rdf:type owl:Class ;
                         rdfs:subClassOf elite:Object ;
                         rdfs:isDefinedBy <https://www.iso.org/obp/ui/en/#iso:std:iso:23551:-1:ed-2:v1:en:term:3.101.1> ;
                         <http://www.w3.org/2004/02/skos/core#definition> """device consisting essentially of a valve body, closure member, and actuator that controls the flow of gas
Note 1 to entry: The actuation can be done by gas pressure, electrical, hydraulic, manual or pneumatic energy."""@en ;
                         <http://www.w3.org/2004/02/skos/core#prefLabel> "Valve"@en .


###  http://w3id.org/emmo/domain/neo#RBtkzbuLn6g0vdtDU3mijH0
:RBtkzbuLn6g0vdtDU3mijH0 rdf:type owl:Class ;
                         rdfs:subClassOf :RLEjSGGgoWOVMGjQsskCsb ,
                                         :RRxSYO9r2FD1rHmRPugfob ,
                                         [ rdf:type owl:Restriction ;
                                           owl:onProperty elite:hasNext ;
                                           owl:someValuesFrom :RCP7vIugzt8V7rXL11buOZH
                                         ] ;
                         rdfs:comment "here there are all the events that can lead to the degradation of the core," ;
                         rdfs:isDefinedBy <http://www-ns.iaea.org/downloads/ni/training/specific_expert_knowledge/psa-level1/III1_1_A%20%20Initiating%20Event%20Analysis.pdf> ;
                         <http://www.w3.org/2004/02/skos/core#altLabel> "InitiatingEvent"@en ;
                         <http://www.w3.org/2004/02/skos/core#definition> "An event that creates a disturbance. in the plant and has a potential to lead to core damage, depending on the successful operation of the various mitigating systems of the plant"@en ;
                         <http://www.w3.org/2004/02/skos/core#prefLabel> "NuclearAccidentInitiatingEvent"@en .


###  http://w3id.org/emmo/domain/neo#RBuKou8LHvh6qFQkn5YcvzK
:RBuKou8LHvh6qFQkn5YcvzK rdf:type owl:Class ;
                         rdfs:subClassOf :R0N27qMQzeRjM0vSOeAvUT ;
                         rdfs:comment "The nuclear reactors and the electric production lines can be either almost identical or different between them, though usually sharing various support or auxiliary installations, systems and/or supplies (ISO 12749-5:2018)"@en ;
                         rdfs:isDefinedBy <https://www.iso.org/obp/ui/#iso:std:iso:12749:-5:ed-1:v1:en:term:3.4.1.2> ;
                         <http://www.w3.org/2004/02/skos/core#altLabel> "MultipleUnitNPP"@en ;
                         <http://www.w3.org/2004/02/skos/core#definition> "Nuclear power plant  having on a common site, two or more electric production lines (ISO 12749-5:2018)"@en ;
                         <http://www.w3.org/2004/02/skos/core#example> "Tennessee Valley Authority Browns Ferry Nuclear Plant (Athens, Alabama, United States)"@en ;
                         <http://www.w3.org/2004/02/skos/core#prefLabel> "MultipleUnitNuclearPowerPlant"@en .


###  http://w3id.org/emmo/domain/neo#RBv35jM3VSFKKxtWNVyDILw
:RBv35jM3VSFKKxtWNVyDILw rdf:type owl:Class ;
                         rdfs:subClassOf :Rryk3Z5XNZ11ZiiLuT5M8Q ;
                         rdfs:isDefinedBy <https://www-pub.iaea.org/MTCD/Publications/PDF/PUB1830_web.pdf> ;
                         <http://www.w3.org/2004/02/skos/core#altLabel> "Assessment"@en ;
                         <http://www.w3.org/2004/02/skos/core#definition> "The process, and the result, of analysing systematically and evaluating the hazards associated with sources and practices, and associated protection and safety measures."@en ;
                         <http://www.w3.org/2004/02/skos/core#prefLabel> "RadioactivityAssessment"@en .


###  http://w3id.org/emmo/domain/neo#RBvFxrHecZjciXe2qvDn2vv
:RBvFxrHecZjciXe2qvDn2vv rdf:type owl:Class ;
                         rdfs:subClassOf :RRxSYO9r2FD1rHmRPugfob ,
                                         [ rdf:type owl:Restriction ;
                                           owl:onProperty elite:hasNext ;
                                           owl:someValuesFrom :RC9Vnqc96TS4VVdygnxu8UP
                                         ] ;
                         <http://www.w3.org/2004/02/skos/core#definition> """A PIE Is an event identified in the
design that leads to Anticipated Operational Occurrences (AOOs)conditions."""@en ;
                         <http://www.w3.org/2004/02/skos/core#prefLabel> "AnticipatedOperationalOccurrenceEvent"@en .


###  http://w3id.org/emmo/domain/neo#RBwST6x27zdyWBgBunjc2Q9
:RBwST6x27zdyWBgBunjc2Q9 rdf:type owl:Class ;
                         rdfs:subClassOf :R1DAH32q3UDTp3GZGqe5Re ;
                         <http://www.w3.org/2004/02/skos/core#prefLabel> "ControlRodInsertion"@en .


###  http://w3id.org/emmo/domain/neo#RBzruvoEUI9hIHVtX34kGJu
:RBzruvoEUI9hIHVtX34kGJu rdf:type owl:Class ;
                         rdfs:subClassOf elite:Object ,
                                         [ rdf:type owl:Restriction ;
                                           owl:onProperty elite:participatesTo ;
                                           owl:someValuesFrom :R8MPIXNWSb8RCelrAeGNxMc
                                         ] ;
                         rdfs:isDefinedBy <https://www.iso.org/obp/ui/en/#iso:std:iso:6877:ed-3:v1:en:term:3.11> ;
                         <http://www.w3.org/2004/02/skos/core#definition> "instrument designed to obturate a root canal with thermoplasticized injection material (3.9) using an injection equipment or device"@en ;
                         <http://www.w3.org/2004/02/skos/core#prefLabel> "InjectionSystems"@en .


###  http://w3id.org/emmo/domain/neo#RC1aeRG1szxYdt4kTKUUOvO
:RC1aeRG1szxYdt4kTKUUOvO rdf:type owl:Class ;
                         rdfs:subClassOf :R8MPIXNWSb8RCelrAeGNxMc ,
                                         [ rdf:type owl:Restriction ;
                                           owl:onProperty elite:isConstitutiveProcessOf ;
                                           owl:someValuesFrom :RBp2yVTrXRyb55JnYdvAGux
                                         ] ;
                         :R8xx0dhbEh1tjGMDwNZfckV "Activation of the Core Spray System in which coolant is sent through the discharge path to the core spray sparger using core spray pumps."@en ;
                         rdfs:isDefinedBy <https://www.nrc.gov/docs/ML1125/ML11258A368.pdf> ;
                         <http://www.w3.org/2004/02/skos/core#altLabel> "CoreSpray"@en ;
                         <http://www.w3.org/2004/02/skos/core#prefLabel> "SprayInjection"@en .


###  http://w3id.org/emmo/domain/neo#RC5Uc3vBrAsYC8gCNkTsLH
:RC5Uc3vBrAsYC8gCNkTsLH rdf:type owl:Class ;
                        rdfs:subClassOf :R8MPIXNWSb8RCelrAeGNxMc ;
                        <http://www.w3.org/2004/02/skos/core#definition> "Material Injection following a well defined cycle without alterations."@en ;
                        <http://www.w3.org/2004/02/skos/core#prefLabel> "RegularInjection"@en .


###  http://w3id.org/emmo/domain/neo#RC5rdqmZ9FmptamkomAjr4J
:RC5rdqmZ9FmptamkomAjr4J rdf:type owl:Class ;
                         rdfs:subClassOf :R7QpMP9Mf1mRrRVeMT7UcIX ;
                         :RR3uD2d7YfhHohfv2Nm6sX "Fission products and actinides produced by neutron absorption of nuclear fuel itself are normally referred to by those specific names, and activation product reserved for products of neutron capture by other materials, such as structural components of the nuclear reactor or nuclear bomb, the reactor coolant, control rods or other neutron poisons, or materials in the environment. All of these, however, need to be handled as radioactive waste. Some nuclides originate in more than one way, as activation products or fission products."@en ;
                         rdfs:isDefinedBy <https://en.wikipedia.org/wiki/Activation_product> ;
                         <http://www.w3.org/2004/02/skos/core#definition> "An activation product is a material that has been made radioactive by the process of neutron activation."@en ;
                         <http://www.w3.org/2004/02/skos/core#prefLabel> "ActivatedMaterial"@en .


###  http://w3id.org/emmo/domain/neo#RC9Vnqc96TS4VVdygnxu8UP
:RC9Vnqc96TS4VVdygnxu8UP rdf:type owl:Class ;
                         rdfs:subClassOf :RtdecAtZ9C9xUJNtjefY4D ;
                         rdfs:comment """Conditions of normal operation that are expected to occur one or
more times during the life of the nuclear power unit and include but
are not limited to loss of power to all recirculation pumps, tripping of
the turbine generator set, isolation of the main condenser, and loss of
all offsite power."""@en ,
                                      "Level 2: Monitoring for abnormal conditions and providing associated control functions"@en ,
                                      "These are procedures only in the case of deviation of standard operation"@en ,
                                      """def ISO)      Operation of the appliance under the effect of internal failures or under the effect of foreseeable influences outside the specified operational conditions

def IAEA)     A deviation of an operational process from normal operation that is expected to occur at least once during the operating lifetime of a facility but which, in view of appropriate design provisions, does not cause any significant damage to items important to safety or lead to accident conditions"""@en ;
                         rdfs:isDefinedBy """ISO 23552-1:2007(en)
Safety and control devices for gas and/or oil burners and gas and/or oil appliances — Particular requirements — Part 1: Fuel/air ratio controls, electronic type

https://www-ns.iaea.org/downloads/standards/glossary/iaea-safety-glossary-draft-2016.pdf""" ;
                         rdfs:seeAlso "INTERNATIONAL ATOMIC ENERGY AGENCY, Approaches for Overall Instrumentation and Control Architectures of Nuclear Power Plants, IAEA Nuclear Energy Series No. NP-T-2.11, IAEA, Vienna (2018)" ;
                         <http://www.w3.org/2004/02/skos/core#altLabel> "DiDLevel2"@en ;
                         <http://www.w3.org/2004/02/skos/core#definition> """Control of deviations from normal operating states to prevent anticipated operational occurrences from
escalating to accident conditions. This can be provided both by electronic means and by operator intervention,
if there is enough time and information for such actions to be credited. The algorithms used are different
from control."""@en ;
                         <http://www.w3.org/2004/02/skos/core#prefLabel> "AOOControl"@en .


###  http://w3id.org/emmo/domain/neo#RCAHezyl4VRbtyt3dbnxBUb
:RCAHezyl4VRbtyt3dbnxBUb rdf:type owl:Class ;
                         rdfs:subClassOf :RDoeQzvUClmOY7fNhDvK0L1 ,
                                         [ rdf:type owl:Restriction ;
                                           owl:onProperty :RB4rNlczhggIx7lqdEK2d9c ;
                                           owl:someValuesFrom :R0ZnwwPdidaBfZOg6tgZJr
                                         ] ;
                         rdfs:isDefinedBy "ISO 21843:2023(en) Determination of the resistance to hydrocarbon pool fires of fire protection materials and systems for pressure vessels" ;
                         <http://www.w3.org/2004/02/skos/core#altLabel> "ReactorThermalProtectionSystem"@en ;
                         <http://www.w3.org/2004/02/skos/core#definition> "protection afforded to the vessel to reduce the rate of heat transfer from the fire to the vessel, throughout the period of exposure to fire, including any protection materials together with any encasement (such as a jacket), and supporting system (such as mesh reinforcement or a framing system) and any specified primer and top coat if applicable."@en ;
                         <http://www.w3.org/2004/02/skos/core#prefLabel> "ThermalProtectionSystem"@en .


###  http://w3id.org/emmo/domain/neo#RCDLrZ9KyXAspBK0GpRfHxG
:RCDLrZ9KyXAspBK0GpRfHxG rdf:type owl:Class ;
                         rdfs:subClassOf :R6dO6yatvM1kcW0Iuf8Z0R ,
                                         :RDoeQzvUClmOY7fNhDvK0L1 ,
                                         [ rdf:type owl:Restriction ;
                                           owl:onProperty elite:isInputOf ;
                                           owl:someValuesFrom :R1DAH32q3UDTp3GZGqe5Re
                                         ] ,
                                         [ rdf:type owl:Restriction ;
                                           owl:onProperty elite:isInputOf ;
                                           owl:someValuesFrom :R80L6MpJJVkL4hoNB7thCRV
                                         ] ,
                                         [ rdf:type owl:Restriction ;
                                           owl:onProperty :RB4rNlczhggIx7lqdEK2d9c ;
                                           owl:someValuesFrom :R70ZOvZxdVYhbMrv2o1bK8I
                                         ] ;
                         rdfs:isDefinedBy <https://www.nrc.gov/docs/ML1125/ML11258A305.pdf> ;
                         <http://www.w3.org/2004/02/skos/core#altLabel> "CRD﻿"@en ;
                         <http://www.w3.org/2004/02/skos/core#definition> "PURPOSES: To make changes in core reactivity by positioning control rods in response to the Reactor Manual Control System (RMCS) signals. To rapidly insert all control rods to shutdown the reactor in response to the Reactor Protection System (RPS) signals.  To provide cooling water for the reactor recirculation and reactor water cleanup pump seals."@en ;
                         <http://www.w3.org/2004/02/skos/core#prefLabel> "ControlRodDriveSystem"@en .


###  http://w3id.org/emmo/domain/neo#RCEdHiyMqhUSNg53tLciXxW
:RCEdHiyMqhUSNg53tLciXxW rdf:type owl:Class ;
                         rdfs:subClassOf :RC9Vnqc96TS4VVdygnxu8UP ;
                         rdfs:isDefinedBy <https://www.nrc.gov/docs/ML1125/ML11258A312.pdf> ;
                         <http://www.w3.org/2004/02/skos/core#definition> """Provide makeup water to the reactor vessel for core cooling when:
the main steam lines are isolated
the condensate and feedwater system is not available."""@en ;
                         <http://www.w3.org/2004/02/skos/core#prefLabel> "RCICOperation"@en .


###  http://w3id.org/emmo/domain/neo#RCJLElMudONs6LAhEPd8PjG
:RCJLElMudONs6LAhEPd8PjG rdf:type owl:Class ;
                         rdfs:subClassOf :Rw4mCgviqd6HTitZEzST6w ,
                                         [ rdf:type owl:Restriction ;
                                           owl:onProperty :RB4rNlczhggIx7lqdEK2d9c ;
                                           owl:someValuesFrom :R0N27qMQzeRjM0vSOeAvUT
                                         ] ;
                         rdfs:comment "A water injection line was installed by connecting 3 fire engines in series and using the Unit 3 reverse cleaning valve pit as water source, to start seawater injection to Unit 1 at 19:04."@en ,
                                      "The Site Superintendent then decided to inject seawater into the Unit 1 reactor from the Unit 3 backwash valve pit, where seawater had pooled after the tsunami, as it was the only available source of water at that time."@en ;
                         rdfs:seeAlso <https://fdada.info/develop/docs/pdf/ES-Unit123-04.pdf> ,
                                      """Pag 21, The Fukushima Daiichi Accident Technical Volume 1/5 
link: https://www-pub.iaea.org/MTCD/Publications/PDF/AdditionalVolumes/P1710/Pub1710-TV1-Web.pdf"""@en ;
                         <http://www.w3.org/2004/02/skos/core#altLabel> "ReverseCleaningValvePit"@en ;
                         <http://www.w3.org/2004/02/skos/core#prefLabel> "BackwashValvePit"@en .


###  http://w3id.org/emmo/domain/neo#RCJhKs4unBpoZD0uMgxsvJh
:RCJhKs4unBpoZD0uMgxsvJh rdf:type owl:Class ;
                         rdfs:subClassOf :RlYMwSSvmqekLRLzmf5IzV ;
                         rdfs:comment "in an electric circuit" ;
                         rdfs:isDefinedBy <https://dictionary.cambridge.org/it/dizionario/inglese/switching> ;
                         <http://www.w3.org/2004/02/skos/core#definition> "to use a switch to change a device from one state or type of operation to another"@en ;
                         <http://www.w3.org/2004/02/skos/core#prefLabel> "Switching"@en .


###  http://w3id.org/emmo/domain/neo#RCJyL3ZfDUXJeZ2m8EwYQO9
:RCJyL3ZfDUXJeZ2m8EwYQO9 rdf:type owl:Class ;
                         rdfs:subClassOf :R7oHlh8OgEkyG3XXGpiYlC5 ;
                         rdfs:seeAlso <https://www-ns.iaea.org/downloads/standards/glossary/iaea-safety-glossary-draft-2016.pdf> ;
                         <http://www.w3.org/2004/02/skos/core#definition> "Loss of the ability of a system to function within acceptance criteria. The system is considered to fail when it becomes incapable of functioning, whether or not this is needed at that time."@en ;
                         <http://www.w3.org/2004/02/skos/core#prefLabel> "SystemFailure"@en .


###  http://w3id.org/emmo/domain/neo#RCNShAJHX3mIvlEif02qYJZ
:RCNShAJHX3mIvlEif02qYJZ rdf:type owl:Class ;
                         rdfs:subClassOf :RlYMwSSvmqekLRLzmf5IzV ;
                         rdfs:isDefinedBy <https://www.iso.org/obp/ui/en/#iso:std:iso:tr:27923:ed-1:v1:en:term:3.22> ;
                         <http://www.w3.org/2004/02/skos/core#altLabel> "NuclearReactorDecommissioning"@en ;
                         <http://www.w3.org/2004/02/skos/core#definition> "take an engineered system or component out of service, render it inoperative, dismantle and decontaminate it"@en ;
                         <http://www.w3.org/2004/02/skos/core#prefLabel> "NPPDecommissioning" .


###  http://w3id.org/emmo/domain/neo#RCP7vIugzt8V7rXL11buOZH
:RCP7vIugzt8V7rXL11buOZH rdf:type owl:Class ;
                         rdfs:subClassOf elite:Process ,
                                         elite:Whole ;
                         rdfs:comment "Any accident involving facilities or activities from which a release of radioactive material occurs or is likely to occur and which has resulted or may result in an international significant transboundary release that could be of radiological safety significance for another State"@en ,
                                      "This is not explicitly stated to be a definition of nuclear accident, but it is derived from the statement of the scope of application in Article 1 of the Convention on Early Notification of a Nuclear Accident. However, this Convention has a limited scope of application, and it is unreasonable to consider a nuclear accident to be only an accident that results or may result in an international significant transboundary release"@en ;
                         rdfs:seeAlso <https://www-ns.iaea.org/downloads/standards/glossary/iaea-safety-glossary-draft-2016.pdf> ;
                         <http://www.w3.org/2004/02/skos/core#definition> "Nuclear Plant Accident are any accident involving nuclear plant causing a radioactivity release. Depending on the magnitude of radioactive release there are different type of Nuclear Accident." ;
                         <http://www.w3.org/2004/02/skos/core#prefLabel> "NuclearPlantAccident"@en .


###  http://w3id.org/emmo/domain/neo#RCPFRkyBbFadwcQUuWavdPl
:RCPFRkyBbFadwcQUuWavdPl rdf:type owl:Class ;
                         rdfs:subClassOf :RDoeQzvUClmOY7fNhDvK0L1 ,
                                         :Rw4mCgviqd6HTitZEzST6w ;
                         rdfs:comment """1.On the IAEA report is called \"primary containment system\".

2.The Primary Containment consists of a drywell which encloses the reactor vessel and recirculation system, a pressure suppression chamber which stores a large volume of water, a connecting vent system between the drywell and the suppression chamber, isolation valves and containment atmosphere control systems. (https://www.nrc.gov/docs/ML1215/ML12159A162.pdf)"""@en ;
                         rdfs:isDefinedBy "ISO 17873:2004(en) Nuclear facilities — Criteria for the design and operation of ventilation systems for nuclear installations other than nuclear reactors ﻿" ;
                         <http://www.w3.org/2004/02/skos/core#altLabel> "ReactorShieldCoolingSystem "@en ;
                         <http://www.w3.org/2004/02/skos/core#definition> "System constituted by a coherent set of physical barriers and/or auxiliary dynamic systems intended to confine radioactive substances in order to ensure the safety of the workers and the public and the protection of the environment ."@en ;
                         <http://www.w3.org/2004/02/skos/core#prefLabel> "ReactorContainmentSystem"@en .


###  http://w3id.org/emmo/domain/neo#RCPsVMpkrs5EqK8G9HKv71m
:RCPsVMpkrs5EqK8G9HKv71m rdf:type owl:Class ;
                         rdfs:subClassOf :R8hTHDGsCdkEbILOuzUhlEr ;
                         <http://www.w3.org/2004/02/skos/core#altLabel> "NuclearSeismicallyIsolatedBuilding﻿"@en ;
                         <http://www.w3.org/2004/02/skos/core#prefLabel> "SeismicallyIsolatedBuilding"@en .


###  http://w3id.org/emmo/domain/neo#RCRVu2hmIevYnx0eZzyJEPs
:RCRVu2hmIevYnx0eZzyJEPs rdf:type owl:Class ;
                         rdfs:subClassOf :RDoeQzvUClmOY7fNhDvK0L1 ,
                                         [ rdf:type owl:Restriction ;
                                           owl:onProperty :RB4rNlczhggIx7lqdEK2d9c ;
                                           owl:someValuesFrom :R85FFwLPHIursWfa6K6sKK9
                                         ] ;
                         rdfs:isDefinedBy "﻿ISO 21347:2005(en)  Space systems — Fracture and damage control﻿"@en ;
                         <http://www.w3.org/2004/02/skos/core#altLabel> "RPV"@en ;
                         <http://www.w3.org/2004/02/skos/core#definition> """container designed primarily for the storage of pressurized fluid, which fulfils at least one of the following criteria:

    a) contains gas or liquid with high energy level;
    b) contains gas or liquid which will create a mishap (accident) if released;
    c) contains gas or liquid with high pressure level﻿"""@en ;
                         <http://www.w3.org/2004/02/skos/core#prefLabel> "ReactorPressureVessel"@en .


###  http://w3id.org/emmo/domain/neo#RCV3rrs00sLryJLTlXR60QN
:RCV3rrs00sLryJLTlXR60QN rdf:type owl:Class ;
                         rdfs:subClassOf :R8hTHDGsCdkEbILOuzUhlEr ;
                         <http://www.w3.org/2004/02/skos/core#altLabel> "ReactorDieselGeneratorBuilding﻿"@en ;
                         <http://www.w3.org/2004/02/skos/core#prefLabel> "DieselGeneratorBuilding"@en .


###  http://w3id.org/emmo/domain/neo#RCY8ddT8JW7G3WicejAxkmn
:RCY8ddT8JW7G3WicejAxkmn rdf:type owl:Class ;
                         rdfs:subClassOf :RCJhKs4unBpoZD0uMgxsvJh ;
                         <http://www.w3.org/2004/02/skos/core#comment> "from off to on" ;
                         <http://www.w3.org/2004/02/skos/core#prefLabel> "SwitchingOn"@en .


###  http://w3id.org/emmo/domain/neo#RCZ2I1XktaR3DBBEbLjHwOz
:RCZ2I1XktaR3DBBEbLjHwOz rdf:type owl:Class ;
                         rdfs:subClassOf :R7MjWOBoCnDd3BD1IBHjlRe ,
                                         [ rdf:type owl:Restriction ;
                                           owl:onProperty :RB4rNlczhggIx7lqdEK2d9c ;
                                           owl:someValuesFrom :RCPsVMpkrs5EqK8G9HKv71m
                                         ] ;
                         rdfs:isDefinedBy <https://ec.europa.eu/echo/files/media/publications/2013/ERC_en.pdf> ;
                         <http://www.w3.org/2004/02/skos/core#altLabel> "ERCs"@en ,
                                                                        "NppEmergencyResponseCentres"@en ;
                         <http://www.w3.org/2004/02/skos/core#definition> "The Emergency Response Centre (ERC) is the operational heart of the EU Civil Protection Mechanism. It enables the European Union to respond to overwhelming natural and man-made disasters quickly and efficiently, both inside and outside Europe. "@en ;
                         <http://www.w3.org/2004/02/skos/core#prefLabel> "EmergencyResponseCentres"@en .


###  http://w3id.org/emmo/domain/neo#RCcdLHL2BqdRJQkmiKL4MDW
:RCcdLHL2BqdRJQkmiKL4MDW rdf:type owl:Class ;
                         rdfs:subClassOf :R8lgbjRv5CeOJ43GygJ143n ;
                         rdfs:isDefinedBy <https://www.iso.org/obp/ui/en/#iso:std:iso:22328:-3:ed-1:v1:en:term:3.2> ;
                         <http://www.w3.org/2004/02/skos/core#definition> "Sudden and violent shaking of the ground, sometimes causing great destruction, as a result of movements within the earth’s crust or volcanic action."@en ;
                         <http://www.w3.org/2004/02/skos/core#prefLabel> "Earthquake"@en .


###  http://w3id.org/emmo/domain/neo#RCembrpB4dbduwWjlJOBBMK
:RCembrpB4dbduwWjlJOBBMK rdf:type owl:Class ;
                         rdfs:subClassOf :RC9Vnqc96TS4VVdygnxu8UP ;
                         rdfs:comment """Confinement is closely related in meaning to containment, but confinement is
typically used to refer to the safety function of preventing the ‘escape’ of radioactive
material, whereas containment refers to the means for achieving that function.
 ! The Transport Regulations [2] adopt a different distinction between confinement
and containment, namely that confinement relates to preventing criticality and
containment to preventing releases of radioactive material (see confinement system
and containment system).
	The main issue here is the differences in usage between the safety of nuclear
installations and safety in the transport of radioactive material. Both terms,
containment and confinement, are used in both areas (in the Transport
Regulations [2], in the form of confinement system and containment system), and
the usages of containment are (it seems) conceptually consistent, but the usages
of confinement are not. Confinement in nuclear safety is the safety function that is
performed by the containment."""@en ;
                         rdfs:isDefinedBy "https://www-pub.iaea.org/MTCD/Publications/PDF/PUB1830_web.pdf p" ;
                         <http://www.w3.org/2004/02/skos/core#definition> """Prevention or control of releases of radioactive material to the environment
in operation or in accidents."""@en ;
                         <http://www.w3.org/2004/02/skos/core#prefLabel> "Confinement"@en .


###  http://w3id.org/emmo/domain/neo#RCfqimjBP1uypJVnd32xcTB
:RCfqimjBP1uypJVnd32xcTB rdf:type owl:Class ;
                         rdfs:subClassOf :RLEjSGGgoWOVMGjQsskCsb ,
                                         [ rdf:type owl:Restriction ;
                                           owl:onProperty elite:isBehaviourOf ;
                                           owl:someValuesFrom :RvBQlxDEMRtFxiHtMstrYY
                                         ] ;
                         rdfs:comment "Seawater injection into Unit 1 was ready to be resumed upon the refilling of the backwash valve pit, but all activities, including the ongoing seawater injection into the Unit 3 reactor, had to stop because of an explosion in Unit 3 (Par. 1.1.3.21., pp 26-27)"@en ;
                         rdfs:seeAlso "Pub1710-TV1-Web.pdf"@en ;
                         <http://www.w3.org/2004/02/skos/core#prefLabel> "LossOfSeaWaterCooling"@en .


###  http://w3id.org/emmo/domain/neo#RCh38CRTgX4tnzCoB8auwPC
:RCh38CRTgX4tnzCoB8auwPC rdf:type owl:Class ;
                         rdfs:subClassOf :R7hYLnBucjQ8XgAj5RsQvpF ,
                                         [ rdf:type owl:Restriction ;
                                           owl:onProperty :RB4rNlczhggIx7lqdEK2d9c ;
                                           owl:someValuesFrom :RCV3rrs00sLryJLTlXR60QN
                                         ] ;
                         rdfs:isDefinedBy <https://inis.iaea.org/collection/NCLCollectionStore/_Public/26/044/26044983.pdf?r=1> ;
                         <http://www.w3.org/2004/02/skos/core#definition> """Emergency Diesel Generators (EDGs) provide on-site emergency alternating current (ac) electric
power for a nuclear plant in the event that all off-site power sources are lost.""" ;
                         <http://www.w3.org/2004/02/skos/core#prefLabel> "DieselGenerator"@en .


###  http://w3id.org/emmo/domain/neo#RCsCw5Imj0XgbP0uOlzcQNe
:RCsCw5Imj0XgbP0uOlzcQNe rdf:type owl:Class ;
                         rdfs:subClassOf :RBnyfPxRohc9STM4mfSMMFq ;
                         rdfs:isDefinedBy "ISO 11675:2005(en)  Textile machinery and accessories — Flatbed knitting machines — Vocabulary " ;
                         <http://www.w3.org/2004/02/skos/core#altLabel> "NppProtectiveGear﻿"@en ;
                         <http://www.w3.org/2004/02/skos/core#definition> "Gear for the prevention of accidents "@en ;
                         <http://www.w3.org/2004/02/skos/core#prefLabel> "ProtectiveGear"@en .


###  http://w3id.org/emmo/domain/neo#RCuTNyDF6kWFazFqJVIvww9
:RCuTNyDF6kWFazFqJVIvww9 rdf:type owl:Class ;
                         rdfs:subClassOf :RCJhKs4unBpoZD0uMgxsvJh ;
                         rdfs:comment "from on to off" ;
                         <http://www.w3.org/2004/02/skos/core#prefLabel> "SwitchingOff"@en .


###  http://w3id.org/emmo/domain/neo#RCzybo2ACvDW8XnRRQcoQTg
:RCzybo2ACvDW8XnRRQcoQTg rdf:type owl:Class ;
                         rdfs:subClassOf :RDoeQzvUClmOY7fNhDvK0L1 ,
                                         [ rdf:type owl:Restriction ;
                                           owl:onProperty elite:isConstituentOf ;
                                           owl:someValuesFrom :RyMmVkVf9zClluOSgfr1Rh
                                         ] ;
                         rdfs:isDefinedBy """IAEA Safety Glossary, Terminology Used in Nuclear Safety 
and Radiation Protection, 2018 Edition """ ;
                         <http://www.w3.org/2004/02/skos/core#definition> """A set of fuel elements and associated components which are loaded into and
subsequently removed from a reactor core as a single unit."""@en ;
                         <http://www.w3.org/2004/02/skos/core#prefLabel> "FuelAssembly"@en .


###  http://w3id.org/emmo/domain/neo#RDA28A6LQxSBpe6UXyS1BwW
:RDA28A6LQxSBpe6UXyS1BwW rdf:type owl:Class ;
                         rdfs:subClassOf :R89Yy2V18LstH4xGXyNb9XN ,
                                         [ rdf:type owl:Restriction ;
                                           owl:onProperty :RB4rNlczhggIx7lqdEK2d9c ;
                                           owl:someValuesFrom :R8CzBJHXymJx05c6sDhbspt
                                         ] ;
                         <http://www.w3.org/2004/02/skos/core#altLabel> "NPPFeedwaterPump"@en ;
                         <http://www.w3.org/2004/02/skos/core#prefLabel> "FeedwaterPump"@en .


###  http://w3id.org/emmo/domain/neo#RDCVLkjId3erZ4ajIA6nHzM
:RDCVLkjId3erZ4ajIA6nHzM rdf:type owl:Class ;
                         rdfs:subClassOf :R7NYEyrtAsNuF6n0QNOFmHm ,
                                         :R89Yy2V18LstH4xGXyNb9XN ,
                                         [ rdf:type owl:Restriction ;
                                           owl:onProperty :RB4rNlczhggIx7lqdEK2d9c ;
                                           owl:someValuesFrom :R8CzBJHXymJx05c6sDhbspt
                                         ] ;
                         rdfs:isDefinedBy "ISO 11086:1996(en) Gas turbines — Vocabulary " ;
                         <http://www.w3.org/2004/02/skos/core#altLabel> "NppPowerTurbine"@en ;
                         <http://www.w3.org/2004/02/skos/core#definition> "Turbine which is driven by the gases from a gas generator, producing power output from the gas turbine through an independent shaft."@en ;
                         <http://www.w3.org/2004/02/skos/core#prefLabel> "PowerTurbine"@en .


###  http://w3id.org/emmo/domain/neo#RDDFiZC2RFaE7RrTNF0CrtA
:RDDFiZC2RFaE7RrTNF0CrtA rdf:type owl:Class ;
                         rdfs:subClassOf :Rw4mCgviqd6HTitZEzST6w ;
                         rdfs:comment """The fire protection system was designed primarily for fire suppression and flooding of the containment vessel, not for
injection of water into the reactor."""@en ;
                         rdfs:seeAlso <https://fdada.info/develop/docs/pdf/ES-Unit123-04.pdf> ,
                                      """Pag 17, The Fukushima Daiichi Accident Technical Volume 1/5 
link: https://www-pub.iaea.org/MTCD/Publications/PDF/AdditionalVolumes/P1710/Pub1710-TV1-Web.pdf"""@en ;
                         <http://www.w3.org/2004/02/skos/core#altLabel> "NPPFireProtectionSystem"@en ;
                         <http://www.w3.org/2004/02/skos/core#prefLabel> "FireProtectionSystem"@en .


###  http://w3id.org/emmo/domain/neo#RDGBzCkWozL4RpG1CuIzwPi
:RDGBzCkWozL4RpG1CuIzwPi rdf:type owl:Class ;
                         rdfs:subClassOf :R7pKuzitkkIAgc5NxDlqfH4 ,
                                         :RDpEA8qdRk99FAT0xSGZgGS ;
                         rdfs:isDefinedBy "ISO 21009-2:2015(en), 3.7" ;
                         <http://www.w3.org/2004/02/skos/core#definition> "escape of gas due to operating conditions, or to malfunctions that cannot be reasonably excluded"@en ;
                         <http://www.w3.org/2004/02/skos/core#prefLabel> "GasRelease"@en .


###  http://w3id.org/emmo/domain/neo#RDGsX7GTlCOL8Jlk3fXBK7U
:RDGsX7GTlCOL8Jlk3fXBK7U rdf:type owl:Class ;
                         rdfs:subClassOf elite:Role ,
                                         :R7qv2nUGxSNZRvXyF3CXPTr ,
                                         [ rdf:type owl:Restriction ;
                                           owl:onProperty elite:isOutputOf ;
                                           owl:someValuesFrom :R9ZCvqvWWCWSwBxX7K82iwL
                                         ] ;
                         rdfs:comment "Used in contexts where the radiation emitted by the radionuclide is the potential hazard."@en ;
                         rdfs:isDefinedBy "IAEA Safety Glossary, Terminology Used in Nuclear Safety and Radiation Protection, 2018 Edition "@en ;
                         <http://www.w3.org/2004/02/skos/core#definition> "A radionuclide produced by nuclear fission."@en ;
                         <http://www.w3.org/2004/02/skos/core#prefLabel> "FissionProduct"@en .


###  http://w3id.org/emmo/domain/neo#RDLYlpbjx3Rhwa0uGxFNWzC
:RDLYlpbjx3Rhwa0uGxFNWzC rdf:type owl:Class ;
                         rdfs:subClassOf :R7hYLnBucjQ8XgAj5RsQvpF ;
                         rdfs:comment "On the IAEA report is called \"Trasmission system\"."@en ;
                         rdfs:isDefinedBy "ISO 52000-1:2017(en) Energy performance of buildings — Overarching EPB assessment — Part 1: General framework and procedures ﻿."@en ;
                         <http://www.w3.org/2004/02/skos/core#definition> "Public electricity network .﻿"@en ;
                         <http://www.w3.org/2004/02/skos/core#prefLabel> "ElectricityGrid"@en .


###  http://w3id.org/emmo/domain/neo#RDM3Wmp5f6fMXTDpEK3Dmsx
:RDM3Wmp5f6fMXTDpEK3Dmsx rdf:type owl:Class ;
                         rdfs:subClassOf :R7gZLWyPCimwGhHTueSRPhd ,
                                         :RBsAUchYFBwAtcVUeFr8EFq ,
                                         :RDoeQzvUClmOY7fNhDvK0L1 ,
                                         [ rdf:type owl:Restriction ;
                                           owl:onProperty :RB4rNlczhggIx7lqdEK2d9c ;
                                           owl:someValuesFrom :R0ZnwwPdidaBfZOg6tgZJr
                                         ] ;
                         rdfs:comment "On the IAEA report is called \"safety relief valve (SRV)\"."@en ;
                         rdfs:isDefinedBy "ISO 21843:2023(en) Determination of the resistance to hydrocarbon pool fires of fire protection materials and systems for pressure vessels " ;
                         <http://www.w3.org/2004/02/skos/core#altLabel> "PRV"@en ,
                                                                        "ReactorPressureReliefValve"@en ;
                         <http://www.w3.org/2004/02/skos/core#definition> """pressure-activated valve intended to limit pressure rise to a specified value
Note 1 to entry: These valves have set opening and reclosing pressures"""@en ;
                         <http://www.w3.org/2004/02/skos/core#prefLabel> "PressureReliefValve"@en .


###  http://w3id.org/emmo/domain/neo#RDN44xs0tgwZS1p11BPMMKr
:RDN44xs0tgwZS1p11BPMMKr rdf:type owl:Class ;
                         rdfs:subClassOf :RBBzyqSEv3bIRXZvqAVCF4x ,
                                         [ rdf:type owl:Restriction ;
                                           owl:onProperty elite:isBehaviourOf ;
                                           owl:someValuesFrom :RCh38CRTgX4tnzCoB8auwPC
                                         ] ;
                         rdfs:isDefinedBy <https://www.nrc.gov/reading-rm/doc-collections/cfr/part050/part050-0063.html> ;
                         <http://www.w3.org/2004/02/skos/core#altLabel> "LossOfEmergencyACPower"@en ;
                         <http://www.w3.org/2004/02/skos/core#definition> "Loss of the AC electricity supplied by the devices entered in functions after the LossOfOffsitePower"@en ;
                         <http://www.w3.org/2004/02/skos/core#prefLabel> "LossOfAllACPower"@en .


###  http://w3id.org/emmo/domain/neo#RDNjoQuhLLxChWFzUtzeUrj
:RDNjoQuhLLxChWFzUtzeUrj rdf:type owl:Class ;
                         rdfs:subClassOf :RDoeQzvUClmOY7fNhDvK0L1 ,
                                         [ rdf:type owl:Restriction ;
                                           owl:onProperty elite:isConstituentOf ;
                                           owl:someValuesFrom :R85FFwLPHIursWfa6K6sKK9
                                         ] ;
                         :R8xx0dhbEh1tjGMDwNZfckV "chamber, below ground level in a pumping installation that receives water to be pumped "@en ;
                         rdfs:isDefinedBy "ISO 6107:2021(en) Water quality — Vocabulary " ;
                         <http://www.w3.org/2004/02/skos/core#altLabel> "ReactorWetWell"@en ;
                         <http://www.w3.org/2004/02/skos/core#prefLabel> "WetWell"@en .


###  http://w3id.org/emmo/domain/neo#RDP6jdP3MdBK59hhoDGY0Vw
:RDP6jdP3MdBK59hhoDGY0Vw rdf:type owl:Class ;
                         rdfs:subClassOf elite:Process ;
                         <http://www.w3.org/2004/02/skos/core#definition> "A thing that happens or takes place, with a well defined beginning and end, a clear specificity and relevance with respect to the surrounding environment."@en ;
                         <http://www.w3.org/2004/02/skos/core#prefLabel> "Event"@en .


###  http://w3id.org/emmo/domain/neo#RDS0g8UekSMDWjEgBp6z2sP
:RDS0g8UekSMDWjEgBp6z2sP rdf:type owl:Class ;
                         rdfs:subClassOf elite:Role ,
                                         :RBfqFRty5Hp4V4caVtEvWdD ,
                                         [ rdf:type owl:Restriction ;
                                           owl:onProperty elite:isOutputOf ;
                                           owl:someValuesFrom :R9ZCvqvWWCWSwBxX7K82iwL
                                         ] ;
                         :RR3uD2d7YfhHohfv2Nm6sX """Fast neutrons are considered as such in the context of a fission nuclear reactor, where the average neutron energy emerging from fission is about 2 MeV, before being slowed down by collisions. 
While in some textbooks you can find a defnition of fast neutron as a neutron with E > 50 keV, there is not a clear definition of the range within which a neutron can be considered \"fast\"."""@en ;
                         rdfs:isDefinedBy <https://www.iso.org/obp/ui/en/#iso:std:iso:12749:-5:ed-1:v1:en:term:3.1.5.1> ;
                         <http://www.w3.org/2004/02/skos/core#definition> "A neutron with kinetic energy greater than its surroundings when released during fission."@en ;
                         <http://www.w3.org/2004/02/skos/core#prefLabel> "FastNeutron"@en .


###  http://w3id.org/emmo/domain/neo#RDT2hV6YibqdGN2HMXay4hK
:RDT2hV6YibqdGN2HMXay4hK rdf:type owl:Class ;
                         rdfs:subClassOf :R9ZCvqvWWCWSwBxX7K82iwL ;
                         rdfs:isDefinedBy <https://www.iso.org/obp/ui/en/#iso:std:iso:12749:-5:ed-1:v1:en:term:3.1.1.2> ;
                         <http://www.w3.org/2004/02/skos/core#definition> "nuclear fission (3.1.1) produced in a nucleus, having an inherent instability, that develops itself in a purely stochastic way and without intervention of any external colliding particle"@en ;
                         <http://www.w3.org/2004/02/skos/core#prefLabel> "SpontaneousNuclearFission"@en .


###  http://w3id.org/emmo/domain/neo#RDTfhSry7c6TzIENETvIs1U
:RDTfhSry7c6TzIENETvIs1U rdf:type owl:Class ;
                         rdfs:subClassOf :RDoeQzvUClmOY7fNhDvK0L1 ,
                                         [ rdf:type owl:Restriction ;
                                           owl:onProperty elite:isConstituentOf ;
                                           owl:someValuesFrom :R7KAfaev0soZNlAXHICHSJd
                                         ] ,
                                         [ rdf:type owl:Restriction ;
                                           owl:onProperty elite:partakesIn ;
                                           owl:someValuesFrom :RyMmVkVf9zClluOSgfr1Rh
                                         ] ,
                                         [ rdf:type owl:Restriction ;
                                           owl:onProperty elite:participatesTo ;
                                           owl:someValuesFrom :R1DAH32q3UDTp3GZGqe5Re
                                         ] ,
                                         [ rdf:type owl:Restriction ;
                                           owl:onProperty elite:participatesTo ;
                                           owl:someValuesFrom :R80L6MpJJVkL4hoNB7thCRV
                                         ] ,
                                         [ rdf:type owl:Restriction ;
                                           owl:onProperty elite:participatesTo ;
                                           owl:someValuesFrom :R9aF6fIPWPEzkHdmnDKNorP
                                         ] ;
                         rdfs:isDefinedBy <https://aris.iaea.org/sites/Glossary.html> ;
                         <http://www.w3.org/2004/02/skos/core#altLabel> "CR"@en ;
                         <http://www.w3.org/2004/02/skos/core#definition> "A rode/plate/tube that is used to absorb the neutrons in the reactor core. These help to control the number of fission events and thus the power of the nuclear reactor. "@en ;
                         <http://www.w3.org/2004/02/skos/core#prefLabel> "ControlRod"@en .


###  http://w3id.org/emmo/domain/neo#RDTtg7PlU70nX1AN6XHiAwK
:RDTtg7PlU70nX1AN6XHiAwK rdf:type owl:Class ;
                         rdfs:subClassOf :R89Yy2V18LstH4xGXyNb9XN ,
                                         :RBsAUchYFBwAtcVUeFr8EFq ,
                                         [ rdf:type owl:Restriction ;
                                           owl:onProperty :RB4rNlczhggIx7lqdEK2d9c ;
                                           owl:someValuesFrom :R8CzBJHXymJx05c6sDhbspt
                                         ] ;
                         rdfs:isDefinedBy <https://inis.iaea.org/collection/NCLCollectionStore/_Public/27/051/27051618.pdf> ;
                         <http://www.w3.org/2004/02/skos/core#altLabel> "NuclearTurbineValve"@en ,
                                                                        "StopValve"@en ;
                         <http://www.w3.org/2004/02/skos/core#definition> "The main turbine is an 1800 rpm, tandem compound machine consisting of one high-pressure turbine and three lowpressure turbines. The steam enters the middle of the high-pressure section and works its way toward each end, dissipating its energy to the turbine blades which are attached to a common shaft. Steam exiting the high-pressure turbine passes through moisture separators where entrained moisture, which could damage the turbine blades, is removed prior to entering the low-pressure turbine (BWR description)"@en ;
                         <http://www.w3.org/2004/02/skos/core#prefLabel> "TurbineValve"@en .


###  http://w3id.org/emmo/domain/neo#RDZtzLsQmngV2BtJvmS5pbg
:RDZtzLsQmngV2BtJvmS5pbg rdf:type owl:Class ;
                         rdfs:subClassOf elite:Object ,
                                         elite:Role ;
                         rdfs:isDefinedBy "IAEA Safety Glossary, Terminology Used in Nuclear Safety and Radiation Protection, 2018 Edition" ;
                         <http://www.w3.org/2004/02/skos/core#altLabel> "NppEmployes"@en ;
                         <http://www.w3.org/2004/02/skos/core#definition> "Any person who works, whether full time, part time or temporarily, for an employer and who has recognized rights and duties in relation to occupational radiation protection."@en ;
                         <http://www.w3.org/2004/02/skos/core#prefLabel> "NuclearPlantWorker"@en .


###  http://w3id.org/emmo/domain/neo#RDdFdbRqtigD5ry1nrSpxkb
:RDdFdbRqtigD5ry1nrSpxkb rdf:type owl:Class ;
                         rdfs:subClassOf :R7oHlh8OgEkyG3XXGpiYlC5 ;
                         rdfs:seeAlso <https://www-ns.iaea.org/downloads/standards/glossary/iaea-safety-glossary-draft-2016.pdf> ;
                         <http://www.w3.org/2004/02/skos/core#definition> "Loss of the ability of a component to function within acceptance criteria. The component is considered to fail when it becomes incapable of functioning, whether or not this is needed at that time."@en ;
                         <http://www.w3.org/2004/02/skos/core#prefLabel> "ComponentFailure"@en .


###  http://w3id.org/emmo/domain/neo#RDh3zL6vQwm8NRNsC9Eo3Sa
:RDh3zL6vQwm8NRNsC9Eo3Sa rdf:type owl:Class ;
                         rdfs:subClassOf :RDoeQzvUClmOY7fNhDvK0L1 ,
                                         [ rdf:type owl:Restriction ;
                                           owl:onProperty :RB4rNlczhggIx7lqdEK2d9c ;
                                           owl:someValuesFrom :RMiSxLtLOMDcYH1jWDJO1b
                                         ] ;
                         rdfs:comment "Spent fuel pools (SFP) are storage pools for spent fuel from nuclear reactors. They are typically 40 or more feet (12 m) deep, with the bottom 14 feet (4.3 m) equipped with storage racks designed to hold fuel assemblies removed from reactors. A reactor's local pool is specially designed for the reactor in which the fuel was used and is situated at the reactor site. Such pools are used for short-term cooling of the fuel rods. This allows short-lived isotopes to decay and thus reduces the ionizing radiation and decay heat emanating from the rods. The water cools the fuel and provides radiological protection from its radiation."@en ;
                         rdfs:isDefinedBy <https://en.wikipedia.org/wiki/Spent_fuel_pool> ;
                         <http://www.w3.org/2004/02/skos/core#altLabel> "SFP"@en ;
                         <http://www.w3.org/2004/02/skos/core#prefLabel> "SpentFuelPool"@en .


###  http://w3id.org/emmo/domain/neo#RDi09Rm801Kr3SGc3oyRzVc
:RDi09Rm801Kr3SGc3oyRzVc rdf:type owl:Class ;
                         rdfs:subClassOf :RdPoUW04SB1jvKPJcXoVCW ,
                                         [ rdf:type owl:Restriction ;
                                           owl:onProperty elite:isSubProcessOf ;
                                           owl:someValuesFrom :RDi09Rm801Kr3SGc3oyRzVc
                                         ] ;
                         rdfs:isDefinedBy <https://www.eionet.europa.eu/gemet/en/concept/1799> ;
                         <http://www.w3.org/2004/02/skos/core#altLabel> "NuclearMeltdown"@en ,
                                                                        "PartialCoreMeltdown"@en ;
                         <http://www.w3.org/2004/02/skos/core#definition> "An accidental overheating of the part of the nuclear reactor where fission takes place, causing fuel elements and other parts of the reactor to melt, potentially leading to catastrophic consequences in which dangerous levels of radioactive materials would be released into the environment."@en ;
                         <http://www.w3.org/2004/02/skos/core#prefLabel> "CoreMeltdown"@en .


###  http://w3id.org/emmo/domain/neo#RDoeQzvUClmOY7fNhDvK0L1
:RDoeQzvUClmOY7fNhDvK0L1 rdf:type owl:Class ;
                         rdfs:subClassOf elite:Object ,
                                         [ rdf:type owl:Restriction ;
                                           owl:onProperty elite:isConstituentOf ;
                                           owl:someValuesFrom :R0N27qMQzeRjM0vSOeAvUT
                                         ] ,
                                         [ rdf:type owl:Restriction ;
                                           owl:onProperty :RB4rNlczhggIx7lqdEK2d9c ;
                                           owl:someValuesFrom :R0ZnwwPdidaBfZOg6tgZJr
                                         ] ;
                         rdfs:seeAlso <https://www.iso.org/obp/ui/en/#iso:std:iso:24679:-1:ed-1:v1:en:term:3.1> ;
                         <http://www.w3.org/2004/02/skos/core#comment> """They are distinguished from elements as integral part of a built environment
Note 1 to entry: This includes floors, walls, beams, columns, doors, and penetrations, but does not include contents."""@en ;
                         <http://www.w3.org/2004/02/skos/core#definition> "Elements that are contained in a Reactor Building"@en ;
                         <http://www.w3.org/2004/02/skos/core#prefLabel> "ReactorBuildingContents"@en .


###  http://w3id.org/emmo/domain/neo#RDpEA8qdRk99FAT0xSGZgGS
:RDpEA8qdRk99FAT0xSGZgGS rdf:type owl:Class ;
                         rdfs:subClassOf :RtdecAtZ9C9xUJNtjefY4D ,
                                         [ rdf:type owl:Restriction ;
                                           owl:onProperty elite:isConstitutiveProcessOf ;
                                           owl:someValuesFrom :R0N27qMQzeRjM0vSOeAvUT
                                         ] ;
                         :RR3uD2d7YfhHohfv2Nm6sX "No off-site radiological impact (bounded by regulatory operating limits for discharge)"@en ;
                         rdfs:comment "Level 1 of Defense in depth: Plant control under normal conditions"@en ,
                                      "StandardOperatingProcedures (SOP)"@en ,
                                      """The prevention of system failures and deviations from normal operations. This is a continuous and largely
repetitive process. The algorithms used are very different from those of protection functions, and experience
with the system functionality may be gained in every clock cycle. Also, the potential development of
undetected failures can be lower."""@en ,
                                      "there are not failures in the plant"@en ;
                         rdfs:isDefinedBy <https://www-ns.iaea.org/downloads/standards/glossary/iaea-safety-glossary-draft-2016.pdf> ;
                         rdfs:seeAlso "INTERNATIONAL ATOMIC ENERGY AGENCY, Approaches for Overall Instrumentation and Control Architectures of Nuclear Power Plants, IAEA Nuclear Energy Series No. NP-T-2.11, IAEA, Vienna (2018)" ;
                         <http://www.w3.org/2004/02/skos/core#altLabel> "NPPPreventiveOperation"@en ;
                         <http://www.w3.org/2004/02/skos/core#definition> "Operation within specified operational limits and conditions. This includes startup, power operation, shutting down, shutdown, maintenance, testing and refuelling"@en ;
                         <http://www.w3.org/2004/02/skos/core#prefLabel> "NPPNormalOperation"@en .


###  http://w3id.org/emmo/domain/neo#RDqGoUzaBPNiIDtLS6qlo3t
:RDqGoUzaBPNiIDtLS6qlo3t rdf:type owl:Class ;
                         rdfs:subClassOf :R80RaxHVqr4QPiv8ASxXxi3 ;
                         rdfs:isDefinedBy "INTERNATIONAL ATOMIC ENERGY AGENCY, Approaches for Overall Instrumentation and Control Architectures of Nuclear Power Plants, IAEA Nuclear Energy Series No. NP-T-2.11, IAEA, Vienna (2018) p.12" ;
                         <http://www.w3.org/2004/02/skos/core#altLabel> "Level2DiD" ;
                         <http://www.w3.org/2004/02/skos/core#definition> """Control of deviations from normal operating states to prevent anticipated operational occurrences from
escalating to accident conditions. This can be provided both by electronic means and by operator intervention,
if there is enough time and information for such actions to be credited. The algorithms used are different
from control."""@en ;
                         <http://www.w3.org/2004/02/skos/core#prefLabel> "ControlOfDeviations"@en .


###  http://w3id.org/emmo/domain/neo#RDqxw9842TBP5U24ILrY1bb
:RDqxw9842TBP5U24ILrY1bb rdf:type owl:Class ;
                         rdfs:subClassOf :RDpEA8qdRk99FAT0xSGZgGS ;
                         rdfs:comment "onsite replacement power facilities"@en ,
                                      "replacement of the damaged hoses"@en ;
                         rdfs:isDefinedBy <https://dictionary.cambridge.org/dictionary/english/replace> ;
                         <http://www.w3.org/2004/02/skos/core#definition> "To take the place of something, or to put something or someone in the place of something or someone else.If you replace something broken, damaged, or lost, you provide a new one."@en ;
                         <http://www.w3.org/2004/02/skos/core#prefLabel> "Replacement"@en .


###  http://w3id.org/emmo/domain/neo#RDuDSbKh236WI6rqMad7Ar4
:RDuDSbKh236WI6rqMad7Ar4 rdf:type owl:Class ;
                         rdfs:subClassOf :RlYMwSSvmqekLRLzmf5IzV ,
                                         [ rdf:type owl:Restriction ;
                                           owl:onProperty elite:isBehaviourOf ;
                                           owl:someValuesFrom :R7NYEyrtAsNuF6n0QNOFmHm
                                         ] ,
                                         [ rdf:type owl:Restriction ;
                                           owl:onProperty elite:isBehaviourOf ;
                                           owl:someValuesFrom :R7Ss5qBF98KBgXN3rhg0rEl
                                         ] ,
                                         [ rdf:type owl:Restriction ;
                                           owl:onProperty elite:isBehaviourOf ;
                                           owl:someValuesFrom :R7hYLnBucjQ8XgAj5RsQvpF
                                         ] ,
                                         [ rdf:type owl:Restriction ;
                                           owl:onProperty elite:isBehaviourOf ;
                                           owl:someValuesFrom :RBp2yVTrXRyb55JnYdvAGux
                                         ] ,
                                         [ rdf:type owl:Restriction ;
                                           owl:onProperty elite:isBehaviourOf ;
                                           owl:someValuesFrom :RBsAUchYFBwAtcVUeFr8EFq
                                         ] ,
                                         [ rdf:type owl:Restriction ;
                                           owl:onProperty elite:isBehaviourOf ;
                                           owl:someValuesFrom :RBzruvoEUI9hIHVtX34kGJu
                                         ] ,
                                         [ rdf:type owl:Restriction ;
                                           owl:onProperty elite:isBehaviourOf ;
                                           owl:someValuesFrom :RCDLrZ9KyXAspBK0GpRfHxG
                                         ] ,
                                         [ rdf:type owl:Restriction ;
                                           owl:onProperty elite:isBehaviourOf ;
                                           owl:someValuesFrom :RCh38CRTgX4tnzCoB8auwPC
                                         ] ;
                         rdfs:isDefinedBy <https://www.collinsdictionary.com/dictionary/english/start> ,
                                          <https://www.iso.org/obp/ui/en/#iso:std:iso-iec:tr:11580:ed-1:v1:en:term:2.12> ;
                         <http://www.w3.org/2004/02/skos/core#altLabel> "Starting"@en ;
                         <http://www.w3.org/2004/02/skos/core#definition> "initiation of a selected function of an object"@en ,
                                                                          "it takes place from a particular time"@en ;
                         <http://www.w3.org/2004/02/skos/core#prefLabel> "Activation"@en .


###  http://w3id.org/emmo/domain/neo#RDv6FAzzuS81VzIfTO1Wkef
:RDv6FAzzuS81VzIfTO1Wkef rdf:type owl:Class ;
                         rdfs:subClassOf elite:Object ,
                                         [ rdf:type owl:Restriction ;
                                           owl:onProperty :RB4rNlczhggIx7lqdEK2d9c ;
                                           owl:someValuesFrom :R0N27qMQzeRjM0vSOeAvUT
                                         ] ;
                         rdfs:comment "Dry cask storage is a method of storing high-level radioactive waste, such as spent nuclear fuel that has already been cooled in the spent fuel pool for at least one year and often as much as ten years. Casks are typically steel cylinders that are either welded or bolted closed. The fuel rods inside are surrounded by inert gas. Ideally, the steel cylinder provides leak-tight containment of the spent fuel. Each cylinder is surrounded by additional steel, concrete, or other material to provide radiation shielding to workers and members of the public."@en ;
                         rdfs:isDefinedBy <https://en.wikipedia.org/wiki/Dry_cask_storage> ;
                         <http://www.w3.org/2004/02/skos/core#definition> "It is a building used for dry cask storage."@en ;
                         <http://www.w3.org/2004/02/skos/core#prefLabel> "DryCaskStorageBuilding"@en .


###  http://w3id.org/emmo/domain/neo#REnnyld9FmnAjLpeDyUsnv
:REnnyld9FmnAjLpeDyUsnv rdf:type owl:Class ;
                        rdfs:subClassOf :RBW32C4x3sn1YahVG7uYVun ,
                                        [ rdf:type owl:Restriction ;
                                          owl:onProperty elite:isConstituentOf ;
                                          owl:someValuesFrom :R0N27qMQzeRjM0vSOeAvUT
                                        ] ;
                        rdfs:isDefinedBy <https://www.iso.org/obp/ui/en/#iso:std:iso:12749:-5:ed-1:v1:en:term:3.2.4.2> ;
                        <http://www.w3.org/2004/02/skos/core#definition> "thermal nuclear reactor (3.1.22) cooled and moderated by light water" ;
                        <http://www.w3.org/2004/02/skos/core#prefLabel> "LightWaterReactor"@en .


###  http://w3id.org/emmo/domain/neo#REwjatmwMA4xgNq0mpx6LO
:REwjatmwMA4xgNq0mpx6LO rdf:type owl:Class ;
                        rdfs:subClassOf :R89Yy2V18LstH4xGXyNb9XN ,
                                        [ rdf:type owl:Restriction ;
                                          owl:onProperty elite:isConstituentOf ;
                                          owl:someValuesFrom :RvBQlxDEMRtFxiHtMstrYY
                                        ] ;
                        <http://www.w3.org/2004/02/skos/core#altLabel> "NppSeaWaterPump"@en ;
                        <http://www.w3.org/2004/02/skos/core#prefLabel> "SeaWaterPump"@en .


###  http://w3id.org/emmo/domain/neo#RG2TvkBghAiQkHQc4GNU8e
:RG2TvkBghAiQkHQc4GNU8e rdf:type owl:Class ;
                        rdfs:subClassOf :R7gZLWyPCimwGhHTueSRPhd ,
                                        :RBsAUchYFBwAtcVUeFr8EFq ,
                                        :RDoeQzvUClmOY7fNhDvK0L1 ,
                                        [ rdf:type owl:Restriction ;
                                          owl:onProperty elite:isConstituentOf ;
                                          owl:someValuesFrom :RCRVu2hmIevYnx0eZzyJEPs
                                        ] ;
                        rdfs:comment "For depressurizing the reactor, the on-site ERC and the MRC staff decided to use the nitrogen operated head vent nozzle (a small valve at top of the RPV) as an alternative method to depressurize the reactor because DC power was available from the 250 V emergency batteries for this purpose."@en ;
                        rdfs:seeAlso """Pag 124, The Fukushima Daiichi Accident Technical Volume 1/5 
link: https://www-pub.iaea.org/MTCD/Publications/PDF/AdditionalVolumes/P1710/Pub1710-TV1-Web.pdf""" ;
                        <http://www.w3.org/2004/02/skos/core#altLabel> "HeadVentValve"@en ;
                        <http://www.w3.org/2004/02/skos/core#definition> "It is a valve on the Reactor Pressure Vessel﻿"@en ;
                        <http://www.w3.org/2004/02/skos/core#prefLabel> "HeadVentNozzle"@en .


###  http://w3id.org/emmo/domain/neo#RG42cv992jX3Deeh35WKwu
:RG42cv992jX3Deeh35WKwu rdf:type owl:Class ;
                        rdfs:subClassOf :RLEjSGGgoWOVMGjQsskCsb ;
                        rdfs:isDefinedBy """ISO 24513:2019(en)
Service activities relating to drinking water supply, wastewater and stormwater systems — Vocabulary""" ;
                        <http://www.w3.org/2004/02/skos/core#definition> "Condition where water flows onto a surface or enters a structure or area where it is not intended."@en ;
                        <http://www.w3.org/2004/02/skos/core#prefLabel> "PlantFloodingAccident"@en .


###  http://w3id.org/emmo/domain/neo#RGNf2JfOQS4CiKraFgzrIc
:RGNf2JfOQS4CiKraFgzrIc rdf:type owl:Class ;
                        rdfs:subClassOf :RRcoLavbFREtzVcprEzyrY ;
                        rdfs:isDefinedBy <https://en.wikipedia.org/wiki/Rupture_disc> ;
                        <http://www.w3.org/2004/02/skos/core#definition> "Destruction of the pressure safety disk that starts a unstoppable pressure relief"@en ;
                        <http://www.w3.org/2004/02/skos/core#prefLabel> "BurstOfRuptureDisc"@en .


###  http://w3id.org/emmo/domain/neo#RHQniV2VTxSsHQobdf4d6d
:RHQniV2VTxSsHQobdf4d6d rdf:type owl:Class ;
                        rdfs:subClassOf :RBBzyqSEv3bIRXZvqAVCF4x ,
                                        [ rdf:type owl:Restriction ;
                                          owl:onProperty elite:isBehaviourOf ;
                                          owl:someValuesFrom :RDLYlpbjx3Rhwa0uGxFNWzC
                                        ] ;
                        rdfs:isDefinedBy <https://www-pub.iaea.org/MTCD/Publications/PDF/TE-1770_web.pdf> ;
                        <http://www.w3.org/2004/02/skos/core#altLabel> "Blackout"@en ,
                                                                       "LOOP"@en ;
                        <http://www.w3.org/2004/02/skos/core#definition> "Design basis in which the supply of AC electricity coming from the preferred power supply is interrupted. By design this cause the starting of the EDG (emergency diesel generator) to restore AC power to the emergency services and to the DC (direct current) power batteries chargers"@en ;
                        <http://www.w3.org/2004/02/skos/core#prefLabel> "LossOfOffSitePower"@en .


###  http://w3id.org/emmo/domain/neo#RJmt9cNm88D71RlMOkJ6WM
:RJmt9cNm88D71RlMOkJ6WM rdf:type owl:Class ;
                        rdfs:subClassOf :R7QpMP9Mf1mRrRVeMT7UcIX ;
                        rdfs:isDefinedBy """https://aris.iaea.org/sites/Glossary.html 
Glossary of Terms in ARIS Reports""" ;
                        <http://www.w3.org/2004/02/skos/core#definition> "A substance that is used to remove or transfer heat from the reactor core. Common coolants include light water, heavy water, air, carbon dioxide, helium, liquid sodium, and a sodium-potassium alloy."@en ;
                        <http://www.w3.org/2004/02/skos/core#prefLabel> "ReactorCoolant"@en .


###  http://w3id.org/emmo/domain/neo#RLEjSGGgoWOVMGjQsskCsb
:RLEjSGGgoWOVMGjQsskCsb rdf:type owl:Class ;
                        rdfs:subClassOf :R7pKuzitkkIAgc5NxDlqfH4 ,
                                        [ rdf:type owl:Restriction ;
                                          owl:onProperty elite:hasNext ;
                                          owl:someValuesFrom :R9TI5UbsBXnAYSIi17pJARr
                                        ] ;
                        :RR3uD2d7YfhHohfv2Nm6sX "Possiamo dire che un unintened event è un evento le cui conseguenze possono mettere a rischio le condizioni operative del reattore fino a portare ad un danneggiamento"@it ;
                        rdfs:comment """An unintended event is any occurrence unintended
by the operator, including operating error, equipment failure or other mishap, and deliberate
action on the part of others, the consequences or potential consequences of which are not
negligible from the point of view of protection and safety"""@en ;
                        rdfs:seeAlso <https://www-ns.iaea.org/downloads/standards/glossary/iaea-safety-glossary-draft-2016.pdf> ;
                        <http://www.w3.org/2004/02/skos/core#definition> """Is any occurrence that can lead to potential consequences that are not
negligible from the point of view of protection and safety of a Nuclear power plant"""@en ;
                        <http://www.w3.org/2004/02/skos/core#prefLabel> "NPPUnintendedEvent"@en .


###  http://w3id.org/emmo/domain/neo#RMiSxLtLOMDcYH1jWDJO1b
:RMiSxLtLOMDcYH1jWDJO1b rdf:type owl:Class ;
                        rdfs:subClassOf :R8hTHDGsCdkEbILOuzUhlEr ;
                        rdfs:isDefinedBy "IAEA Safety Glossary, Terminology Used in Nuclear Safety and Radiation Protection, 2018 Edition﻿" ;
                        <http://www.w3.org/2004/02/skos/core#altLabel> "SpentFuelManagementFacility"@en ;
                        <http://www.w3.org/2004/02/skos/core#prefLabel> "CommonSpentFuelBuilding"@en .


###  http://w3id.org/emmo/domain/neo#RNNqkJui2M9zYKvBkz3iQ
:RNNqkJui2M9zYKvBkz3iQ rdf:type owl:Class ;
                       rdfs:subClassOf :RDoeQzvUClmOY7fNhDvK0L1 ,
                                       [ rdf:type owl:Restriction ;
                                         owl:onProperty elite:isConstituentOf ;
                                         owl:someValuesFrom :RCzybo2ACvDW8XnRRQcoQTg
                                       ] ;
                       rdfs:comment "Commonly referred to as a fuel rod in light water reactors."@en ;
                       rdfs:isDefinedBy """IAEA Safety Glossary, Terminology Used in Nuclear Safety 
and Radiation Protection, 2018 Edition """ ;
                       <http://www.w3.org/2004/02/skos/core#altLabel> "FuelRod"@en ;
                       <http://www.w3.org/2004/02/skos/core#definition> "A rod of nuclear fuel, its cladding and any associated components necessary to form a structural entity.﻿"@en ;
                       <http://www.w3.org/2004/02/skos/core#prefLabel> "FuelElement"@en .


###  http://w3id.org/emmo/domain/neo#RPURhpVoxOOYoC2J28Rgfd
:RPURhpVoxOOYoC2J28Rgfd rdf:type owl:Class ;
                        rdfs:subClassOf :R9PjB5mvpVfreaI0pbTQFj6 ,
                                        :RtX7ESf673Z9eYoseycPyl ;
                        rdfs:isDefinedBy """IAEA Safety Glossary, Terminology Used in Nuclear Safety 
and Radiation Protection, 2018 Edition """ ;
                        <http://www.w3.org/2004/02/skos/core#definition> """Fissionable nuclear material in the form of fabricated elements for loading
into the reactor core of a civil nuclear power plant or research reactor."""@en ;
                        <http://www.w3.org/2004/02/skos/core#prefLabel> "﻿NuclearFuel"@en .


###  http://w3id.org/emmo/domain/neo#RRKk7nTYd2pj3LFUG4j9yj
:RRKk7nTYd2pj3LFUG4j9yj rdf:type owl:Class ;
                        rdfs:subClassOf elite:Object ,
                                        [ rdf:type owl:Restriction ;
                                          owl:onProperty elite:isConstituentOf ;
                                          owl:someValuesFrom :R0N27qMQzeRjM0vSOeAvUT
                                        ] ;
                        rdfs:comment "The NPP unit includes the nuclear reactor plus all its associated systems and buildings not shared by other nuclear reactors (ISO 12749-5:2018)"@en ;
                        rdfs:isDefinedBy <https://www.iso.org/obp/ui/#iso:std:iso:12749:-5:ed-1:v1:en:term:3.4.3> ,
                                         "IAEA “Construction technologies for nuclear power plants”. IAEA Nuclear Energy Series No. NP-T-2.5. IAEA, Vienna, 2011. p. 190" ;
                        <http://www.w3.org/2004/02/skos/core#altLabel> "NPPUnit"@en ;
                        <http://www.w3.org/2004/02/skos/core#definition> "part of the NPP implementing NPP´s functions with the scope specified in the NPP´s design basis (ISO 12749-5:2018)"@en ;
                        <http://www.w3.org/2004/02/skos/core#prefLabel> "NuclearPowerPlantUnit"@en .


###  http://w3id.org/emmo/domain/neo#RRPYBSdeHQObrzQD5UT74I
:RRPYBSdeHQObrzQD5UT74I rdf:type owl:Class ;
                        rdfs:subClassOf :R8MPIXNWSb8RCelrAeGNxMc ;
                        rdfs:isDefinedBy <https://www.iso.org/obp/ui/en/#iso:std:iso:7967:-11:ed-2:v1:en:term:3.3.69> ;
                        <http://www.w3.org/2004/02/skos/core#definition> "abnormal cyclic change of injection fuel flow during constant fuel operation"@en ;
                        <http://www.w3.org/2004/02/skos/core#prefLabel> "IrregularInjection"@en .


###  http://w3id.org/emmo/domain/neo#RRVTDj2E9x5cjit7EQ9Dkx
:RRVTDj2E9x5cjit7EQ9Dkx rdf:type owl:Class ;
                        rdfs:subClassOf :R7hYLnBucjQ8XgAj5RsQvpF ,
                                        [ rdf:type owl:Restriction ;
                                          owl:onProperty :RB4rNlczhggIx7lqdEK2d9c ;
                                          owl:someValuesFrom :R0N27qMQzeRjM0vSOeAvUT
                                        ] ;
                        rdfs:comment "On the IAEA report is called \"DC Power system\".﻿"@en ;
                        rdfs:isDefinedBy "IWA 33-1:2019(en) Technical guidelines for the development of small hydropower plants — Part 1: Vocabulary ﻿" ;
                        <http://www.w3.org/2004/02/skos/core#altLabel> "DCPowerSystem﻿"@en ;
                        <http://www.w3.org/2004/02/skos/core#definition> "DC power source supplying power to control, signal and automatic devices, as well as relay protection, tripping and closing coils of switching devices and emergency lighting﻿."@en ;
                        <http://www.w3.org/2004/02/skos/core#prefLabel> "DCOperationalPowerSource"@en .


###  http://w3id.org/emmo/domain/neo#RRcoLavbFREtzVcprEzyrY
:RRcoLavbFREtzVcprEzyrY rdf:type owl:Class ;
                        rdfs:subClassOf :R7s6BZ18NYlgydAQozd7POd ;
                        rdfs:isDefinedBy <https://www.britannica.com/dictionary/destruction> ;
                        <http://www.w3.org/2004/02/skos/core#definition> "The act or process of damaging something so badly that it no longer exists or cannot be repaired."@en ;
                        <http://www.w3.org/2004/02/skos/core#prefLabel> "Destruction"@en .


###  http://w3id.org/emmo/domain/neo#RRxSYO9r2FD1rHmRPugfob
:RRxSYO9r2FD1rHmRPugfob rdf:type owl:Class ;
                        rdfs:subClassOf :R9TI5UbsBXnAYSIi17pJARr ,
                                        [ rdf:type owl:Restriction ;
                                          owl:onProperty elite:hasNext ;
                                          owl:someValuesFrom :RC9Vnqc96TS4VVdygnxu8UP
                                        ] ;
                        rdfs:isDefinedBy <https://www.nrc.gov/docs/ML2031/ML20318A171.pdf> ;
                        <http://www.w3.org/2004/02/skos/core#definition> """A PIE Is an event identified in the
design that leads to Anticipated Operational Occurrences (AOOs) or accident conditions. Accident
conditions include Design Basis Accidents (DBAs) and Beyond Design Basis Accidents (BDBAs). BDBAs
include a subset of severe accidents."""@en ;
                        <http://www.w3.org/2004/02/skos/core#prefLabel> "PostulatedInitiatingEvent"@en .


###  http://w3id.org/emmo/domain/neo#RSvx83QCmkRfOzQUtOkIeS
:RSvx83QCmkRfOzQUtOkIeS rdf:type owl:Class ;
                        rdfs:subClassOf :R7fkBdyMeKQvQzm3yRgM2iz ;
                        rdfs:isDefinedBy """ISO/TS 22330:2018(en)
Security and resilience — Business continuity management systems — Guidelines for people aspects of business continuity""" ;
                        <http://www.w3.org/2004/02/skos/core#definition> "Action to move people to predetermined areas inside the building/site in order to protect them from external dangers during an incident."@en ;
                        <http://www.w3.org/2004/02/skos/core#prefLabel> "ShelterInPlace"@en .


###  http://w3id.org/emmo/domain/neo#RTywWKZwkjxu5ChUU9jvyq
:RTywWKZwkjxu5ChUU9jvyq rdf:type owl:Class ;
                        rdfs:subClassOf :RDpEA8qdRk99FAT0xSGZgGS ,
                                        [ rdf:type owl:Restriction ;
                                          owl:onProperty elite:isBehaviourOf ;
                                          owl:someValuesFrom :RPURhpVoxOOYoC2J28Rgfd
                                        ] ;
                        rdfs:isDefinedBy <https://www.nrc.gov/reading-rm/basic-ref/glossary/refueling.html> ;
                        <http://www.w3.org/2004/02/skos/core#definition> "The process of removing older fuel and loading new fuel. These actions are all performed underwater to supply continuous cooling for the fuel and provide shielding from the radioactive spent fuel."@en ;
                        <http://www.w3.org/2004/02/skos/core#prefLabel> "NPPRefueling"@en .


###  http://w3id.org/emmo/domain/neo#RUfmPQytgoT4sAaWFKoKAG
:RUfmPQytgoT4sAaWFKoKAG rdf:type owl:Class ;
                        rdfs:subClassOf :R7fkBdyMeKQvQzm3yRgM2iz ;
                        rdfs:isDefinedBy """ISO/TR 24188:2022(en)
Large outdoor fires and the built environment — Global overview of different approaches to standardization""" ;
                        <http://www.w3.org/2004/02/skos/core#definition> "Dispersal or removal of people from dangerous areas and their arrival at a place of relative safety."@en ;
                        <http://www.w3.org/2004/02/skos/core#prefLabel> "Evacuation"@en .


###  http://w3id.org/emmo/domain/neo#RY81DSQhpDKzGrzvuAjU5m
:RY81DSQhpDKzGrzvuAjU5m rdf:type owl:Class ;
                        rdfs:subClassOf :RDoeQzvUClmOY7fNhDvK0L1 ,
                                        :Rw4mCgviqd6HTitZEzST6w ,
                                        [ rdf:type owl:Restriction ;
                                          owl:onProperty :RB4rNlczhggIx7lqdEK2d9c ;
                                          owl:someValuesFrom :R85FFwLPHIursWfa6K6sKK9
                                        ] ;
                        rdfs:isDefinedBy <https://www.nrc.gov/docs/ML1215/ML12159A162.pdf> ;
                        <http://www.w3.org/2004/02/skos/core#altLabel> "ReactorSuppressionChamber"@en ,
                                                                       "SC"@en ;
                        <http://www.w3.org/2004/02/skos/core#definition> "The suppression chamber consists of a steel pressure vessel with a toroidal shape (sometimes referred to as torus) and a large body of water inside the suppression chamber (referred to as the suppression pool). The purposes of the suppression chamber are to condense steam released from a LOCA and to prevent radioactive materials from passing through this portion of the primary containment boundary.  ﻿"@en ;
                        <http://www.w3.org/2004/02/skos/core#prefLabel> "SuppressionChamber"@en .


###  http://w3id.org/emmo/domain/neo#RZ7eQ19CTPh8iKBmvqWp16
:RZ7eQ19CTPh8iKBmvqWp16 rdf:type owl:Class ;
                        rdfs:subClassOf :R9TI5UbsBXnAYSIi17pJARr ,
                                        [ rdf:type owl:Restriction ;
                                          owl:onProperty elite:hasNext ;
                                          owl:someValuesFrom :RvJRwvUJjnFg7pvJ4yXd69
                                        ] ,
                                        [ rdf:type owl:Restriction ;
                                          owl:onProperty elite:isStageOf ;
                                          owl:someValuesFrom :RCP7vIugzt8V7rXL11buOZH
                                        ] ;
                        <http://www.w3.org/2004/02/skos/core#definition> "It is any event, in temporary order, between the initial and the final event of the sequence of the events in a nuclear accident" ;
                        <http://www.w3.org/2004/02/skos/core#prefLabel> "NuclearAccidentIntermediateEvent"@en .


###  http://w3id.org/emmo/domain/neo#RZtNAG3BL7lDm8L77EbEBd
:RZtNAG3BL7lDm8L77EbEBd rdf:type owl:Class ;
                        rdfs:subClassOf :RDoeQzvUClmOY7fNhDvK0L1 ,
                                        [ rdf:type owl:Restriction ;
                                          owl:onProperty elite:isConstituentOf ;
                                          owl:someValuesFrom :R85FFwLPHIursWfa6K6sKK9
                                        ] ;
                        rdfs:isDefinedBy "ISO 6107:2021(en) Water quality — Vocabulary ﻿" ;
                        <http://www.w3.org/2004/02/skos/core#altLabel> "ReactorDryWell﻿"@en ;
                        <http://www.w3.org/2004/02/skos/core#definition> "Chamber, below ground level, that remains dry, and houses pumping apparatus with its associated pipework and equipment."@en ;
                        <http://www.w3.org/2004/02/skos/core#prefLabel> "DryWell"@en .


###  http://w3id.org/emmo/domain/neo#Ra61ijkU0v73woMBs0urSn
:Ra61ijkU0v73woMBs0urSn rdf:type owl:Class ;
                        rdfs:subClassOf :RPURhpVoxOOYoC2J28Rgfd ,
                                        [ rdf:type owl:Restriction ;
                                          owl:onProperty elite:isInputOf ;
                                          owl:someValuesFrom :RBU28e2pgiTqsaTCPWnAJ6y
                                        ] ;
                        rdfs:isDefinedBy "IAEA Safety Glossary, Terminology Used in Nuclear Safety and Radiation Protection, 2018 Edition"@en ;
                        <http://www.w3.org/2004/02/skos/core#definition> "New fuel or unirradiated fuel, including fuel fabricated from fissionable material recovered by reprocessing previously irradiated fuel." ;
                        <http://www.w3.org/2004/02/skos/core#prefLabel> "Nuclear﻿FreshFuel"@en .


###  http://w3id.org/emmo/domain/neo#RaEj4uH02jwi8e78Nr9PvH
:RaEj4uH02jwi8e78Nr9PvH rdf:type owl:Class ;
                        rdfs:subClassOf :RBtkzbuLn6g0vdtDU3mijH0 ;
                        rdfs:seeAlso "INTERNATIONAL ATOMIC ENERGY AGENCY, Approaches for Overall Instrumentation and Control Architectures of Nuclear Power Plants, IAEA Nuclear Energy Series No. NP-T-2.11, IAEA, Vienna (2018)" ;
                        <http://www.w3.org/2004/02/skos/core#prefLabel> "PostulatedSingleEvent"@en .


###  http://w3id.org/emmo/domain/neo#RaKxhZBSqtO6ceVm10Ca6Y
:RaKxhZBSqtO6ceVm10Ca6Y rdf:type owl:Class ;
                        rdfs:subClassOf :R7Ss5qBF98KBgXN3rhg0rEl ,
                                        [ rdf:type owl:Restriction ;
                                          owl:onProperty elite:isConstituentOf ;
                                          owl:someValuesFrom :R0N27qMQzeRjM0vSOeAvUT
                                        ] ;
                        rdfs:isDefinedBy "ISO 20539:2023(en) Translation, interpreting and related technology — Vocabulary" ;
                        <http://www.w3.org/2004/02/skos/core#altLabel> "NppPublicAddressSystem"@en ,
                                                                       "PASystem"@en ,
                                                                       "SoundReinforcementSystem"@en ,
                                                                       "SpeechReinforcementSystem"@en ;
                        <http://www.w3.org/2004/02/skos/core#definition> "system (3.5.2.17) that amplifies sound (3.5.2.22)"@en ;
                        <http://www.w3.org/2004/02/skos/core#prefLabel> "PublicAddressSystem"@en .


###  http://w3id.org/emmo/domain/neo#RapiFOXlLXIKxdiWW4ljdc
:RapiFOXlLXIKxdiWW4ljdc rdf:type owl:Class ;
                        rdfs:subClassOf :RBtkzbuLn6g0vdtDU3mijH0 ;
                        rdfs:isDefinedBy <https://www.nrc.gov/docs/ML0707/ML070710376.pdf> ;
                        <http://www.w3.org/2004/02/skos/core#definition> """Unanticipated conditions of operation (i.e., not expected to occur
during the life of the nuclear power unit).
Postulated accidents are also known as Condition IV events.""" ;
                        <http://www.w3.org/2004/02/skos/core#prefLabel> "PostulatedAccident"@en .


###  http://w3id.org/emmo/domain/neo#Rba6gbJ70iyZgFOVY5Z6Vo
:Rba6gbJ70iyZgFOVY5Z6Vo rdf:type owl:Class ;
                        rdfs:subClassOf :RBBzyqSEv3bIRXZvqAVCF4x ,
                                        [ rdf:type owl:Restriction ;
                                          owl:onProperty elite:isBehaviourOf ;
                                          owl:someValuesFrom :RRVTDj2E9x5cjit7EQ9Dkx
                                        ] ;
                        :R8xx0dhbEh1tjGMDwNZfckV "Loss of those devices like batteries and solar panel that during SBO conditions are required to power a minimum set of critical equipment important to safety, as well as critical instrumentation for monitoring of plant parameters, and emergency lighting"@en ;
                        rdfs:isDefinedBy <https://www-pub.iaea.org/MTCD/Publications/PDF/TE-1770_web.pdf> ;
                        <http://www.w3.org/2004/02/skos/core#definition> "Loss of those devices like batteries and solar panel that during SBO conditions are required to power a minimum set of critical equipment important to safety, as well as critical instrumentation for monitoring of plant parameters, and emergency lighting"@en ;
                        <http://www.w3.org/2004/02/skos/core#prefLabel> "LossOfDCPower"@en .


###  http://w3id.org/emmo/domain/neo#RbscqwUSgWtKWJZrcgSNr9
:RbscqwUSgWtKWJZrcgSNr9 rdf:type owl:Class ;
                        rdfs:subClassOf :R91s5ihcKvYBOzeCaNlNVVK ;
                        rdfs:comment """The exact definition of ‘significant amounts’ would be a regulatory decision.
Material in which the activity concentrations of the naturally occurring radionuclides have been changed by a process is included in naturally occurring radioactive material (NORM).
 Naturally occurring radioactive material or NORM should be used in the singular unless reference is explicitly being made to various materials."""@en ;
                        rdfs:isDefinedBy """IAEA Safety Glossary, Terminology Used in Nuclear Safety 
and Radiation Protection, 2018 Edition """ ;
                        <http://www.w3.org/2004/02/skos/core#definition> "Radioactive material containing no significant amounts of radionuclides other than naturally occurring radionuclides.﻿"@en ;
                        <http://www.w3.org/2004/02/skos/core#prefLabel> "NaturallyOccurringRadioactiveMaterial"@en .


###  http://w3id.org/emmo/domain/neo#RdPoUW04SB1jvKPJcXoVCW
:RdPoUW04SB1jvKPJcXoVCW rdf:type owl:Class ;
                        rdfs:subClassOf :R95M6reIX3ya776PtOPLGmY ;
                        rdfs:isDefinedBy """ISO 26802:2010(en)
Nuclear facilities — Criteria for the design and the operation of containment and ventilation systems for nuclear reactors"""@en ;
                        <http://www.w3.org/2004/02/skos/core#altLabel> "SevereAccident"@en ;
                        <http://www.w3.org/2004/02/skos/core#definition> "accident conditions more severe than a design basis accident and involving significant core degradation"@en ;
                        <http://www.w3.org/2004/02/skos/core#prefLabel> "NuclearSevereAccident"@en .


###  http://w3id.org/emmo/domain/neo#ReAOaKplsxuu3rxqPb4Jz4
:ReAOaKplsxuu3rxqPb4Jz4 rdf:type owl:Class ;
                        rdfs:subClassOf :RDpEA8qdRk99FAT0xSGZgGS ;
                        rdfs:isDefinedBy """ISO 3977-9:1999(en)
Gas turbines — Procurement — Part 9: Reliability, availability, maintainability and safety""" ;
                        <http://www.w3.org/2004/02/skos/core#definition> "Removal of a unit from service to perform work on specific components that can be deferred beyond the end of the next weekend, but requires the unit be removed from service before the next planned outage."@en ;
                        <http://www.w3.org/2004/02/skos/core#prefLabel> "MaintenanceOutage"@en .


###  http://w3id.org/emmo/domain/neo#Rff5M43GHvSXYByyfZSSyk
:Rff5M43GHvSXYByyfZSSyk rdf:type owl:Class ;
                        rdfs:subClassOf :R0N27qMQzeRjM0vSOeAvUT ;
                        rdfs:isDefinedBy <https://www.iso.org/obp/ui#iso:std:iso:12749:-5:ed-1:v1:en:term:3.4.1.1> ;
                        <http://www.w3.org/2004/02/skos/core#altLabel> "SingleUnitNPP"@en ;
                        <http://www.w3.org/2004/02/skos/core#definition> "Nuclear power plant having a single electric production line (ISO 12749-5:2018)"@en ;
                        <http://www.w3.org/2004/02/skos/core#example> "Emsland Nuclear Power Plant (Lingen, Germany)"@en ;
                        <http://www.w3.org/2004/02/skos/core#prefLabel> "SingleUnitNuclearPowerPlant"@en .


###  http://w3id.org/emmo/domain/neo#RgAy137nXA9FNxJLdXeh2G
:RgAy137nXA9FNxJLdXeh2G rdf:type owl:Class ;
                        rdfs:subClassOf :Rryk3Z5XNZ11ZiiLuT5M8Q ;
                        rdfs:isDefinedBy """ISO 20043-1:2021(en)
Measurement of radioactivity in the environment — Guidelines for effective dose assessment using environmental monitoring data — Part 1: Planned and existing exposure situation""" ;
                        <http://www.w3.org/2004/02/skos/core#altLabel> "RadioactiveRelease"@en ;
                        <http://www.w3.org/2004/02/skos/core#definition> "Radioactive substances arising from a source (3.22) within a practice (3.13) which are discharged as gases, aerosols, liquids or solids to the environment, generally with the purpose of dilution and dispersion or disposal."@en ;
                        <http://www.w3.org/2004/02/skos/core#prefLabel> "RadioactiveDischarging"@en .


###  http://w3id.org/emmo/domain/neo#RiaJiI8PAvV7grwixkMCcr
:RiaJiI8PAvV7grwixkMCcr rdf:type owl:Class ;
                        rdfs:subClassOf elite:Object ,
                                        [ rdf:type owl:Restriction ;
                                          owl:onProperty elite:isConstituentOf ;
                                          owl:someValuesFrom :R0N27qMQzeRjM0vSOeAvUT
                                        ] ;
                        rdfs:isDefinedBy <https://www-pub.iaea.org/MTCD/Publications/PDF/P1526_Web.pdf> ,
                                         <https://www.iso.org/obp/ui#iso:std:iso:12749:-5:ed-1:v1:en:term:3.1.23> ;
                        <http://www.w3.org/2004/02/skos/core#definition> "A part of the nuclear power plant that consists of the containment, auxiliary and fuel building."@en ;
                        <http://www.w3.org/2004/02/skos/core#prefLabel> "NuclearIsland"@en .


###  http://w3id.org/emmo/domain/neo#RlYMwSSvmqekLRLzmf5IzV
:RlYMwSSvmqekLRLzmf5IzV rdf:type owl:Class ;
                        rdfs:subClassOf :R79WXwPF5ZWjRPArxbbVAgU ;
                        rdfs:isDefinedBy "ttps://www-ns.iaea.org/downloads/standards/glossary/iaea-safety-glossary-draft-2016.pdf" ;
                        <http://www.w3.org/2004/02/skos/core#altLabel> "FacilitiesOperation" ;
                        <http://www.w3.org/2004/02/skos/core#definition> """All activities performed to achieve the purpose for which an authorized facility was
constructed"""@en ;
                        <http://www.w3.org/2004/02/skos/core#prefLabel> "Operation"@en .


###  http://w3id.org/emmo/domain/neo#Rld2UEpLG7yzdQrBtq6RPL
:Rld2UEpLG7yzdQrBtq6RPL rdf:type owl:Class ;
                        rdfs:subClassOf :R7qv2nUGxSNZRvXyF3CXPTr ,
                                        [ rdf:type owl:Restriction ;
                                          owl:onProperty elite:isConstituentOf ;
                                          owl:someValuesFrom :R8KlSYQnSKI6PoJZNIdhwNI
                                        ] ;
                        rdfs:isDefinedBy <https://en.wikipedia.org/wiki/Hydrogen> ;
                        <http://www.w3.org/2004/02/skos/core#definition> "Itis a chemical element; it has symbol H and atomic number 1. It is the lightest element and, at standard conditions, is a gas of diatomic molecules with the formula H2. It is colorless, odorless, tasteless, non-toxic, and highly combustible. Hydrogen is the most abundant chemical substance in the universe, constituting roughly 75% of all normal matter."@en ;
                        <http://www.w3.org/2004/02/skos/core#prefLabel> "Hydrogen"@en .


###  http://w3id.org/emmo/domain/neo#RnTowd9AGtNiJRicoarsyr
:RnTowd9AGtNiJRicoarsyr rdf:type owl:Class ;
                        rdfs:subClassOf :R7ASmNcKrlRjzYHkUz3vfQT ;
                        rdfs:comment """The company has 3 nuclear power plants which in the past had provided up to 40% of the electricity needed by TEPCO and therefore Tokyo and its region:

Kashiwazaki Kariwa,
Fukushima Dai-ichi.
Fukushima Dai-ni,"""@en ;
                        rdfs:isDefinedBy <https://en.wikipedia.org/wiki/Tokyo_Electric_Power_Company> ;
                        <http://www.w3.org/2004/02/skos/core#altLabel> "TEPCO"@en ;
                        <http://www.w3.org/2004/02/skos/core#definition> "Tokyo Electric Power Company (東京電力株式会社?, Tōkyō Denryoku Kabushiki-gaisha), also known as Tōden (東電?) or TEPCO, is Japan's largest electric power company. Serving the Kantō region.﻿"@en ;
                        <http://www.w3.org/2004/02/skos/core#prefLabel> "TokyoElectricPowerCompany"@en .


###  http://w3id.org/emmo/domain/neo#RoO35j2Hgqm540PRLDF9Jy
:RoO35j2Hgqm540PRLDF9Jy rdf:type owl:Class ;
                        rdfs:subClassOf :R89Yy2V18LstH4xGXyNb9XN ,
                                        [ rdf:type owl:Restriction ;
                                          owl:onProperty :RB4rNlczhggIx7lqdEK2d9c ;
                                          owl:someValuesFrom :R8CzBJHXymJx05c6sDhbspt
                                        ] ;
                        rdfs:isDefinedBy <https://en.wikipedia.org/wiki/Electric_generator> ;
                        <http://www.w3.org/2004/02/skos/core#altLabel> "NPPGenerator"@en ;
                        <http://www.w3.org/2004/02/skos/core#definition> "In electricity generation, a generator is a device that converts motion-based power (potential and kinetic energy) or fuel-based power (chemical energy) into electric power for use in an external circuit. "@en ;
                        <http://www.w3.org/2004/02/skos/core#prefLabel> "Generator"@en .


###  http://w3id.org/emmo/domain/neo#RrfuHy45DxsWTOKgkP9TFG
:RrfuHy45DxsWTOKgkP9TFG rdf:type owl:Class ;
                        rdfs:subClassOf :RRPYBSdeHQObrzQD5UT74I ;
                        rdfs:isDefinedBy """ISO 7967-11:2022(en)
Reciprocating internal combustion engines — Vocabulary of components and systems — Part 11: Liquid fuel systems""" ;
                        <http://www.w3.org/2004/02/skos/core#definition> "irregular injection (3.3.69) with stoppage of fuel injection"@en ;
                        <http://www.w3.org/2004/02/skos/core#prefLabel> "IntermittentInjection"@en .


###  http://w3id.org/emmo/domain/neo#Rryk3Z5XNZ11ZiiLuT5M8Q
:Rryk3Z5XNZ11ZiiLuT5M8Q rdf:type owl:Class ;
                        rdfs:subClassOf :RtdecAtZ9C9xUJNtjefY4D ;
                        rdfs:isDefinedBy "INTERNATIONAL ATOMIC ENERGY AGENCY, Approaches for Overall Instrumentation and Control Architectures of Nuclear Power Plants, IAEA Nuclear Energy Series No. NP-T-2.11, IAEA, Vienna (2018) p.12" ;
                        <http://www.w3.org/2004/02/skos/core#altLabel> "Level5DiD"@en ;
                        <http://www.w3.org/2004/02/skos/core#definition> """Emergency management (e.g. monitoring of radioactive releases) to mitigate the consequences of radioactive
release. For this, the main functions are to understand what radiological materials are being released and in
which direction. Many of these functions may be, and perhaps need to be, entirely separate from the overall
I&C architecture."""@en ;
                        <http://www.w3.org/2004/02/skos/core#prefLabel> "EmergencyManagement"@en .


###  http://w3id.org/emmo/domain/neo#RtX7ESf673Z9eYoseycPyl
:RtX7ESf673Z9eYoseycPyl rdf:type owl:Class ;
                        rdfs:subClassOf elite:Role ,
                                        [ rdf:type owl:Restriction ;
                                          owl:onProperty elite:isConstituentOf ;
                                          owl:someValuesFrom :RyMmVkVf9zClluOSgfr1Rh
                                        ] ;
                        <http://www.w3.org/2004/02/skos/core#definition> "Any material that takes a part of a nuclear Core"@en ;
                        <http://www.w3.org/2004/02/skos/core#prefLabel> "ReactorCoreMaterial"@en .


###  http://w3id.org/emmo/domain/neo#RtdecAtZ9C9xUJNtjefY4D
:RtdecAtZ9C9xUJNtjefY4D rdf:type owl:Class ;
                        rdfs:subClassOf :RlYMwSSvmqekLRLzmf5IzV ,
                                        [ rdf:type owl:Restriction ;
                                          owl:onProperty elite:isSubProcessOf ;
                                          owl:someValuesFrom :RyLZ508FsJKMTIHvSNuJZk
                                        ] ;
                        rdfs:isDefinedBy """INTERNATIONAL ATOMIC ENERGY AGENCY, IAEA Safety Glossary, Terminology Used in Nuclear Safety and Radiation
Protection, 2018 Edition, IAEA, Vienna (in press).""" ;
                        <http://www.w3.org/2004/02/skos/core#definition> """A hierarchical deployment of different levels of diverse equipment and procedures to prevent the escalation
of anticipated operational occurrences and to maintain the effectiveness of physical barriers placed between
a radiation source or radioactive material and workers, members of the public or the environment, in
operational states and, for some barriers, in accident conditions"""@en ;
                        <http://www.w3.org/2004/02/skos/core#prefLabel> "DefenceinDepthProcedures"@en .


###  http://w3id.org/emmo/domain/neo#Rtq4tb3S29hdhJZtzFB2Bg
:Rtq4tb3S29hdhJZtzFB2Bg rdf:type owl:Class ;
                        rdfs:subClassOf :R84TLuFmfSZMhgSh0uL0LXk ;
                        rdfs:isDefinedBy <https://www.britannica.com/technology/radiation-measurement> ;
                        <http://www.w3.org/2004/02/skos/core#definition> "Technique for detecting the intensity and characteristics of ionizing radiation, such as alpha, beta, and gamma rays or neutrons, for the purpose of measurement."@en ;
                        <http://www.w3.org/2004/02/skos/core#prefLabel> "RadiationMeasurements"@en .


###  http://w3id.org/emmo/domain/neo#RvBQlxDEMRtFxiHtMstrYY
:RvBQlxDEMRtFxiHtMstrYY rdf:type owl:Class ;
                        rdfs:subClassOf :R7gZLWyPCimwGhHTueSRPhd ;
                        <http://www.w3.org/2004/02/skos/core#prefLabel> "SeaWaterCoolingSystem"@en .


###  http://w3id.org/emmo/domain/neo#RvJRwvUJjnFg7pvJ4yXd69
:RvJRwvUJjnFg7pvJ4yXd69 rdf:type owl:Class ;
                        rdfs:subClassOf :R9TI5UbsBXnAYSIi17pJARr ,
                                        [ rdf:type owl:Restriction ;
                                          owl:onProperty elite:isStageOf ;
                                          owl:someValuesFrom :RCP7vIugzt8V7rXL11buOZH
                                        ] ;
                        <http://www.w3.org/2004/02/skos/core#definition> "It is the last event, in temporary order, of the sequence of the events in a nuclear accident"@en ;
                        <http://www.w3.org/2004/02/skos/core#prefLabel> "NuclearAccidentFinalEvent"@en .


###  http://w3id.org/emmo/domain/neo#RvsRWyrgBeZBDE8PCeQpFd
:RvsRWyrgBeZBDE8PCeQpFd rdf:type owl:Class ;
                        rdfs:subClassOf :RBzruvoEUI9hIHVtX34kGJu ,
                                        :Rw4mCgviqd6HTitZEzST6w ,
                                        [ rdf:type owl:Restriction ;
                                          owl:onProperty elite:isConstituentOf ;
                                          owl:someValuesFrom :RDDFiZC2RFaE7RrTNF0CrtA
                                        ] ;
                        rdfs:comment """The alternative, using fire trucks connected to the FP water injection
port outside the TB, which had been installed in the previous year as a fire protection measure based on the experience of the Niigata-Chuetsu-Oki earthquake, was put into action."""@en ;
                        rdfs:seeAlso <https://fdada.info/develop/docs/pdf/ES-Unit123-04.pdf﻿> ,
                                     """Pag 19,  The Fukushima Daiichi Accident Technical Volume 1/5 
link: https://www-pub.iaea.org/MTCD/Publications/PDF/AdditionalVolumes/P1710/Pub1710-TV1-Web.pdf"""@en ;
                        <http://www.w3.org/2004/02/skos/core#altLabel> "ReactorFireProtectionWaterInjectionPort"@en ;
                        <http://www.w3.org/2004/02/skos/core#prefLabel> "FireProtectionWaterInjectionPort"@en .


###  http://w3id.org/emmo/domain/neo#RvstZtdRQckXTqUl1UK5Is
:RvstZtdRQckXTqUl1UK5Is rdf:type owl:Class ;
                        rdfs:subClassOf :R8lgbjRv5CeOJ43GygJ143n ;
                        rdfs:isDefinedBy <https://www.iso.org/obp/ui/en/#iso:std:iso:21650:ed-1:v1:en:term:2.76> ;
                        <http://www.w3.org/2004/02/skos/core#definition> "Long waves with the period of several minutes to one hour and the height up to a few tens of meters, which are generated by the vertical movement of sea floor associated with a submarine earthquake, by plunging of large mass of earth into water by land slide or volcanic eruption, and other causes."@en ;
                        <http://www.w3.org/2004/02/skos/core#prefLabel> "Tsunami"@en .


###  http://w3id.org/emmo/domain/neo#Rw4mCgviqd6HTitZEzST6w
:Rw4mCgviqd6HTitZEzST6w rdf:type owl:Class ;
                        rdfs:subClassOf :R7Ss5qBF98KBgXN3rhg0rEl ,
                                        [ rdf:type owl:Restriction ;
                                          owl:onProperty elite:participatesTo ;
                                          owl:someValuesFrom :R8PAMnGRP5NOBTguHsOmRSl
                                        ] ;
                        rdfs:comment "They fulfill their function as soon as the accident happened"@en ;
                        rdfs:seeAlso <https://www.iso.org/obp/ui/en/#iso:std:iso:ts:16901:ed-2:v1:en:term:3.20> ;
                        <http://www.w3.org/2004/02/skos/core#definition> "devices that aim to the limitation of any negative consequence (3.6) of a particular event"@en ;
                        <http://www.w3.org/2004/02/skos/core#prefLabel> "ReactorMitigationSystem"@en .


###  http://w3id.org/emmo/domain/neo#RxnLc7O29Jiy2Z0qg7iTh6
:RxnLc7O29Jiy2Z0qg7iTh6 rdf:type owl:Class ;
                        rdfs:subClassOf :R84TLuFmfSZMhgSh0uL0LXk ;
                        rdfs:isDefinedBy <https://en.wikipedia.org/wiki/Pressure_measurement> ;
                        <http://www.w3.org/2004/02/skos/core#definition> "Pressure measurement is the measurement of an applied force by a fluid (liquid or gas) on a surface"@en ;
                        <http://www.w3.org/2004/02/skos/core#prefLabel> "PressureMeasurement"@en .


###  http://w3id.org/emmo/domain/neo#RyLZ508FsJKMTIHvSNuJZk
:RyLZ508FsJKMTIHvSNuJZk rdf:type owl:Class ;
                        rdfs:subClassOf :RlYMwSSvmqekLRLzmf5IzV ;
                        <http://www.w3.org/2004/02/skos/core#definition> "The global process of manage the operation of a nuclear power plant, considering the design procedures" ;
                        <http://www.w3.org/2004/02/skos/core#prefLabel> "NPPOperationManagement"@en .


###  http://w3id.org/emmo/domain/neo#RyMmVkVf9zClluOSgfr1Rh
:RyMmVkVf9zClluOSgfr1Rh rdf:type owl:Class ;
                        rdfs:subClassOf elite:Whole ,
                                        :RDoeQzvUClmOY7fNhDvK0L1 ,
                                        [ rdf:type owl:Restriction ;
                                          owl:onProperty elite:isConstituentOf ;
                                          owl:someValuesFrom :RBW32C4x3sn1YahVG7uYVun
                                        ] ,
                                        [ rdf:type owl:Restriction ;
                                          owl:onProperty :RB4rNlczhggIx7lqdEK2d9c ;
                                          owl:someValuesFrom :RCRVu2hmIevYnx0eZzyJEPs
                                        ] ;
                        rdfs:isDefinedBy "ISO 12749-5:2018(en) Nuclear energy, nuclear technologies, and radiological protection — Vocabulary — Part 5: Nuclear reactors" ;
                        <http://www.w3.org/2004/02/skos/core#definition> """part of a nuclear reactor (3.1.22), where the fissionable nuclides (3.1.2) sustaining the fission chain are located
Note 1 to entry: In most cases, moderator (3.1.23.1.2) and coolant are also included in the reactor core (3.1.23.1)."""@en ;
                        <http://www.w3.org/2004/02/skos/core#prefLabel> "ReactorCore"@en .


#################################################################
#    Individuals
#################################################################

###  http://w3id.org/emmo/domain/neo#R4UMKMNvIkmVZ4OSRIQ6Qv
:R4UMKMNvIkmVZ4OSRIQ6Qv rdf:type owl:NamedIndividual ,
                                 :RDuDSbKh236WI6rqMad7Ar4 ;
                        elite:isConstitutiveProcessOf :R7uvG224iPqEldlfFwndlKr ;
                        <http://www.w3.org/2004/02/skos/core#prefLabel> "RCICActivation_unit2"@en .


###  http://w3id.org/emmo/domain/neo#R56puCaUpuR7eQFm7rEWOv
:R56puCaUpuR7eQFm7rEWOv rdf:type owl:NamedIndividual ,
                                 :RBwST6x27zdyWBgBunjc2Q9 ;
                        elite:hasNext :R7RRzaczCz4wVsf2ZSE3cz5 ;
                        elite:isConstitutiveProcessOf :R7uvG224iPqEldlfFwndlKr ;
                        <http://www.w3.org/2004/02/skos/core#prefLabel> "CRInsertion_Unit2"@en .


###  http://w3id.org/emmo/domain/neo#R5vADU834XOdmmbqErqMjD
:R5vADU834XOdmmbqErqMjD rdf:type owl:NamedIndividual ,
                                 :Rba6gbJ70iyZgFOVY5Z6Vo ;
                        elite:hasNext :R8BzCYxsJkpBVMzHmrLDfBN ;
                        elite:isBehaviourOf :R8nP70kb2tjsTW1qDOmrdbC ;
                        <http://www.w3.org/2004/02/skos/core#prefLabel> "DCPowerLoss_unit4"@en .


###  http://w3id.org/emmo/domain/neo#R71kogAKcOnrzKRRvJYzEnf
:R71kogAKcOnrzKRRvJYzEnf rdf:type owl:NamedIndividual ,
                                  :RC5Uc3vBrAsYC8gCNkTsLH ;
                         elite:hasNext :RCZSMiyXPZ1w9KtBMir31du ;
                         elite:isConstitutiveProcessOf :Rb5hP2Q5XG2czxqOFu5nb9 ;
                         <http://www.w3.org/2004/02/skos/core#prefLabel> "regularWaterInjection_unit3"@en .


###  http://w3id.org/emmo/domain/neo#R7MYrOmgGBYZ0JwNSP9CKGJ
:R7MYrOmgGBYZ0JwNSP9CKGJ rdf:type owl:NamedIndividual ,
                                  :R9j7jE0NWQS6xBqDD8iJRbf ;
                         elite:hasNext :R8SCvSsZInboPn0aMi5hJ2b ;
                         <http://www.w3.org/2004/02/skos/core#prefLabel> "RCICSystem_unit2"@en .


###  http://w3id.org/emmo/domain/neo#R7MkAFLocpCOTpR1W4846Wv
:R7MkAFLocpCOTpR1W4846Wv rdf:type owl:NamedIndividual ,
                                  :RDN44xs0tgwZS1p11BPMMKr ;
                         elite:hasNext :R5vADU834XOdmmbqErqMjD ;
                         elite:isBehaviourOf :R8nP70kb2tjsTW1qDOmrdbC ;
                         <http://www.w3.org/2004/02/skos/core#prefLabel> "ACPowerLoss_unit4"@en .


###  http://w3id.org/emmo/domain/neo#R7OojlUGWcg81Y4DnKKUYtE
:R7OojlUGWcg81Y4DnKKUYtE rdf:type owl:NamedIndividual ,
                                  :R8bUZpp1yY81qmfgGNH0TyF ;
                         elite:hasNext :RBnZe6rQs3iQOzfyrY5AKRG ;
                         elite:isBehaviourOf :RTiXMunsU6yEXKeRVxMuQV ;
                         elite:isConstitutiveProcessOf :R8nP70kb2tjsTW1qDOmrdbC ;
                         <http://www.w3.org/2004/02/skos/core#prefLabel> "closingMSIV_Unit4"@en .


###  http://w3id.org/emmo/domain/neo#R7RRzaczCz4wVsf2ZSE3cz5
:R7RRzaczCz4wVsf2ZSE3cz5 rdf:type owl:NamedIndividual ;
                         elite:affects :R7uvG224iPqEldlfFwndlKr ,
                                       :R8nP70kb2tjsTW1qDOmrdbC ,
                                       :R9icMA5hIFg4wyRyuVCUEYW ,
                                       :Rb5hP2Q5XG2czxqOFu5nb9 ;
                         elite:hasNext :R7OojlUGWcg81Y4DnKKUYtE ,
                                       :RBc3mI1yVMSGjTWyWdVvMiP ,
                                       :RBfahJ7XEvDRY0I74gA4EhW ,
                                       :RCJ4sUQgpXReJhv2l3TNlPt ;
                         <http://www.w3.org/2004/02/skos/core#prefLabel> "lossOfOffSitePower_Fukushima"@en .


###  http://w3id.org/emmo/domain/neo#R7RYQTRTJpydcZySPvfj97U
:R7RYQTRTJpydcZySPvfj97U rdf:type owl:NamedIndividual ,
                                  :RBwST6x27zdyWBgBunjc2Q9 ;
                         elite:hasNext :R7RRzaczCz4wVsf2ZSE3cz5 ;
                         elite:isConstitutiveProcessOf :R9icMA5hIFg4wyRyuVCUEYW ;
                         <http://www.w3.org/2004/02/skos/core#prefLabel> "CRInsertion_Unit1"@en .


###  http://w3id.org/emmo/domain/neo#R7TeIrUcoeFIohoZFYT6oHo
:R7TeIrUcoeFIohoZFYT6oHo rdf:type owl:NamedIndividual ,
                                  :R7t1vs1VKDAzHkcQsFbt9JC ;
                         elite:hasNext :R71kogAKcOnrzKRRvJYzEnf ,
                                       :RCIQAmGtY5oJHuuVHp7Y9OF ;
                         elite:isConstitutiveProcessOf :Rb5hP2Q5XG2czxqOFu5nb9 ;
                         <http://www.w3.org/2004/02/skos/core#prefLabel> "HPCIOperation_unit3"@en .


###  http://w3id.org/emmo/domain/neo#R7UHidTtMLlwJsXw3LunBVr
:R7UHidTtMLlwJsXw3LunBVr rdf:type owl:NamedIndividual ,
                                  :Rba6gbJ70iyZgFOVY5Z6Vo ;
                         elite:hasNext :R9ci3rSU9PmVM9hDoObI7GN ,
                                       :R9t3qBNc7hgSJ9CltHNvCc4 ;
                         elite:isBehaviourOf :R9icMA5hIFg4wyRyuVCUEYW ;
                         <http://www.w3.org/2004/02/skos/core#prefLabel> "DCPowerLoss_unit1"@en .


###  http://w3id.org/emmo/domain/neo#R7c6WbN81RxcJpHXeGHXv8
:R7c6WbN81RxcJpHXeGHXv8 rdf:type owl:NamedIndividual ,
                                 :RB5vIXZFuMYcHWSzNAPjPtF ;
                        elite:hasNext :RBKxneXt3UWJzKxOD5Inibz ;
                        elite:isBehaviourOf :R9icMA5hIFg4wyRyuVCUEYW ;
                        <http://www.w3.org/2004/02/skos/core#prefLabel> "lossOfUltimateHeatSink_unit1"@en .


###  http://w3id.org/emmo/domain/neo#R7uvG224iPqEldlfFwndlKr
:R7uvG224iPqEldlfFwndlKr rdf:type owl:NamedIndividual ,
                                  :RRKk7nTYd2pj3LFUG4j9yj ;
                         <http://www.w3.org/2004/02/skos/core#prefLabel> "unit_2"@en .


###  http://w3id.org/emmo/domain/neo#R7xpEdKwbxANkjtrQrh0ep
:R7xpEdKwbxANkjtrQrh0ep rdf:type owl:NamedIndividual ,
                                 :RCh38CRTgX4tnzCoB8auwPC ;
                        <http://www.w3.org/2004/02/skos/core#prefLabel> "dieselGenerator_Fukushima"@en .


###  http://w3id.org/emmo/domain/neo#R8BzCYxsJkpBVMzHmrLDfBN
:R8BzCYxsJkpBVMzHmrLDfBN rdf:type owl:NamedIndividual ,
                                  :RBq9x5WmblYOc4D7eFlfpdJ ;
                         elite:isBehaviourOf :R8nP70kb2tjsTW1qDOmrdbC ,
                                             :RDQ6WRHz0rKpRxnQ9WLdTh9 ;
                         <http://www.w3.org/2004/02/skos/core#prefLabel> "explosionOfReactorBuilding_unit4"@en .


###  http://w3id.org/emmo/domain/neo#R8MEESkThrtwrxXoXG6Fhjm
:R8MEESkThrtwrxXoXG6Fhjm rdf:type owl:NamedIndividual ,
                                  :R9MK7U9YLf7RtEpfQTDDr1q ;
                         <http://www.w3.org/2004/02/skos/core#prefLabel> "MSIV_Unit1"@en .


###  http://w3id.org/emmo/domain/neo#R8NisCJkeUXZCMxKr9tKNJq
:R8NisCJkeUXZCMxKr9tKNJq rdf:type owl:NamedIndividual ,
                                  :RCRVu2hmIevYnx0eZzyJEPs ;
                         elite:isConstituentOf :R9icMA5hIFg4wyRyuVCUEYW ;
                         <http://www.w3.org/2004/02/skos/core#prefLabel> "reactor_1_vessel"@en .


###  http://w3id.org/emmo/domain/neo#R8SCvSsZInboPn0aMi5hJ2b
:R8SCvSsZInboPn0aMi5hJ2b rdf:type owl:NamedIndividual ,
                                  :RvstZtdRQckXTqUl1UK5Is ;
                         elite:affects :R7uvG224iPqEldlfFwndlKr ,
                                       :R8nP70kb2tjsTW1qDOmrdbC ,
                                       :R9icMA5hIFg4wyRyuVCUEYW ,
                                       :Rb5hP2Q5XG2czxqOFu5nb9 ;
                         elite:hasNext :R7c6WbN81RxcJpHXeGHXv8 ,
                                       :R9om4FPZlN1Gg2qFReIfI60 ,
                                       :RMp5GbDdB45DJyWFDXk4qT ,
                                       :RsZEl0qfySUbopX7Z6mlXE ;
                         <http://www.w3.org/2004/02/skos/core#prefLabel> "tohokuTzunami"@en .


###  http://w3id.org/emmo/domain/neo#R8Yr6YUUe0lh5UU0KHqF8Or
:R8Yr6YUUe0lh5UU0KHqF8Or rdf:type owl:NamedIndividual ,
                                  :RlYMwSSvmqekLRLzmf5IzV ;
                         elite:hasNext :R4UMKMNvIkmVZ4OSRIQ6Qv ;
                         elite:isBehaviourOf :R9ww5067sycKsLf6pU7vT06 ;
                         <http://www.w3.org/2004/02/skos/core#prefLabel> "repeatedlyOpeningClosing_SRV_unit2"@en .


###  http://w3id.org/emmo/domain/neo#R8nP70kb2tjsTW1qDOmrdbC
:R8nP70kb2tjsTW1qDOmrdbC rdf:type owl:NamedIndividual ,
                                  :RRKk7nTYd2pj3LFUG4j9yj ;
                         <http://www.w3.org/2004/02/skos/core#prefLabel> "unit_4"@en .


###  http://w3id.org/emmo/domain/neo#R8wL8gWueAFQTEzJ4Rj2QKI
:R8wL8gWueAFQTEzJ4Rj2QKI rdf:type owl:NamedIndividual ,
                                  :R9MK7U9YLf7RtEpfQTDDr1q ,
                                  [ rdf:type owl:Restriction ;
                                    owl:onProperty :RB4rNlczhggIx7lqdEK2d9c ;
                                    owl:someValuesFrom :R0ZnwwPdidaBfZOg6tgZJr
                                  ] ,
                                  [ rdf:type owl:Restriction ;
                                    owl:onProperty :RB4rNlczhggIx7lqdEK2d9c ;
                                    owl:someValuesFrom :RZtNAG3BL7lDm8L77EbEBd
                                  ] ;
                         <http://www.w3.org/2004/02/skos/core#prefLabel> "MSIV_Unit2"@en .


###  http://w3id.org/emmo/domain/neo#R9Iwyc5qtHhh0QHOXsiris3
:R9Iwyc5qtHhh0QHOXsiris3 rdf:type owl:NamedIndividual ,
                                  :RDpEA8qdRk99FAT0xSGZgGS ;
                         elite:hasNext :RBHjDlLwaPMxKKtjq16Lw1c ;
                         elite:isBehaviourOf :R9icMA5hIFg4wyRyuVCUEYW ;
                         <http://www.w3.org/2004/02/skos/core#prefLabel> "NPPNormalOperationRatedPower_Unit1"@en .


###  http://w3id.org/emmo/domain/neo#R9L3ykUI6w5qe20x5hVL2mK
:R9L3ykUI6w5qe20x5hVL2mK rdf:type owl:NamedIndividual ,
                                  :RDuDSbKh236WI6rqMad7Ar4 ;
                         elite:hasNext :R7TeIrUcoeFIohoZFYT6oHo ;
                         elite:isConstitutiveProcessOf :Rb5hP2Q5XG2czxqOFu5nb9 ;
                         <http://www.w3.org/2004/02/skos/core#prefLabel> "RCICActivation_unit3"@en .


###  http://w3id.org/emmo/domain/neo#R9ci3rSU9PmVM9hDoObI7GN
:R9ci3rSU9PmVM9hDoObI7GN rdf:type owl:NamedIndividual ,
                                  :RC5Uc3vBrAsYC8gCNkTsLH ;
                         elite:hasNext :RPcjVut6ArBpfKG9sYPMsM ;
                         elite:isConstitutiveProcessOf :R9icMA5hIFg4wyRyuVCUEYW ;
                         <http://www.w3.org/2004/02/skos/core#prefLabel> "regularWaterInjection_unit1"@en .


###  http://w3id.org/emmo/domain/neo#R9d1EKHudbhPmfvQxlND3Wr
:R9d1EKHudbhPmfvQxlND3Wr rdf:type owl:NamedIndividual ,
                                  [ rdf:type owl:Restriction ;
                                    owl:onProperty elite:isBehaviourOf ;
                                    owl:someValuesFrom :RRVTDj2E9x5cjit7EQ9Dkx
                                  ] ;
                         elite:hasNext :RDAWOe94vcv6aVGTD0p8Rh6 ;
                         elite:isBehaviourOf :R7uvG224iPqEldlfFwndlKr ;
                         <http://www.w3.org/2004/02/skos/core#prefLabel> "DCPowerLoss_unit2"@en .


###  http://w3id.org/emmo/domain/neo#R9icMA5hIFg4wyRyuVCUEYW
:R9icMA5hIFg4wyRyuVCUEYW rdf:type owl:NamedIndividual ,
                                  :RRKk7nTYd2pj3LFUG4j9yj ;
                         <http://www.w3.org/2004/02/skos/core#prefLabel> "unit_1"@en .


###  http://w3id.org/emmo/domain/neo#R9lguEUksKNv9gLzWkqBDJ4
:R9lguEUksKNv9gLzWkqBDJ4 rdf:type owl:NamedIndividual ,
                                  :RDN44xs0tgwZS1p11BPMMKr ;
                         elite:hasNext :R9L3ykUI6w5qe20x5hVL2mK ;
                         elite:isBehaviourOf :Rb5hP2Q5XG2czxqOFu5nb9 ;
                         <http://www.w3.org/2004/02/skos/core#prefLabel> "ACPowerLoss_unit3"@en .


###  http://w3id.org/emmo/domain/neo#R9om4FPZlN1Gg2qFReIfI60
:R9om4FPZlN1Gg2qFReIfI60 rdf:type owl:NamedIndividual ,
                                  :RB5vIXZFuMYcHWSzNAPjPtF ;
                         elite:hasNext :R9lguEUksKNv9gLzWkqBDJ4 ;
                         elite:isBehaviourOf :Rb5hP2Q5XG2czxqOFu5nb9 ;
                         <http://www.w3.org/2004/02/skos/core#prefLabel> "lossOfUltimateHeatSink_unit3"@en .


###  http://w3id.org/emmo/domain/neo#R9t3qBNc7hgSJ9CltHNvCc4
:R9t3qBNc7hgSJ9CltHNvCc4 rdf:type owl:NamedIndividual ,
                                  :R8FmlobZiHsCZi4CHKxgtMg ;
                         elite:hasNext :RPcjVut6ArBpfKG9sYPMsM ;
                         elite:isConstitutiveProcessOf :R9icMA5hIFg4wyRyuVCUEYW ;
                         <http://www.w3.org/2004/02/skos/core#prefLabel> "SCVentilation_unit1"@en .


###  http://w3id.org/emmo/domain/neo#R9ww5067sycKsLf6pU7vT06
:R9ww5067sycKsLf6pU7vT06 rdf:type owl:NamedIndividual ,
                                  [ rdf:type owl:Restriction ;
                                    owl:onProperty :RB4rNlczhggIx7lqdEK2d9c ;
                                    owl:someValuesFrom :R0ZnwwPdidaBfZOg6tgZJr
                                  ] ;
                         <http://www.w3.org/2004/02/skos/core#prefLabel> "SRV_unit2"@en .


###  http://w3id.org/emmo/domain/neo#RB4janzOcDoxSfpU6974nab
:RB4janzOcDoxSfpU6974nab rdf:type owl:NamedIndividual ,
                                  :R7pKuzitkkIAgc5NxDlqfH4 ;
                         elite:hasNext :R8Yr6YUUe0lh5UU0KHqF8Or ;
                         elite:isConstitutiveProcessOf :R7uvG224iPqEldlfFwndlKr ;
                         <http://www.w3.org/2004/02/skos/core#prefLabel> "pressureIncreasing_Unit2"@en .


###  http://w3id.org/emmo/domain/neo#RB9SU6UpAJ8MygM1uCXbEzt
:RB9SU6UpAJ8MygM1uCXbEzt rdf:type owl:NamedIndividual ,
                                  [ rdf:type owl:Restriction ;
                                    owl:onProperty elite:isConstitutiveProcessOf ;
                                    owl:someValuesFrom :R0N27qMQzeRjM0vSOeAvUT
                                  ] ;
                         elite:hasNext :RBHjDlLwaPMxKKtjq16Lw1c ;
                         elite:isBehaviourOf :R7uvG224iPqEldlfFwndlKr ;
                         <http://www.w3.org/2004/02/skos/core#prefLabel> "NPPNormalOperationRatedPower_Unit2"@en .


###  http://w3id.org/emmo/domain/neo#RBEpkkG2mXF3wnnZPT5lDoa
:RBEpkkG2mXF3wnnZPT5lDoa rdf:type owl:NamedIndividual ,
                                  :RDGBzCkWozL4RpG1CuIzwPi ;
                         elite:hasNext :R8BzCYxsJkpBVMzHmrLDfBN ;
                         <http://www.w3.org/2004/02/skos/core#prefLabel> "HydrogenRelease_unit3"@en .


###  http://w3id.org/emmo/domain/neo#RBHjDlLwaPMxKKtjq16Lw1c
:RBHjDlLwaPMxKKtjq16Lw1c rdf:type owl:NamedIndividual ,
                                  :RCcdLHL2BqdRJQkmiKL4MDW ;
                         elite:affects :R7uvG224iPqEldlfFwndlKr ,
                                       :R8nP70kb2tjsTW1qDOmrdbC ,
                                       :R9icMA5hIFg4wyRyuVCUEYW ,
                                       :Rb5hP2Q5XG2czxqOFu5nb9 ;
                         elite:hasNext :R56puCaUpuR7eQFm7rEWOv ,
                                       :R7RRzaczCz4wVsf2ZSE3cz5 ,
                                       :R7RYQTRTJpydcZySPvfj97U ,
                                       :RDmRDuXNQJPOriCxkLUlrUE ;
                         <http://www.w3.org/2004/02/skos/core#prefLabel> "tohokuEarthquake"@en .


###  http://w3id.org/emmo/domain/neo#RBKxneXt3UWJzKxOD5Inibz
:RBKxneXt3UWJzKxOD5Inibz rdf:type owl:NamedIndividual ,
                                  :RDN44xs0tgwZS1p11BPMMKr ;
                         elite:hasNext :R7UHidTtMLlwJsXw3LunBVr ;
                         elite:isBehaviourOf :R9icMA5hIFg4wyRyuVCUEYW ;
                         <http://www.w3.org/2004/02/skos/core#prefLabel> "ACPowerLoss_unit1"@en .


###  http://w3id.org/emmo/domain/neo#RBc3mI1yVMSGjTWyWdVvMiP
:RBc3mI1yVMSGjTWyWdVvMiP rdf:type owl:NamedIndividual ,
                                  [ rdf:type owl:Restriction ;
                                    owl:onProperty elite:isBehaviourOf ;
                                    owl:someValuesFrom :RBsAUchYFBwAtcVUeFr8EFq
                                  ] ;
                         elite:hasNext :RBnZe6rQs3iQOzfyrY5AKRG ;
                         elite:isBehaviourOf :RBrcoh6pN7tToFnM1m59yXl ;
                         elite:isConstitutiveProcessOf :Rb5hP2Q5XG2czxqOFu5nb9 ;
                         <http://www.w3.org/2004/02/skos/core#prefLabel> "closingMSIV_Unit3"@en .


###  http://w3id.org/emmo/domain/neo#RBfahJ7XEvDRY0I74gA4EhW
:RBfahJ7XEvDRY0I74gA4EhW rdf:type owl:NamedIndividual ,
                                  [ rdf:type owl:Restriction ;
                                    owl:onProperty elite:isBehaviourOf ;
                                    owl:someValuesFrom :RBsAUchYFBwAtcVUeFr8EFq
                                  ] ;
                         elite:hasNext :RBnZe6rQs3iQOzfyrY5AKRG ;
                         elite:isBehaviourOf :R8wL8gWueAFQTEzJ4Rj2QKI ;
                         elite:isConstitutiveProcessOf :R7uvG224iPqEldlfFwndlKr ;
                         <http://www.w3.org/2004/02/skos/core#prefLabel> "closingMSIV_Unit2"@en .


###  http://w3id.org/emmo/domain/neo#RBnZe6rQs3iQOzfyrY5AKRG
:RBnZe6rQs3iQOzfyrY5AKRG rdf:type owl:NamedIndividual ,
                                  :RDuDSbKh236WI6rqMad7Ar4 ;
                         elite:affects :R7uvG224iPqEldlfFwndlKr ,
                                       :R8nP70kb2tjsTW1qDOmrdbC ,
                                       :R9icMA5hIFg4wyRyuVCUEYW ,
                                       :Rb5hP2Q5XG2czxqOFu5nb9 ;
                         elite:hasNext :R8SCvSsZInboPn0aMi5hJ2b ,
                                       :RB4janzOcDoxSfpU6974nab ,
                                       :RC2M3wEsCROuuDC6Bjz9TLz ,
                                       :RC6oDea7metjydM6Dr1mJsi ;
                         elite:isBehaviourOf :R7xpEdKwbxANkjtrQrh0ep ;
                         <http://www.w3.org/2004/02/skos/core#prefLabel> "dieselGeneratorActivation_Fukushima"@en .


###  http://w3id.org/emmo/domain/neo#RBrcoh6pN7tToFnM1m59yXl
:RBrcoh6pN7tToFnM1m59yXl rdf:type owl:NamedIndividual ,
                                  :R9MK7U9YLf7RtEpfQTDDr1q ,
                                  [ rdf:type owl:Restriction ;
                                    owl:onProperty :RB4rNlczhggIx7lqdEK2d9c ;
                                    owl:someValuesFrom :R0ZnwwPdidaBfZOg6tgZJr
                                  ] ,
                                  [ rdf:type owl:Restriction ;
                                    owl:onProperty :RB4rNlczhggIx7lqdEK2d9c ;
                                    owl:someValuesFrom :RZtNAG3BL7lDm8L77EbEBd
                                  ] ;
                         <http://www.w3.org/2004/02/skos/core#prefLabel> "MSIV_Unit3"@en .


###  http://w3id.org/emmo/domain/neo#RC2M3wEsCROuuDC6Bjz9TLz
:RC2M3wEsCROuuDC6Bjz9TLz rdf:type owl:NamedIndividual ,
                                  :R7pKuzitkkIAgc5NxDlqfH4 ;
                         elite:hasNext :RCSOjPEJEBrRfStCCjfidCL ;
                         elite:isConstitutiveProcessOf :R9icMA5hIFg4wyRyuVCUEYW ;
                         <http://www.w3.org/2004/02/skos/core#prefLabel> "pressureIncreasing_Unit1"@en .


###  http://w3id.org/emmo/domain/neo#RC6oDea7metjydM6Dr1mJsi
:RC6oDea7metjydM6Dr1mJsi rdf:type owl:NamedIndividual ;
                         elite:hasNext :RFvEhkHbiPwVuY8AasDXll ;
                         elite:isConstitutiveProcessOf :Rb5hP2Q5XG2czxqOFu5nb9 ;
                         <http://www.w3.org/2004/02/skos/core#prefLabel> "pressureIncreasing_Unit3"@en .


###  http://w3id.org/emmo/domain/neo#RCGLvp3oNj6WAo2tvVy7DeU
:RCGLvp3oNj6WAo2tvVy7DeU rdf:type owl:NamedIndividual ,
                                  :R7twPwtQmmXFTKrDWM3POCD ;
                         <http://www.w3.org/2004/02/skos/core#prefLabel> "ICSystem_unit1"@en .


###  http://w3id.org/emmo/domain/neo#RCGk9WIE1u7wKk5PswM0eOU
:RCGk9WIE1u7wKk5PswM0eOU rdf:type owl:NamedIndividual ,
                                  :R0ZnwwPdidaBfZOg6tgZJr ;
                         <http://www.w3.org/2004/02/skos/core#prefLabel> "reactorBuilding_unit3"@en .


###  http://w3id.org/emmo/domain/neo#RCIQAmGtY5oJHuuVHp7Y9OF
:RCIQAmGtY5oJHuuVHp7Y9OF rdf:type owl:NamedIndividual ,
                                  :R8FmlobZiHsCZi4CHKxgtMg ;
                         elite:hasNext :RBEpkkG2mXF3wnnZPT5lDoa ,
                                       :RCZSMiyXPZ1w9KtBMir31du ;
                         elite:isConstitutiveProcessOf :Rb5hP2Q5XG2czxqOFu5nb9 ;
                         <http://www.w3.org/2004/02/skos/core#prefLabel> "SCVentilation_unit3"@en .


###  http://w3id.org/emmo/domain/neo#RCJ4sUQgpXReJhv2l3TNlPt
:RCJ4sUQgpXReJhv2l3TNlPt rdf:type owl:NamedIndividual ,
                                  :R8bUZpp1yY81qmfgGNH0TyF ;
                         elite:hasNext :RBnZe6rQs3iQOzfyrY5AKRG ;
                         elite:isBehaviourOf :R8MEESkThrtwrxXoXG6Fhjm ;
                         elite:isConstitutiveProcessOf :R9icMA5hIFg4wyRyuVCUEYW ;
                         <http://www.w3.org/2004/02/skos/core#prefLabel> "closingMSIV_Unit1"@en .


###  http://w3id.org/emmo/domain/neo#RCOfDWUyHIup4OUW4FsBUNW
:RCOfDWUyHIup4OUW4FsBUNW rdf:type owl:NamedIndividual ,
                                  :RDM3Wmp5f6fMXTDpEK3Dmsx ;
                         <http://www.w3.org/2004/02/skos/core#altLabel> "SafetyReliefValve_unit3" ;
                         <http://www.w3.org/2004/02/skos/core#prefLabel> "SRV_unit3"@en .


###  http://w3id.org/emmo/domain/neo#RCSOjPEJEBrRfStCCjfidCL
:RCSOjPEJEBrRfStCCjfidCL rdf:type owl:NamedIndividual ,
                                  :RDuDSbKh236WI6rqMad7Ar4 ;
                         elite:hasNext :R8SCvSsZInboPn0aMi5hJ2b ;
                         elite:isBehaviourOf :RCGLvp3oNj6WAo2tvVy7DeU ;
                         elite:isConstitutiveProcessOf :R9icMA5hIFg4wyRyuVCUEYW ;
                         <http://www.w3.org/2004/02/skos/core#prefLabel> "ICActivation_unit1"@en .


###  http://w3id.org/emmo/domain/neo#RCZSMiyXPZ1w9KtBMir31du
:RCZSMiyXPZ1w9KtBMir31du rdf:type owl:NamedIndividual ,
                                  :RBq9x5WmblYOc4D7eFlfpdJ ;
                         elite:hasNext :Rld8nnNRbLNp5DMRfVK1Hs ;
                         elite:isBehaviourOf :RCGk9WIE1u7wKk5PswM0eOU ;
                         elite:isConstitutiveProcessOf :Rb5hP2Q5XG2czxqOFu5nb9 ;
                         <http://www.w3.org/2004/02/skos/core#prefLabel> "explosionOfReactorBuilding_unit3"@en .


###  http://w3id.org/emmo/domain/neo#RDAWOe94vcv6aVGTD0p8Rh6
:RDAWOe94vcv6aVGTD0p8Rh6 rdf:type owl:NamedIndividual ,
                                  :RRPYBSdeHQObrzQD5UT74I ;
                         elite:isConstitutiveProcessOf :R7uvG224iPqEldlfFwndlKr ;
                         <http://www.w3.org/2004/02/skos/core#prefLabel> "irregularWaterInjection_unit2"@en .


###  http://w3id.org/emmo/domain/neo#RDNEIxMazl0JpSeCgw0Nxqo
:RDNEIxMazl0JpSeCgw0Nxqo rdf:type owl:NamedIndividual ,
                                  :RDpEA8qdRk99FAT0xSGZgGS ;
                         elite:hasNext :RBHjDlLwaPMxKKtjq16Lw1c ;
                         elite:isBehaviourOf :R8nP70kb2tjsTW1qDOmrdbC ;
                         <http://www.w3.org/2004/02/skos/core#prefLabel> "NPPNormalOperation_noFuel"@en .


###  http://w3id.org/emmo/domain/neo#RDQ6WRHz0rKpRxnQ9WLdTh9
:RDQ6WRHz0rKpRxnQ9WLdTh9 rdf:type owl:NamedIndividual ,
                                  :R0ZnwwPdidaBfZOg6tgZJr ;
                         <http://www.w3.org/2004/02/skos/core#prefLabel> "reactorBuilding_unit4"@en .


###  http://w3id.org/emmo/domain/neo#RDmRDuXNQJPOriCxkLUlrUE
:RDmRDuXNQJPOriCxkLUlrUE rdf:type owl:NamedIndividual ,
                                  :RBwST6x27zdyWBgBunjc2Q9 ;
                         elite:hasNext :R7RRzaczCz4wVsf2ZSE3cz5 ;
                         elite:isConstitutiveProcessOf :Rb5hP2Q5XG2czxqOFu5nb9 ;
                         <http://www.w3.org/2004/02/skos/core#prefLabel> "CRInsertion_Unit3"@en .


###  http://w3id.org/emmo/domain/neo#RFvEhkHbiPwVuY8AasDXll
:RFvEhkHbiPwVuY8AasDXll rdf:type owl:NamedIndividual ,
                                 :RlYMwSSvmqekLRLzmf5IzV ;
                        elite:hasNext :R9L3ykUI6w5qe20x5hVL2mK ;
                        elite:isBehaviourOf :RCOfDWUyHIup4OUW4FsBUNW ;
                        <http://www.w3.org/2004/02/skos/core#prefLabel> "repeatedlyOpeningClosing_SRV_unit3"@en .


###  http://w3id.org/emmo/domain/neo#RMp5GbDdB45DJyWFDXk4qT
:RMp5GbDdB45DJyWFDXk4qT rdf:type owl:NamedIndividual ,
                                 :RB5vIXZFuMYcHWSzNAPjPtF ;
                        elite:hasNext :RVDTdBhCWWXCt9qvBB5o8o ;
                        elite:isBehaviourOf :R7uvG224iPqEldlfFwndlKr ;
                        <http://www.w3.org/2004/02/skos/core#prefLabel> "lossOfUltimateHeatSink_unit2"@en .


###  http://w3id.org/emmo/domain/neo#RPcjVut6ArBpfKG9sYPMsM
:RPcjVut6ArBpfKG9sYPMsM rdf:type owl:NamedIndividual ,
                                 :RBq9x5WmblYOc4D7eFlfpdJ ;
                        elite:hasNext :RXcgBdYtloBN8Exe0yyXMw ;
                        elite:isBehaviourOf :R9icMA5hIFg4wyRyuVCUEYW ,
                                            :RUsOGEERLNgPu3mgta5Sm1 ;
                        <http://www.w3.org/2004/02/skos/core#prefLabel> "explosionOfReactorBuilding_unit1"@en .


###  http://w3id.org/emmo/domain/neo#RPlulHioiJxZgZC1QMUgOL
:RPlulHioiJxZgZC1QMUgOL rdf:type owl:NamedIndividual ,
                                 :R9j7jE0NWQS6xBqDD8iJRbf ,
                                 [ rdf:type owl:Restriction ;
                                   owl:onProperty :RB4rNlczhggIx7lqdEK2d9c ;
                                   owl:someValuesFrom :R0ZnwwPdidaBfZOg6tgZJr
                                 ] ;
                        elite:hasNext :R8SCvSsZInboPn0aMi5hJ2b ;
                        <http://www.w3.org/2004/02/skos/core#prefLabel> "RCICSystem_unit3"@en .


###  http://w3id.org/emmo/domain/neo#RTiXMunsU6yEXKeRVxMuQV
:RTiXMunsU6yEXKeRVxMuQV rdf:type owl:NamedIndividual ,
                                 :R9MK7U9YLf7RtEpfQTDDr1q ;
                        <http://www.w3.org/2004/02/skos/core#prefLabel> "MSIV_Unit4"@en .


###  http://w3id.org/emmo/domain/neo#RUsOGEERLNgPu3mgta5Sm1
:RUsOGEERLNgPu3mgta5Sm1 rdf:type owl:NamedIndividual ,
                                 :R0ZnwwPdidaBfZOg6tgZJr ;
                        <http://www.w3.org/2004/02/skos/core#prefLabel> "reactorBuilding_unit1"@en .


###  http://w3id.org/emmo/domain/neo#RVDTdBhCWWXCt9qvBB5o8o
:RVDTdBhCWWXCt9qvBB5o8o rdf:type owl:NamedIndividual ;
                        elite:hasNext :R4UMKMNvIkmVZ4OSRIQ6Qv ;
                        elite:isBehaviourOf :R7uvG224iPqEldlfFwndlKr ;
                        <http://www.w3.org/2004/02/skos/core#prefLabel> "ACPowerLoss_unit2"@en .


###  http://w3id.org/emmo/domain/neo#RXcgBdYtloBN8Exe0yyXMw
:RXcgBdYtloBN8Exe0yyXMw rdf:type owl:NamedIndividual ,
                                 :RRPYBSdeHQObrzQD5UT74I ;
                        elite:isConstitutiveProcessOf :R9icMA5hIFg4wyRyuVCUEYW ;
                        <http://www.w3.org/2004/02/skos/core#prefLabel> "irregularWaterInjection_unit1"@en .


###  http://w3id.org/emmo/domain/neo#RaHh8VTYDHA1krUVvo6jGG
:RaHh8VTYDHA1krUVvo6jGG rdf:type owl:NamedIndividual ,
                                 :RRKk7nTYd2pj3LFUG4j9yj ;
                        elite:hasNext :RBHjDlLwaPMxKKtjq16Lw1c ;
                        elite:isBehaviourOf :Rb5hP2Q5XG2czxqOFu5nb9 ;
                        <http://www.w3.org/2004/02/skos/core#prefLabel> "NPPNormalOperationRatedPower_Unit3" .


###  http://w3id.org/emmo/domain/neo#Rb5hP2Q5XG2czxqOFu5nb9
:Rb5hP2Q5XG2czxqOFu5nb9 rdf:type owl:NamedIndividual ,
                                 :RRKk7nTYd2pj3LFUG4j9yj ;
                        <http://www.w3.org/2004/02/skos/core#prefLabel> "unit_3"@en .


###  http://w3id.org/emmo/domain/neo#Rld8nnNRbLNp5DMRfVK1Hs
:Rld8nnNRbLNp5DMRfVK1Hs rdf:type owl:NamedIndividual ,
                                 :RRPYBSdeHQObrzQD5UT74I ;
                        elite:isConstitutiveProcessOf :Rb5hP2Q5XG2czxqOFu5nb9 ;
                        <http://www.w3.org/2004/02/skos/core#prefLabel> "irregularWaterInjection_unit3"@en .


###  http://w3id.org/emmo/domain/neo#RsZEl0qfySUbopX7Z6mlXE
:RsZEl0qfySUbopX7Z6mlXE rdf:type owl:NamedIndividual ,
                                 :RB5vIXZFuMYcHWSzNAPjPtF ;
                        elite:hasNext :R7MkAFLocpCOTpR1W4846Wv ;
                        elite:isBehaviourOf :R8nP70kb2tjsTW1qDOmrdbC ;
                        <http://www.w3.org/2004/02/skos/core#prefLabel> "lossOfUltimateHeatSink_unit4"@en .


###  Generated by the OWL API (version 4.5.26.2023-07-17T20:34:13Z) https://github.com/owlcs/owlapi
